new_proof/TermOrdering.v
@@ -3,103 +3,688 @@ From Coq Require Import Logic.ClassicalFacts.
 From Coq Require Import Classical.
 From CT Require Import CoreLang.
 From CT Require Import CoreLangProp.
-From CT Require Import OperationalSemantics.
+From CT Require Import OperationalSemanticsProp.
+From CT Require Import ErrOperationalSemanticsProp.
+From CT Require Import BasicTypingProp.
+From CT Require Import SyntaxSugar.
 
 Import Atom.
 Import CoreLang.
 Import Tactics.
 Import NamelessTactics.
 Import OperationalSemantics.
+Import OperationalSemanticsProp.
+Import ErrOperationalSemantics.
+Import ErrOperationalSemanticsProp.
+Import BasicTyping.
+Import ListCtx.
+Import SyntaxSugar.
 
-Definition termR: relation tm := fun (e e': tm) => forall (v: value), e ↪* v -> e' ↪* v.
-Notation " e1 '<-<' e2 " := (termR e1 e2) (at level 10).
-Notation " e1 '>=<' e2 " := (termR e1 e2 /\ termR e2 e1) (at level 10).
+Definition env := listctx value.
+Fixpoint tm_msubst (ss:env) (t:tm) : tm :=
+  match ss with
+  | nil => t
+  | ((x,s)::ss') => tm_msubst ss' ({x := s}t t)
+  end.
 
-#[global]
-Instance termR_refl: Reflexive termR.
-Proof. intros e v. auto. Qed.
-Arguments termR_refl /.
+Fixpoint value_msubst (ss:env) (t:value) : value :=
+  match ss with
+  | nil => t
+  | ((x,s)::ss') => value_msubst ss' ({x := s}v t)
+  end.
 
-#[global]
-Instance termR_trans: Transitive termR.
-Proof. intros e1 e2 e3. unfold termR. intros. auto. Qed.
-Arguments termR_trans /.
+Inductive instantiation : (listctx ty) -> env -> Prop :=
+| instantiation_nil: instantiation [] []
+| instantiation_cons: forall x T (v: value) c e,
+    [] ⊢t v ⋮v T ->
+    x ∉ ctxdom c ->
+    instantiation c e ->
+    instantiation ((x, T) :: c) ((x, v) :: e).
 
+Global Hint Constructors instantiation: core.
 
-Lemma let_reduction_spec_forward_one_step: forall (e_x: tm) e (e': tm),
-    tlete e_x e ↪ e' -> (exists (v_x: value), e_x = v_x /\ e' = e ^t^ v_x) \/ (exists (e_x': tm), e_x ↪ e_x' /\ e' = tlete e_x' e).
+Lemma instantiation_regular_ok: forall Γt Γv, instantiation Γt Γv -> ctxdom Γt = ctxdom Γv /\ ok Γt /\ ok Γv.
 Proof.
-  intros.
-  inversion H; subst; clear H.
-  - right. exists e1'. split; auto.
-  - left. exists v1. split; auto.
+  intros. induction H; repeat destruct_hyp_conj; repeat split; intros; auto;
+    try  listctx_set_solver;
+  try (simpl; rewrite H2; auto; try listctx_set_solver).
+  - rewrite ok_pre_destruct; split; auto. rewrite <- H2; auto.
 Qed.
 
-(* Need logical relation *)
-
-Lemma let_reduction_spec_forward: forall (e_x: tm),
-    lc e_x ->
-    (forall e (v: value),
-        (tlete e_x e ↪* v -> exists (v_x: value), e_x ↪* v_x /\ e ^t^ v_x ↪* v)).
+Lemma instantiation_regular_lc: forall Γt Γv, instantiation Γt Γv -> (forall x v, ctxfind Γv x = Some v -> lc v).
 Proof.
-  intros e_x H.
-  induction H; intros.
-  - admit.
-  - admit.
-  - admit.
-  - admit.
-  - admit.
-  - admit.
-  - 
+  intros. assert (ok Γv). apply instantiation_regular_ok in H. repeat destruct_hyp_conj; auto.
+  induction H; simpl; auto.
+  - simpl in H0. listctx_set_solver.
+  - simpl in H0. repeat var_dec_solver; basic_typing_solver.
+Qed.
 
-  induction e_x; intros.
-  - op_simpl.
-  - op_simpl. eexists. split; eauto.
-  - 
-
-
-
-
-Lemma let_reduction_spec_forward: forall (e_x: tm) e (v: value),
-    (tlete e_x e ↪* v -> exists (v_x: value), e_x ↪* v_x /\ e ^t^ v_x ↪* v).
+Lemma instantiation_regular_closed: forall Γt Γv, instantiation Γt Γv -> (forall x v, ctxfind Γv x = Some v -> closed_value v).
 Proof.
-  induction e_x; induction e; intros; try op_simpl; try (op_simpl; eexists; split; eauto).
-  - admit.
-  - op_simpl.
-    
-    end.
-      exists v. split; auto.
-  - op_simpl.
-  - op_simpl. eexists. split; eauto.
-  - specialize (IHe_x1 e_x2)
+  intros. assert (ok Γv). apply instantiation_regular_ok in H. repeat destruct_hyp_conj; auto.
+  induction H; auto.
+  - listctx_set_solver.
+  - simpl in H0. repeat var_dec_solver;
+    basic_typing_solver3.
+Qed.
 
-Lemma let_reduction_spec_forward: forall (e_x: tm) e (v: value),
-    (tlete e_x e ↪* v -> exists (v_x: value), e_x ↪* v_x /\ e ^t^ v_x ↪* v).
+Lemma instantiation_regular: forall Γt Γv, instantiation Γt Γv ->
+                                      (forall x v, ctxfind Γv x = Some v -> lc v) /\
+                                        (forall x v, ctxfind Γv x = Some v -> closed_value v) /\
+                                        ctxdom Γt = ctxdom Γv /\ ok Γt /\ ok Γv.
 Proof.
-  induction e_x; intros.
-  - op_simpl.
-  - op_simpl. eexists. split; eauto.
-  - 
+  intros. split.
+  eapply instantiation_regular_lc; eauto.
+  split.
+  eapply instantiation_regular_closed; eauto.
+  apply instantiation_regular_ok; auto.
+Qed.
 
-    
 
-    admit.
-  - 
+Lemma tm_msubst_closed: ∀ e, closed_tm e -> (forall ss, tm_msubst ss e = e).
+Proof.
+  unfold closed_tm.
   intros.
-  induction H0. admit.
+  induction ss; simpl; auto.
+  destruct a. rewrite subst_fresh_tm; auto. fast_set_solver!!.
+Qed.
 
-Lemma let_reduction_spec_tm: forall (e_x: tm) e (v: value),
-    lc e_x ->
-    (tlete e_x e ↪* v <-> exists (v_x: value), e_x ↪* v_x /\ e ^t^ v_x ↪* v).
+Lemma value_msubst_closed: ∀ e, closed_value e -> (forall ss, value_msubst ss e = e).
 Proof.
+  unfold closed_value.
+  intros.
+  induction ss; simpl; auto.
+  destruct a. rewrite subst_fresh_value; auto. fast_set_solver!!.
+Qed.
 
+Lemma instantiation_R : ∀ c e,
+    instantiation c e →
+    ∀ x t T,
+      ctxfind c x = Some T →
+      ctxfind e x = Some t → [] ⊢t t ⋮t T.
+Proof.
+  intros c e V. induction V; simpl ; intros.
+  - inversion H.
+  - repeat var_dec_solver.
+    eapply IHV; eauto.
+Qed.
 
-(* Lemma termR_fst: forall (e e': tm), termR e e' -> (forall (v: value), e -->* v -> e' -->* v). *)
-(* Proof. intros. destruct H. auto. Qed. *)
+Lemma instantiation_R_exists : ∀ c e,
+    instantiation c e →
+    ∀ x T,
+      ctxfind c x = Some T →
+      (exists t, ctxfind e x = Some t /\ [] ⊢t t ⋮t T /\ closed_value t).
+Proof.
+  intros c e V. induction V; simpl ; intros.
+  - inversion H.
+  - repeat var_dec_solver. exists v. split; auto. split; auto; basic_typing_solver3.
+Qed.
 
-(* Global Hint Resolve termR_fst: core. *)
+Lemma msubst_var: ∀ ss (x: atom) (v: value), closed_value v -> ctxfind ss x = Some v -> value_msubst ss x = v.
+Proof.
+  induction ss; simpl; intros.
+  - inversion H0.
+  - destruct a. repeat var_dec_solver. rewrite value_msubst_closed; auto.
+Qed.
 
-(* Lemma termR_snd: forall (e e': tm), termR e e' -> (forall Gamma T, Gamma \N- e \Tin T -> Gamma \N- e' \Tin T). *)
-(* Proof. intros. destruct H. eapply H1. auto. Qed. *)
+Lemma msubst_var_none: ∀ ss (x: atom), ctxfind ss x = None -> value_msubst ss x = x.
+Proof.
+  induction ss; simpl; intros; auto.
+  - destruct a. repeat var_dec_solver.
+Qed.
 
-(* Global Hint Resolve termR_snd: core. *)
+Lemma msubst_vlam: ∀ ss Tx e, value_msubst ss (vlam Tx e) = vlam Tx (tm_msubst ss e).
+Proof.
+  induction ss; simpl; intros; auto; auto_destruct_pair.
+  eapply IHss.
+Qed.
+
+Lemma msubst_open_tm: ∀ Γv e k (x: atom),
+  ok Γv ->
+  (forall x v, ctxfind Γv x = Some v -> closed_value v /\ lc v) ->
+  x ∉ ctxdom Γv ->
+  {k ~t> x} (tm_msubst Γv e) = tm_msubst Γv ({k ~t> x} e).
+Proof.
+  induction Γv; simpl; intros; auto.
+  - auto_destruct_pair.
+    assert (closed_value v /\ lc v). eapply (H0 a v); eauto. repeat var_dec_solver.
+    rewrite subst_open_var_tm.
+    rewrite IHΓv; auto. listctx_set_solver.
+    intros. specialize (H0 x0 v0). repeat var_dec_solver. apply ctxfind_some_implies_in_dom in H3. rewrite ok_pre_destruct in H. destruct H. fast_set_solver. fast_set_solver. fast_set_solver. destruct H2; auto.
+Qed.
+
+Lemma msubst_open_value: ∀ Γv e k (x: atom),
+  ok Γv ->
+  (forall x v, ctxfind Γv x = Some v -> closed_value v /\ lc v) ->
+  x ∉ ctxdom Γv ->
+  {k ~v> x} (value_msubst Γv e) = value_msubst Γv ({k ~v> x} e).
+Proof.
+  induction Γv; simpl; intros; auto.
+  - auto_destruct_pair.
+    assert (closed_value v /\ lc v). eapply (H0 a v); eauto. repeat var_dec_solver.
+    rewrite subst_open_var_value.
+    rewrite IHΓv; auto. listctx_set_solver.
+    intros. specialize (H0 x0 v0). repeat var_dec_solver. apply ctxfind_some_implies_in_dom in H3. rewrite ok_pre_destruct in H. destruct H. fast_set_solver. fast_set_solver. fast_set_solver. destruct H2; auto.
+Qed.
+
+Ltac instantiation_regular_solver :=
+  match goal with
+  | [H: instantiation ?a ?b |- _ ∉ _ ] =>
+      apply instantiation_regular in H; repeat destruct_hyp_conj; auto; listctx_set_simpl; set_solver
+  | [H: instantiation ?a ?b |- ok _ ] =>
+      apply instantiation_regular_ok in H; repeat destruct_hyp_conj; auto; listctx_set_solver
+  | [H: instantiation ?a ?b |- forall x v, ctxfind ?b x = Some v -> _ ] =>
+      apply instantiation_regular in H; repeat destruct_hyp_conj; eauto; listctx_set_solver
+  end.
+
+Lemma msubst_vfix: ∀ ss Tx (e: value), value_msubst ss (vfix Tx e) = vfix Tx (value_msubst ss e).
+Proof.
+  induction ss; simpl; intros; auto; auto_destruct_pair.
+  eapply IHss.
+Qed.
+
+Lemma msubst_value: ∀ ss (v: value), tm_msubst ss v = tvalue (value_msubst ss v).
+Proof.
+  induction ss; simpl; intros; auto; auto_destruct_pair.
+  eapply IHss.
+Qed.
+
+Lemma msubst_tlete: ∀ ss e1 e2, tm_msubst ss (tlete e1 e2) = tlete (tm_msubst ss e1) (tm_msubst ss e2).
+Proof.
+  induction ss; simpl; intros; auto; auto_destruct_pair.
+  eapply IHss.
+Qed.
+
+Lemma msubst_tletbiop: ∀ ss op v1 v2 e,
+    tm_msubst ss (tletbiop op v1 v2 e) = tletbiop op (value_msubst ss v1) (value_msubst ss v2) (tm_msubst ss e).
+Proof.
+  induction ss; simpl; intros; auto; auto_destruct_pair.
+  eapply IHss.
+Qed.
+
+Lemma msubst_tletapp: ∀ ss v1 v2 e,
+    tm_msubst ss (tletapp v1 v2 e) = tletapp (value_msubst ss v1) (value_msubst ss v2) (tm_msubst ss e).
+Proof.
+  induction ss; simpl; intros; auto; auto_destruct_pair.
+  eapply IHss.
+Qed.
+
+Lemma msubst_tmatchb: ∀ ss v e1 e2,
+    tm_msubst ss (tmatchb v e1 e2) = tmatchb (value_msubst ss v) (tm_msubst ss e1) (tm_msubst ss e2).
+Proof.
+  induction ss; simpl; intros; auto; auto_destruct_pair.
+  eapply IHss.
+Qed.
+
+Lemma msubst_vbvar: ∀ ss k, value_msubst ss (vbvar k) = (vbvar k).
+Proof.
+  induction ss; simpl; intros; mydestr; auto.
+Qed.
+
+Lemma msubst_terr: ∀ ss, tm_msubst ss terr = terr.
+Proof.
+  induction ss; simpl; intros; auto.
+  - destruct a. auto.
+Qed.
+
+Ltac msubst_simpl :=
+  repeat match goal with
+    | [H: context [value_msubst ?env (vbvar ?k)] |- _ ] =>
+        setoid_rewrite (msubst_vbvar env k) in H
+    | [ |- context [value_msubst ?env (vbvar ?k)] ] =>
+        setoid_rewrite (msubst_vbvar env k)
+    | [H: context [value_msubst ?env (vlam ?Tx ?e)] |- _ ] =>
+        setoid_rewrite (msubst_vlam env Tx) in H
+    | [ |- context [value_msubst ?env (vlam ?Tx ?e)] ] =>
+        setoid_rewrite (msubst_vlam env Tx)
+    | [H: context [value_msubst ?env (vfix ?Tx ?e)] |- _ ] =>
+        setoid_rewrite (msubst_vfix env Tx) in H
+    | [ |- context [value_msubst ?env (vfix ?Tx ?e)] ] =>
+        setoid_rewrite (msubst_vfix env Tx)
+    | [H: context [tm_msubst ?env (tvalue ?v)] |- _ ] =>
+        setoid_rewrite (msubst_value env v) in H
+    | [ |- context [tm_msubst ?env (tvalue ?v)] ] =>
+        setoid_rewrite (msubst_value env v)
+    | [H: context [tm_msubst ?env (tlete ?e1 ?e2)] |- _ ] =>
+        setoid_rewrite (msubst_tlete env e1 e2) in H
+    | [ |- context [tm_msubst ?env (tlete ?e1 ?e2)] ] =>
+        setoid_rewrite (msubst_tlete env e1 e2)
+    | [H: context [tm_msubst ?env (tletbiop ?op ?v1 ?v2 ?e)] |- _ ] =>
+        setoid_rewrite (msubst_tletbiop env op v1 v2 e) in H
+    | [ |- context [tm_msubst ?env (tletbiop ?op ?v1 ?v2 ?e)] ] =>
+        setoid_rewrite (msubst_tletbiop env op v1 v2 e)
+    | [H: context [tm_msubst ?env (tletapp ?v1 ?v2 ?e)] |- _ ] =>
+        setoid_rewrite (msubst_tletapp env v1 v2 e) in H
+    | [ |- context [tm_msubst ?env (tletapp ?v1 ?v2 ?e)] ] =>
+        setoid_rewrite (msubst_tletapp env v1 v2 e)
+    | [H: context [tm_msubst ?env (tmatchb ?v ?e1 ?e2)] |- _ ] =>
+        setoid_rewrite (msubst_tmatchb env v e1 e2) in H
+    | [ |- context [tm_msubst ?env (tmatchb ?v ?e1 ?e2)] ] =>
+        setoid_rewrite (msubst_tmatchb env v e1 e2)
+    | [H: context [tm_msubst ?env terr] |- _ ] => rewrite (msubst_terr env) in H
+    | [ |- context [tm_msubst ?env terr] ] => rewrite (msubst_terr env)
+    end.
+
+Lemma closed_has_type_under_any_ctx_value: forall Γ (v: value) T, Γ ⊢t v ⋮v T -> closed_value v -> (forall Γ', ok Γ' -> Γ' ⊢t v ⋮v T).
+Proof.
+  intros. apply closed_has_type_under_empty_value in H; auto. basic_typing_solver2.
+Qed.
+
+Lemma closed_has_type_under_any_ctx_tm: forall Γ (v: tm) T, Γ ⊢t v ⋮t T -> closed_tm v -> (forall Γ', ok Γ' -> Γ' ⊢t v ⋮t T).
+Proof.
+  intros. apply closed_has_type_under_empty_tm in H; auto. basic_typing_solver2.
+Qed.
+
+Ltac msubst_preserves_typing_tac :=
+  match goal with
+  | [a: atom |- _ ] => repeat specialize_with a
+  end;
+  repeat match goal with
+    | [|- _ ⊢t ((tm_msubst _ _) ^t^ _) ⋮t _ ] =>
+        rewrite msubst_open_tm; try instantiation_regular_solver; try fast_set_solver
+    | [|- _ ⊢t ((value_msubst _ _) ^v^ _) ⋮v _ ] =>
+        rewrite msubst_open_value; try instantiation_regular_solver; try fast_set_solver
+    | [H: context [_ ⊢t (tm_msubst _ _) ⋮t ?T] |- _ ⊢t _ ⋮t ?T] =>
+        eapply H; eauto; try (rewrite app_assoc; auto)
+    end.
+
+Ltac msubst_preserves_typing_tac2 :=
+  (repeat match goal with
+     | [|- closed_value _] => unfold closed_value; intros; listctx_set_solver
+     | [ |- _ ⊢t mk_app _ _ ⋮t ?T ] => eapply mk_app_typable; eauto
+     | [ |- _ ⊢t (value_msubst _ _) ⋮v ?T ] => rewrite value_msubst_closed
+     | [ |- _ ⊢t (tvalue (value_msubst _ _)) ⋮t ?T ] => rewrite value_msubst_closed
+     end; basic_typing_solver2).
+
+Lemma msubst_preserves_typing_tm_aux: ∀ Γ e T,
+    Γ ⊢t e ⋮t T -> (forall Γt Γt' Γv, Γ = Γt ++ Γt' -> instantiation Γt Γv -> Γt' ⊢t (tm_msubst Γv e) ⋮t T).
+Proof.
+  apply (tm_has_type_mutual_rec
+           (fun Γ v T P => forall Γt Γt' Γv, Γ = Γt ++ Γt' -> instantiation Γt Γv -> Γt' ⊢t (value_msubst Γv v) ⋮v T)
+           (fun Γ e T P => forall Γt Γt' Γv, Γ = Γt ++ Γt' -> instantiation Γt Γv -> Γt' ⊢t (tm_msubst Γv e) ⋮t T)
+        ); simpl; intros; subst; listctx_set_simpl; repeat destruct_hyp_conj; msubst_simpl; eauto;
+  try (msubst_preserves_typing_tac2; constructor; listctx_set_solver);
+  try (auto_exists_L; simpl; intros; msubst_preserves_typing_tac).
+  - assert (forall x v, ctxfind Γv x = Some v -> closed_value v). eapply instantiation_regular_closed; eauto.
+    rewrite ctxfind_app in e; auto. destruct e.
+    + eapply instantiation_R_exists in H0; eauto. destruct H0 as (v & Hv1 & Hv2 & Hv3).
+      erewrite msubst_var; eauto. basic_typing_solver2.
+    + rewrite msubst_var_none; basic_typing_solver2.
+      apply instantiation_regular_ok in H0. mydestr. rewrite <- H0.
+      apply ctxfind_app_exclude in o. my_set_solver.
+  - (* auto_exists_L; simpl; intros. repeat specialize_with f. *)
+    msubst_preserves_typing_tac.
+    specialize (H Γt (Γt' ++ [(f, Tx ⤍ T)]) Γv).
+    rewrite msubst_vlam in H.
+    rewrite msubst_open_tm; try instantiation_regular_solver. apply H; auto.
+    rewrite app_assoc; auto.
+Qed.
+
+Lemma msubst_preserves_typing_tm: ∀ Γ Γv e T,
+    Γ ⊢t e ⋮t T -> instantiation Γ Γv -> [] ⊢t (tm_msubst Γv e) ⋮t T.
+Proof.
+  intros. eapply msubst_preserves_typing_tm_aux; eauto. listctx_set_simpl.
+Qed.
+
+Lemma msubst_preserves_typing_value_aux: ∀ Γ (e: value) T,
+    Γ ⊢t e ⋮v T -> (forall Γt Γt' Γv, Γ = Γt ++ Γt' -> instantiation Γt Γv -> Γt' ⊢t (value_msubst Γv e) ⋮v T).
+Proof.
+  apply (value_has_type_mutual_rec
+           (fun Γ v T P => forall Γt Γt' Γv, Γ = Γt ++ Γt' -> instantiation Γt Γv -> Γt' ⊢t (value_msubst Γv v) ⋮v T)
+           (fun Γ e T P => forall Γt Γt' Γv, Γ = Γt ++ Γt' -> instantiation Γt Γv -> Γt' ⊢t (tm_msubst Γv e) ⋮t T)
+        ); simpl; intros; subst; listctx_set_simpl; repeat destruct_hyp_conj; msubst_simpl; eauto;
+  try (msubst_preserves_typing_tac2; constructor; listctx_set_solver);
+  try (auto_exists_L; simpl; intros; msubst_preserves_typing_tac).
+  - assert (forall x v, ctxfind Γv x = Some v -> closed_value v). eapply instantiation_regular_closed; eauto.
+    rewrite ctxfind_app in e; auto. destruct e.
+    + eapply instantiation_R_exists in H0; eauto. destruct H0 as (v & Hv1 & Hv2 & Hv3).
+      erewrite msubst_var; eauto. basic_typing_solver2.
+    + rewrite msubst_var_none; basic_typing_solver2.
+      apply instantiation_regular_ok in H0. repeat destruct_hyp_conj. rewrite <- H0.
+      apply ctxfind_app_exclude in o. my_set_solver.
+  - (* auto_exists_L; simpl; intros. repeat specialize_with f. *)
+    msubst_preserves_typing_tac.
+    specialize (H Γt (Γt' ++ [(f, Tx ⤍ T)]) Γv).
+    rewrite msubst_vlam in H.
+    rewrite msubst_open_tm; try instantiation_regular_solver. apply H; auto.
+    rewrite app_assoc; auto.
+Qed.
+
+Lemma msubst_preserves_typing_value: ∀ Γ Γv e T,
+    Γ ⊢t e ⋮v T -> instantiation Γ Γv -> [] ⊢t (value_msubst Γv e) ⋮v T.
+Proof.
+  intros. eapply msubst_preserves_typing_value_aux; eauto. listctx_set_simpl.
+Qed.
+
+Definition termRraw Γ e e' :=
+forall env (v: value), instantiation Γ env ->
+                  (tm_msubst env e) ↪* v -> (tm_msubst env e') ↪* v.
+
+Global Hint Unfold termRraw: core.
+
+Inductive termR: listctx ty -> ty -> tm -> tm -> Prop :=
+| termR_c: forall Γ T (e e': tm),
+    Γ ⊢t e ⋮t T -> Γ ⊢t e' ⋮t T -> termRraw Γ e e' -> termR Γ T e e'.
+
+Notation " e1 '<-<{' Γ ';' T '}' e2 " := (termR Γ T e1 e2) (at level 10).
+Notation " e1 '>=<{' Γ ';' T '}' e2 " := (termR Γ T e1 e2 /\ termR Γ T e2 e1) (at level 10).
+
+Global Hint Constructors termR: core.
+
+Lemma termR_refl: forall Γ T e, Γ ⊢t e ⋮t T -> termR Γ T e e.
+Proof.
+  intros. constructor; auto.
+Qed.
+
+Lemma termR_trans: forall Γ T e1 e2 e3, Γ ⊢t e1 ⋮t T -> Γ ⊢t e2 ⋮t T -> Γ ⊢t e3 ⋮t T ->
+                                   termR Γ T e1 e2 -> termR Γ T e2 e3 -> termR Γ T e1 e3.
+Proof.
+  intros. invclear H2. invclear H3. constructor; auto.
+Qed.
+
+Lemma termRraw_emp: forall e e' T,
+    [] ⊢t e ⋮t T -> [] ⊢t e' ⋮t T ->
+    termRraw [] e e' -> (forall (v: value), e ↪* v -> e' ↪* v).
+Proof.
+  intros. unfold termRraw in H1. specialize (H1 [] v).
+  rewrite tm_msubst_closed in H1; basic_typing_solver3.
+  (* rewrite tm_msubst_closed in H1; basic_typing_solver3. *)
+  (* apply H1; eauto. constructor. *)
+Qed.
+
+Definition value_inhabitant_oracle (T: ty) : value :=
+  match T with
+  | TBool => false
+  | TNat => 0
+  | T1 ⤍ T2 => vlam T1 terr
+  end.
+
+Lemma value_inhabitant_oracle_spec: forall Γ T, ok Γ -> Γ ⊢t value_inhabitant_oracle T ⋮v T.
+Proof.
+  intros. destruct T.
+  - destruct b; constructor; auto.
+  - auto_exists_L.
+Qed.
+
+Lemma value_inhabitant_oracle_spec_empty: forall T, [] ⊢t value_inhabitant_oracle T ⋮v T.
+Proof.
+  intros. apply value_inhabitant_oracle_spec; auto.
+Qed.
+
+Global Hint Resolve value_inhabitant_oracle_spec_empty: core.
+
+Lemma instantiation_msubst_perserve_ty: forall Γ env e T,
+    instantiation Γ env -> Γ ⊢t e ⋮t T -> [] ⊢t (tm_msubst env e) ⋮t T.
+Proof.
+  induction Γ; intros; invclear H; auto.
+  simpl. apply IHΓ; auto. basic_typing_solver3.
+Qed.
+
+Lemma termR_tlete_dummy: forall Γ Tx T (e_x e: tm), Γ ⊢t e_x ⋮t Tx -> Γ ⊢t e ⋮t T -> (tlete e_x e) <-<{Γ;T} e.
+Proof.
+  intros. constructor; auto.
+  - basic_typing_solver.
+  - unfold termRraw. intros. msubst_simpl.
+    rewrite lete_step_spec in H2; mydestr.
+    eapply instantiation_msubst_perserve_ty in H1; eauto.
+    lc_simpl.
+Qed.
+
+Ltac mk_app_perserve_termR_tac :=
+  match goal with
+  | [H: ?e ↪* (tvalue ?v),
+        H': ∀ v1 : value, ?e ↪* (tvalue v1) → ?e' ↪* (tvalue v1) |-
+                            exists v_x: value, ?e' ↪* (tvalue v_x) /\ _ ] => exists v; split; auto
+  end.
+
+Ltac termR_solver1 :=
+  intros; auto;
+  repeat match goal with
+    | [H: ?e <-<{_;_} ?e' |- ?Γ ⊢t ?e' ⋮t _ ] => invclear H; mydestr; eauto
+    | [H: ?e <-<{_;_} ?e' |- ?Γ ⊢t ?e ⋮t _ ] => invclear H; mydestr; eauto
+    | [H: ?e <-<{_;_} ?e' |- ?e' ↪* _ ] => invclear H; mydestr; eauto
+    | [ |- ?e <-<{_;_} ?e] => constructor; eauto
+    | [H: termRraw [] ?e ?e' |- ?e' ↪* _ ] =>
+        apply termRraw_emp in H; try basic_typing_solver3; eauto
+    end.
+
+Lemma instantiation_implies_open_msubst:
+      ∀ Γ Γv, instantiation Γ Γv -> forall e T Tu k (u: value),
+          Γ ⊢t e ⋮t T -> [] ⊢t u ⋮v Tu ->
+                {k ~t> u} (tm_msubst Γv e) = tm_msubst Γv ({k ~t> u} e).
+Proof.
+  intros Γ Γv Hi. induction Hi; simpl; intros; auto.
+  rewrite IHHi with (T:=T0) (Tu:=Tu); eauto.
+  - rewrite -> subst_open_tm; basic_typing_solver3.
+    rewrite subst_fresh_value; basic_typing_solver3.
+  - basic_typing_solver3.
+Qed.
+
+Lemma instantiation_implies_close_msubst:
+  ∀ Γ Γv, instantiation Γ Γv ->
+                    forall e k (x: atom), x ∉ ctxdom Γ -> {k <t~ x} (tm_msubst Γv e) = tm_msubst Γv ({k <t~ x} e).
+Proof.
+  intros Γ Γv Hi. induction Hi; simpl; intros; auto.
+  rewrite IHHi; try fast_set_solver.
+  - rewrite -> subst_close_tm; basic_typing_solver3.
+Qed.
+
+Lemma instantiation_implies_msubst_lc:
+      ∀ Γ Γv, instantiation Γ Γv -> forall e, lc e -> lc (tm_msubst Γv e).
+Proof.
+  intros Γ Γv Hi. induction Hi; simpl; intros; auto.
+  - apply IHHi. apply subst_lc_tm; basic_typing_solver3.
+Qed.
+
+Lemma mk_app_perserve_termR: forall Γ Tx T(e1 e2 e1' e2': tm),
+    e1 <-<{Γ;Tx ⤍ T} e1' -> e2 <-<{Γ;Tx} e2' -> (mk_app e1 e2) <-<{Γ;T} (mk_app e1' e2').
+Proof.
+  intros.
+  constructor; auto.
+  - eapply mk_app_typable; termR_solver1.
+  - eapply mk_app_typable; termR_solver1.
+  - intros. invclear H. invclear H0. unfold mk_app; intros; mydestr.
+    unfold termRraw; intros. msubst_simpl.
+    rewrite lete_step_spec in H6; simpl; mydestr. rewrite lete_step_spec; simpl.
+    split.
+    + unfold body in H0; mydestr. auto_exists_L; intros. lc_simpl.
+      simpl in H8.
+      assert (lc e2') as He2' by basic_typing_solver3.
+      eapply instantiation_implies_msubst_lc in He2'; eauto.
+      rewrite open_rec_lc_tm; basic_typing_solver3.
+    + apply H3 in H7; auto. exists x. split; auto. lc_simpl.
+      assert ([] ⊢t x ⋮v Tx ⤍ T).
+      { eapply instantiation_msubst_perserve_ty in H2; eauto.
+        basic_typing_solver3. }
+      simpl in H8.
+      erewrite instantiation_implies_open_msubst; eauto.
+      erewrite instantiation_implies_open_msubst in H8; eauto.
+      lc_simpl.
+      rewrite lete_step_spec in H8; simpl; mydestr.
+      rewrite lete_step_spec; simpl. split; auto.
+      eexists; split; eauto.
+Qed.
+
+Lemma tyable_implies_terr_termR: forall (e: tm) Γ T, Γ ⊢t e ⋮t T -> terr <-<{ Γ; T} e.
+Proof.
+  intros. repeat split; auto.
+  - constructor; basic_typing_solver2.
+  - econstructor; eauto. msubst_simpl. auto_reduction_exfalso.
+Qed.
+
+Lemma tyable_implies_terr_termR_terr: forall (e: tm) Γ T1 T, Γ ⊢t e ⋮t T1 -> tlete e terr <-<{ Γ; T} terr.
+Proof.
+  intros. repeat split; auto.
+  - auto_exists_L. intros. simpl. constructor. basic_typing_solver.
+  - econstructor; basic_typing_solver.
+  - econstructor; eauto. msubst_simpl. auto_reduction_exfalso.
+Qed.
+
+Lemma msubst_subst_commute_tm: forall Γ Γv,
+    instantiation Γ Γv ->
+    forall x u e, x ∉ ctxdom Γv -> closed_value u ->
+             {x := u }t tm_msubst Γv e = tm_msubst Γv ({x := u }t e).
+Proof.
+  intros Γv Γ Hi; induction Hi; simpl; intros; mydestr; auto.
+  rewrite IHHi; try fast_set_solver.
+  rewrite subst_commute_tm; auto; basic_typing_solver3; set_solver.
+Qed.
+
+Lemma msubst_subst_commute_value: forall Γ Γv,
+    instantiation Γ Γv ->
+    forall x u e, x ∉ ctxdom Γv -> closed_value u ->
+             {x := u }v value_msubst Γv e = value_msubst Γv ({x := u }v e).
+Proof.
+  intros Γv Γ Hi; induction Hi; simpl; intros; mydestr; auto.
+  rewrite IHHi; try fast_set_solver.
+  rewrite subst_commute_value; auto; basic_typing_solver3; set_solver.
+Qed.
+
+Lemma tm_msubst_mid_subst: forall Γv1 x u Γv2 Γ,
+    instantiation Γ (Γv1 ++ (x, u) :: Γv2) -> closed_value u ->
+    ∀ e, tm_msubst (Γv1 ++ (x, u) :: Γv2) e = tm_msubst (Γv1 ++ Γv2) ({x:= u}t e).
+Proof.
+  induction Γv1; simpl; intros; mydestr; auto.
+  invclear H.
+  erewrite IHΓv1; eauto. apply instantiation_regular in H7; mydestr. listctx_set_simpl.
+  rewrite subst_commute_tm; auto; basic_typing_solver3; set_solver.
+Qed.
+
+Lemma value_msubst_mid_subst: forall Γv1 x u Γv2 Γ,
+    instantiation Γ (Γv1 ++ (x, u) :: Γv2) -> closed_value u ->
+    ∀ e, value_msubst (Γv1 ++ (x, u) :: Γv2) e = value_msubst (Γv1 ++ Γv2) ({x:= u}v e).
+Proof.
+  induction Γv1; simpl; intros; mydestr; auto.
+  invclear H.
+  erewrite IHΓv1; eauto. apply instantiation_regular in H7; mydestr. listctx_set_simpl.
+  rewrite subst_commute_value; auto; basic_typing_solver3; set_solver.
+Qed.
+
+Lemma instantiation_app_spec: forall Γv1 Γv2 Γ,
+    instantiation Γ (Γv1 ++ Γv2) <->
+      ∃ Γ1 Γ2, Γ = Γ1 ++ Γ2 /\ ok Γ /\ instantiation Γ1 Γv1 /\ instantiation Γ2 Γv2 .
+Proof.
+  induction Γv1; split; simpl; intros.
+  - exists [], Γ. repeat split; simpl; auto; instantiation_regular_solver.
+  - mydestr; subst. invclear H1. auto.
+  - invclear H. apply IHΓv1 in H5; mydestr.
+    exists ((x, T) :: x0), x1. subst. repeat split; auto.
+    + rewrite ok_pre_destruct; split; auto.
+    + constructor; listctx_set_solver.
+  - mydestr; subst. invclear H1. listctx_set_simpl.
+    constructor; auto; listctx_set_simpl.
+    rewrite IHΓv1. exists c, x0. repeat split; auto.
+Qed.
+
+Ltac instantiation_regular_simp :=
+  repeat match goal with
+    | [H: instantiation _ _ |- _ ∉ _ ] => apply instantiation_regular in H; mydestr
+    end.
+
+Lemma instantiation_app_spec': forall Γ1 Γ2 Γv,
+    instantiation (Γ1 ++ Γ2) Γv <->
+      ∃ Γv1 Γv2, Γv = Γv1 ++ Γv2 /\ ok Γv /\ instantiation Γ1 Γv1 /\ instantiation Γ2 Γv2 .
+Proof.
+  induction Γ1; split; simpl; intros.
+  - exists [], Γv. repeat split; simpl; auto; instantiation_regular_solver.
+  - mydestr; subst. invclear H1. auto.
+  - invclear H. apply IHΓ1 in H5; mydestr.
+    exists ((x, v) :: x0), x1. subst. repeat split; auto.
+    + rewrite ok_pre_destruct; split; auto.
+      instantiation_regular_simp. listctx_set_simpl. set_solver.
+    + constructor; listctx_set_solver.
+  - mydestr; subst. invclear H1. listctx_set_simpl.
+    constructor; auto; listctx_set_simpl. instantiation_regular_simp. set_solver.
+    rewrite IHΓ1. exists e, x0. repeat split; auto.
+Qed.
+
+Lemma tm_msubst_swap_hd_tl: forall Γv Γ Γv',
+    instantiation Γ (Γv ++ Γv') -> ∀ e, tm_msubst (Γv ++ Γv') e = tm_msubst (Γv' ++ Γv) e.
+Proof.
+  induction Γv; intros.
+  - listctx_set_simpl.
+  - invclear H. rewrite instantiation_app_spec in H5; mydestr; subst.
+    listctx_set_simpl. simpl.
+    rewrite IHΓv with (Γ := (x0 ++ x1)); auto.
+    rewrite tm_msubst_mid_subst with (Γ := (x1 ++ (x, T) :: x0)); eauto.
+    + rewrite instantiation_app_spec. exists x1, ((x, T) :: x0). repeat split; auto.
+      apply ok_mid_insert; split; listctx_set_solver5.
+      constructor; auto; listctx_set_solver5.
+    + basic_typing_solver3.
+    + rewrite instantiation_app_spec. exists x0, x1. split; auto.
+Qed.
+
+Lemma msubst_preserves_body_tm: forall Γ Γv e,
+    instantiation Γ Γv -> body e -> body (tm_msubst Γv e).
+Proof.
+  intros. induction H; simpl; auto.
+  erewrite <- msubst_subst_commute_tm; eauto.
+  apply subst_body_tm; auto; basic_typing_solver3.
+  - instantiation_regular_solver.
+  - basic_typing_solver3.
+Qed.
+
+Lemma termRraw_swap: forall e e' Γ1 Γ2, termRraw (Γ1 ++ Γ2) e e' -> termRraw (Γ2 ++ Γ1) e e'.
+Proof.
+  unfold termRraw. intros.
+  apply instantiation_app_spec' in H0; mydestr; subst.
+  assert (instantiation (Γ2 ++ Γ1) (x ++ x0)).
+  { apply instantiation_app_spec'. exists x, x0. repeat split; auto. }
+  erewrite tm_msubst_swap_hd_tl; eauto.
+  erewrite tm_msubst_swap_hd_tl in H1; eauto.
+  apply H; auto.
+  rewrite instantiation_app_spec'. exists x0, x. repeat split; auto.
+  listctx_set_solver5.
+Qed.
+
+Lemma termR_swap: forall e e' Γ1 Γ2 T, e <-<{ Γ1 ++ Γ2; T} e' <-> e <-<{ Γ2 ++ Γ1; T} e'.
+Proof.
+  split; intros; invclear H; constructor; auto; basic_typing_solver4; apply termRraw_swap; auto.
+Qed.
+
+Lemma termR_elete: forall γ Tx T e_x e_x' e e' (x: atom),
+    e_x <-<{γ; Tx} e_x' -> e <-<{γ ++ [(x, Tx)]; T} e' ->
+    (tlete e_x (x \t\ e)) <-<{γ; T} (tlete e_x' (x \t\ e')).
+Proof.
+    intros.
+    assert (ok (γ ++ [(x, Tx)])) as HH. invclear H0. basic_typing_solver.
+    invclear H. invclear H0. repeat split; auto.
+  - auto_exists_L; intros. rewrite subst_as_close_open_tm; try basic_typing_solver.
+    apply basic_has_type_renaming; eauto;  basic_typing_solver3.
+  - auto_exists_L; intros. rewrite subst_as_close_open_tm; try basic_typing_solver.
+    apply basic_has_type_renaming; eauto;  basic_typing_solver3.
+  - unfold termRraw. intros Γv u Hi. intros. msubst_simpl.
+    rewrite lete_step_spec in H0; simpl; mydestr.
+    rewrite lete_step_spec; simpl.
+    split.
+    { eapply msubst_preserves_body_tm; eauto.
+      auto_exists_L; intros. rewrite subst_as_close_open_tm; try basic_typing_solver3.
+      apply subst_lc_tm; auto. }
+    exists x0. split; auto.
+    setoid_rewrite <- instantiation_implies_close_msubst in H7; eauto; basic_typing_solver3.
+    setoid_rewrite <- instantiation_implies_close_msubst; eauto; basic_typing_solver3.
+    setoid_rewrite subst_as_close_open_tm in H7; basic_typing_solver3.
+    setoid_rewrite subst_as_close_open_tm; basic_typing_solver3.
+    + specialize (H5 (Γv ++ [(x, x0)]) u).
+      assert ([] ⊢t (tm_msubst Γv e_x ) ⋮t Tx) by (eapply msubst_preserves_typing_tm; eauto).
+      assert ([] ⊢t x0 ⋮v Tx) by basic_typing_solver3.
+      assert (instantiation (γ ++ [(x, Tx)]) (Γv ++ [(x, x0)])).
+      { rewrite instantiation_app_spec. exists γ, [(x, Tx)]; repeat split; auto.
+        repeat constructor; auto; try fast_set_solver. }
+      rewrite tm_msubst_swap_hd_tl with (Γ := (γ ++ [(x, Tx)])) in H5; auto; simpl in H5.
+      rewrite tm_msubst_swap_hd_tl with (Γ := (γ ++ [(x, Tx)])) in H5; auto; simpl in H5.
+      rewrite <- msubst_subst_commute_tm with (Γ := γ) in H5; auto; basic_typing_solver3; try instantiation_regular_solver.
+      rewrite <- msubst_subst_commute_tm with (Γ := γ) in H5; auto; basic_typing_solver3; try instantiation_regular_solver.
+    + eapply instantiation_implies_msubst_lc; eauto.
+    + eapply instantiation_implies_msubst_lc; eauto.
+Qed.
+
+Ltac termR_solver :=
+  repeat (match goal with
+          | [H: termRraw [] ?e ?e' |- ?e' ↪* _ ] =>
+              assert ((forall (v: value), e ↪* v -> e' ↪* v)); auto;
+              eapply termRraw_emp; eauto; try basic_typing_solver3
+          | [|- (mk_app _ _) <-<{ _; _} (mk_app _ _)] => eapply mk_app_perserve_termR; eauto
+          | [H: ?e <-<{ ?a ++ ?b; ?T} ?e' |- ?e <-<{ ?b ++ ?a; ?T} ?e'] => rewrite termR_swap; eauto
+          | [H: ?e <-<{ (?x, ?t) :: ?b; ?T} ?e' |- ?e <-<{ ?b ++ [(?x, ?t)]; ?T} ?e'] => rewrite termR_swap; eauto
+          end || termR_solver1).
