new_proof/AuxTyping.v
@@ -1,0 +1,208 @@
+From stdpp Require Import mapset.
+From stdpp Require Import natmap.
+From CT Require Import CoreLangProp.
+From CT Require Import OperationalSemanticsProp.
+From CT Require Import BasicTypingProp.
+From CT Require Import SyntaxSugar.
+From CT Require Import Refinement.
+From CT Require Import RefinementDenotation.
+
+Import Atom.
+Import CoreLang.
+Import Tactics.
+Import NamelessTactics.
+Import ListCtx.
+Import OperationalSemantics.
+Import OperationalSemanticsProp.
+Import BasicTyping.
+Import SyntaxSugar.
+Import Refinement.
+Import RefinementDenotation.
+
+(* Well Formedness *)
+
+Inductive wf_ctx: listctx rty -> Prop :=
+| wf_ctx_nil: wf_ctx []
+| wf_ctx_cons_ubase: forall Γ x b n d ϕ,
+    wf_ctx Γ ->
+    x ∉ ctxdom Γ ->
+    ~ (⟦ [v: b | n | d | ϕ ] ⟧{ Γ } terr) ->
+    wf_ctx (Γ ++ [(x, [v: b | n | d | ϕ ])])
+| wf_ctx_cons: forall Γ x τ,
+    wf_ctx Γ ->
+    x ∉ ctxdom Γ ->
+    not_underbasety τ ->
+    wf_ctx (Γ ++ [(x, τ)]).
+
+Lemma err_exists_denotation_excluded: forall Γ b n d ϕ,
+    (∃ e, ⟦ [v: b | n | d | ϕ ] ⟧{ Γ } e) <-> ~ (⟦ [v: b | n | d | ϕ ] ⟧{ Γ } terr).
+Admitted.
+
+Lemma wf_ctx_implies_ok: forall Γ, wf_ctx Γ -> ok Γ.
+Admitted.
+
+Lemma wf_ctx_implies_valid: forall Γ x τ,  wf_ctx Γ -> ctxfind Γ x = Some τ -> valid_rty τ.
+Admitted.
+
+Lemma wf_ctx_implies_lc_rty: forall Γ x τ,  wf_ctx Γ -> ctxfind Γ x = Some τ -> lc_rty τ.
+Admitted.
+
+Lemma wf_ctx_regular:
+  ∀ Γ, wf_ctx Γ -> ok Γ /\ (forall x τ, ctxfind Γ x = Some τ -> valid_rty τ) /\ (forall x τ, ctxfind Γ x = Some τ -> lc_rty τ).
+Admitted.
+
+Lemma wf_ctx_implies_mid_closed: forall Γ1 x τ Γ2, wf_ctx (Γ1 ++ [(x, τ)] ++ Γ2) -> (rty_fv τ) ⊆ (ctxdom Γ1).
+Admitted.
+
+Lemma wf_ctx_implies_inhabitant_exists: forall Γ1 x τ Γ2, wf_ctx (Γ1 ++ [(x, τ)] ++ Γ2) -> (exists e, ⟦ τ ⟧{ Γ1 } e).
+Admitted.
+
+Definition wf (Γ: listctx rty) (τ: rty) := wf_ctx Γ /\ closed_rty 0 (ctxdom Γ) τ.
+
+Notation " Γ '⊢WF' τ " := (wf Γ τ) (at level 20, τ constr, Γ constr).
+
+(* Disjunction *)
+
+Definition disjunction (Γ: listctx rty) (τ1 τ2 τ3: rty) := forall e, (⟦ τ1 ⟧{ Γ } e) /\ (⟦ τ2 ⟧{ Γ } e) <-> (⟦ τ3 ⟧{ Γ } e).
+
+Notation " Γ '⊢' τ1 '⩔' τ2 '⩵' τ3 " := (disjunction Γ τ1 τ2 τ3) (at level 20, τ1 constr, τ2 constr, τ3 constr, Γ constr).
+
+(* Subtyping *)
+
+Inductive subtyping: listctx rty -> rty -> rty -> Prop :=
+| subtyping_ubase: forall Γ b n d ϕ1 ϕ2,
+    ⟦ [v: b | n | d | ϕ1 ] ⟧⊆⟦ [v: b | n | d | ϕ2 ] ⟧{ Γ } ->
+    subtyping Γ [v: b | n | d | ϕ1 ] [v: b | n | d | ϕ2 ]
+| subtyping_obase: forall Γ b n d ϕ1 ϕ2,
+    ⟦ [v: b | n | d | ϕ2 ] ⟧⊆⟦ [v: b | n | d | ϕ1 ] ⟧{ Γ } ->
+    subtyping Γ {v: b | n | d | ϕ1 } {v: b | n | d | ϕ2 }
+| subtyping_oarr: forall Γ b n d ϕ1 ϕ2 τ1 τ2 (L: aset),
+    subtyping Γ {v: b | n | d | ϕ2 } {v: b | n | d | ϕ1 } ->
+    (forall x, x ∉ L -> subtyping (Γ ++ [(x, {v: b | n | d | ϕ2 })]) τ1 τ2) ->
+    ⟦ [v: b | n | d | ϕ2 ] ⟧⊆⟦ [v: b | n | d | ϕ1 ] ⟧{ Γ } ->
+    subtyping Γ (-:{v: b | n | d | ϕ1 }⤑ τ1) (-:{v: b | n | d | ϕ2 }⤑ τ2).
+
+Notation " Γ '⊢' τ1 '⪡' τ2 " := (subtyping Γ τ1 τ2) (at level 20, τ1 constr, τ2 constr, Γ constr).
+
+Definition subtyping_spec: forall Γ τ1 τ2, Γ ⊢WF τ2 -> Γ ⊢ τ1 ⪡ τ2 -> (forall e, ⟦ τ1 ⟧{ Γ } e -> ⟦ τ2 ⟧{ Γ } e).
+Admitted.
+
+Reserved Notation "Γ '⊢' τ '⋮t' T" (at level 20).
+Reserved Notation "Γ '⊢' τ '⋮v' T"  (at level 20).
+
+Inductive term_under_type_check : listctx rty -> tm -> rty -> Prop :=
+| UT_Value: forall Γ v τ, Γ ⊢ v ⋮v τ -> Γ ⊢ v ⋮t τ
+| UT_terr: forall Γ b, Γ ⊢WF (mk_under_bot b) -> Γ ⊢ terr ⋮t (mk_under_bot b)
+| UT_Sub: forall Γ e (τ1 τ2:rty), Γ ⊢WF τ2 -> [] ⊢ e ⋮t τ1 -> [] ⊢ τ1 ⪡ τ2 ->  (Γ ⊢ e ⋮t τ2)
+| UT_Eq: forall Γ e τ1 τ2, Γ ⊢WF τ2 -> Γ ⊢ e ⋮t τ1 -> Γ ⊢ τ1 ⪡ τ2 -> Γ ⊢ τ2 ⪡ τ1 -> Γ ⊢ e ⋮t τ2
+| UT_Merge: forall Γ e (τ1 τ2 τ3: rty), Γ ⊢WF τ3 -> Γ ⊢ e ⋮t τ1 -> Γ ⊢ e ⋮t τ2 -> Γ ⊢ τ1 ⩔ τ2 ⩵ τ3 -> Γ ⊢ e ⋮t τ3
+| UT_Lete: forall Γ e_x e τ τ_x (L: aset),
+    Γ ⊢WF τ -> Γ ⊢ e_x ⋮t τ_x -> (forall x, x ∉ L -> (Γ ++ [(x, τ_x)]) ⊢ (e ^t^ x) ⋮t τ ) -> Γ ⊢ (tlete e_x e) ⋮t τ
+(* operators only take nat type *)
+| UT_LetOp: forall (Γ: listctx rty) op (v1 v2: value) e τ d1 d2 ϕ1 ϕ2 (L: aset),
+    Γ ⊢WF τ ->
+    Γ ⊢ v1 ⋮v [v: fst_ty_of_op op | 0 | d1 | ϕ1 ] ->
+    Γ ⊢ v2 ⋮v [v: snd_ty_of_op op | 0 | d2 | ϕ2 ] ->
+    (forall x, x ∉ L -> (Γ ++ [(x, ((mk_op_ret op) ^r^ v1) ^r^ v2)]) ⊢ e ⋮t τ) ->
+    Γ ⊢ (tletbiop op v1 v2 e) ⋮t τ
+| UT_LetAppIndepend: forall Γ (v1 v2: value) e τ τ2 τ_x (L: aset),
+    Γ ⊢WF τ -> Γ ⊢ v1 ⋮v (τ2 ⤑ τ_x) -> Γ ⊢ v2 ⋮v τ2 -> (forall x, x ∉ L -> (Γ ++ [(x, τ_x)]) ⊢ (e ^t^ x) ⋮t τ) ->
+    Γ ⊢ (tletapp v1 v2 e) ⋮t τ
+(* the value should only be constant or variables *)
+| UT_LetAppDepend: forall Γ (v1 v2: value) e τ b d ϕ τ_x (L: aset),
+    Γ ⊢WF τ -> Γ ⊢ v1 ⋮v (-:{v: b | 0 | d | ϕ}⤑ τ_x) -> Γ ⊢ v2 ⋮v [v: b | 0 | d | ϕ] ->
+    (forall x, x ∉ L -> (Γ ++ [(x, τ_x ^r^ v2)]) ⊢ (e ^t^ x) ⋮t τ ) ->
+    Γ ⊢ (tletapp v1 v2 e) ⋮t τ
+| UT_Matchb_true: forall Γ (v: value) e1 e2 τ,
+    Γ ⊢WF τ -> Γ ⊢ v ⋮v (mk_eq_constant true) -> Γ ⊢ e1 ⋮t τ -> ⌊ Γ ⌋* ⊢t e2 ⋮t ⌊ τ ⌋ -> Γ ⊢ (tmatchb v e1 e2) ⋮t τ
+| UT_Matchb_false: forall Γ (v: value) e1 e2 τ,
+    Γ ⊢WF τ -> Γ ⊢ v ⋮v (mk_eq_constant false) -> Γ ⊢ e2 ⋮t τ -> ⌊ Γ ⌋* ⊢t e1 ⋮t ⌊ τ ⌋ -> Γ ⊢ (tmatchb v e1 e2) ⋮t τ
+with value_under_type_check : listctx rty -> tm -> rty -> Prop :=
+| UT_Contant: forall Γ (c: constant), Γ ⊢WF (mk_eq_constant c) -> Γ ⊢ c ⋮v (mk_eq_constant c)
+| UT_VarOver: forall Γ b (x: atom),
+    Γ ⊢WF (mk_eq_var b x) -> (exists n d ϕ, ctxfind Γ x = Some {v: b | n | d | ϕ}) -> Γ ⊢ x ⋮v (mk_eq_var b x)
+| UT_VarBase: forall Γ b (x: atom),
+    Γ ⊢WF (mk_eq_var b x) -> (exists n d ϕ, ctxfind Γ x = Some [v: b | n | d | ϕ]) -> Γ ⊢ x ⋮v (mk_eq_var b x)
+| UT_VarArr: forall Γ x τ_x, Γ ⊢WF τ_x -> is_arr τ_x -> ctxfind Γ x = Some τ_x -> Γ ⊢ x ⋮v τ_x
+| UT_LamDep: forall Γ b d ϕ e τ (L: aset),
+    Γ ⊢WF (-:{v: b | 0 | d | ϕ}⤑ τ) -> (forall x, x ∉ L -> (Γ ++ [(x, {v: b | 0 | d | ϕ})]) ⊢ (e ^t^ x) ⋮t (τ ^r^ x)) ->
+    Γ ⊢ (vlam b e) ⋮v (-:{v: b | 0 | d | ϕ}⤑ τ)
+| UT_LamIndep: forall Γ τ1 τ2 e τ (L: aset),
+    Γ ⊢WF ((τ1 ⤑ τ2) ⤑ τ) -> (forall x, x ∉ L -> (Γ ++ [(x, (τ1 ⤑ τ2))]) ⊢ (e ^t^ x) ⋮t τ) ->
+    Γ ⊢ (vlam ⌊ τ1 ⤑ τ2 ⌋ e) ⋮v ((τ1 ⤑ τ2) ⤑ τ)
+| UT_LamFix: forall Γ b d ϕ e τ,
+    Γ ⊢WF (-:{v: b | 0 | d | ϕ}⤑ τ) ->
+    Γ ⊢ (vlam b (vlam (b ⤍ ⌊ τ ⌋) e)) ⋮v (-:{v: b | 0 | d | ϕ}⤑ (-:{v: b | 1 | d | ≻≻ ϕ}⤑ τ) ⤑ τ) ->
+    Γ ⊢ (vfix (b ⤍ ⌊ τ ⌋) (vlam b e)) ⋮v (-:{v: b | 0 | d | ϕ}⤑ τ)
+where
+"Γ '⊢' τ '⋮t' T" := (term_under_type_check Γ τ T) and "Γ '⊢' τ '⋮v' T" := (value_under_type_check Γ τ T).
+
+Scheme value_under_type_check_rec := Induction for value_under_type_check Sort Prop
+    with term_under_type_check_rec := Induction for term_under_type_check Sort Prop.
+
+Lemma rRctx_pre_weakening: forall Γ1 Γ2 τ, (Γ1 ++ Γ2) ⊢WF τ -> (forall e, ⟦τ⟧{Γ1} e -> ⟦τ⟧{Γ1 ++ Γ2} e).
+Admitted.
+
+Lemma rRctx_weakening_empty: forall Γ τ, Γ ⊢WF τ -> (forall e, ⟦τ⟧ e -> ⟦τ⟧{Γ} e).
+Admitted.
+
+Lemma rRctx_backward_over: forall Γ z b n d ϕ (e: tm) τ,
+    ⟦ τ ⟧{ Γ ++ [(z, {v: b | n | d | ϕ})] } e <->
+    (forall (u: value), ⟦ {v: b | n | d | ϕ} ⟧{ Γ } u -> ⟦ { z := u }r τ ⟧{ Γ } ({ z := u }t e)).
+Admitted.
+
+Lemma rRctx_backward_under: forall Γ z τ_z (e: tm) τ,
+    ~ not_overbasety τ_z ->
+    ⟦ τ ⟧{ Γ ++ [(z, τ_z)] } e <->
+      (∃ (u_hat: tm), ⟦ τ_z ⟧{ Γ } u_hat /\
+                        (forall (u: tm), ⟦ τ_z ⟧{ Γ } u ->
+                                    (∀ (v_u: value), u_hat ↪* v_u -> ⟦ { z:= v_u }r τ ⟧{ Γ } (tlete u (e ^t^ z)))
+                        )).
+Admitted.
+
+Theorem soundness: forall (Γ: listctx rty) (e: tm) (τ: rty), Γ ⊢ e ⋮t τ -> ⟦ τ ⟧{ Γ } e.
+Proof.
+  apply (term_under_type_check_rec
+           (fun Γ v τ _ => ⟦ τ ⟧{ Γ } v)
+           (fun Γ e τ _ => ⟦ τ ⟧{ Γ } e)); intros Γ; intros; mydestr.
+  (* constant *)
+  - apply rRctx_weakening_empty; auto. admit.
+  (* var base *)
+  - apply ctxfind_some_spec in H; auto; mydestr; subst.
+    rewrite app_assoc. apply rRctx_pre_weakening; auto. admit. rewrite rRctx_backward_over.
+    intros. apply rRctx_weakening_empty. admit. admit. admit.
+  - apply ctxfind_some_spec in H; auto; mydestr; subst.
+    rewrite app_assoc. apply rRctx_pre_weakening; auto. admit. rewrite rRctx_backward_under. admit. admit. admit.
+  (* var arr *)
+  - apply ctxfind_some_spec in e; auto; mydestr; subst.
+    rewrite app_assoc. apply rRctx_pre_weakening; auto. admit. rewrite rRctx_backward_under. admit. admit. admit.
+  (* lam *)
+  - auto_pose_fv x. repeat specialize_with x. admit.
+  - auto_pose_fv x. repeat specialize_with x. admit.
+  (* fix *)
+  - admit.
+  (* value *)
+  - auto.
+  (* err *)
+  - admit.
+  (* sub *)
+  - repeat match goal with
+    | [H: ⟦ ?τ ⟧{ [] } ?e |- ⟦ ?τ ⟧{ ?Γ } ?e ] => invclear H; apply rRctx_weakening_empty; auto
+    | [H: _ ⊢ _ ⪡ _ |- _ ?e ] => apply subtyping_spec with (e := e) in H
+    end. admit. admit.
+  (* eq *)
+  - eapply subtyping_spec; eauto.
+  (* merge *)
+  - match goal with
+    | [H: _ ⊢ _ ⩔ _ ⩵ _ |- _ ] => unfold disjunction in H; erewrite <- H; split; auto
+    end.
+  (* lete *)
+  - auto_pose_fv x. repeat specialize_with x. admit.
+  (* letop *)
+  - auto_pose_fv x. repeat specialize_with x. admit.
+  - auto_pose_fv x. repeat specialize_with x. admit.
+  - auto_pose_fv x. repeat specialize_with x. admit.
+  (* matchb true *)
+  - admit.
+  - admit.
+Admitted.
