new_proof/BasicTypingProp.v
@@ -30,7 +30,7 @@ Proof.
                 (Γ = Γ1 ++ Γ3) -> ok (Γ1 ++ Γ2 ++ Γ3) → (Γ1 ++ Γ2 ++ Γ3) ⊢t v ⋮v T)
            (fun Γ e T P => ∀ (Γ1 Γ2 Γ3 : list (atom * ty)),
                 (Γ = Γ1 ++ Γ3) -> ok (Γ1 ++ Γ2 ++ Γ3) → (Γ1 ++ Γ2 ++ Γ3) ⊢t e ⋮t T)
-        ); simpl; intros; subst; econstructor; auto;
+        ); simpl; intros; subst; econstructor; eauto;
     try (instantiate_atom_listctx; auto_apply; listctx_set_solver);
     try listctx_set_solver.
 Qed.
@@ -44,7 +44,7 @@ Proof.
                 (Γ = Γ1 ++ Γ3) -> ok (Γ1 ++ Γ2 ++ Γ3) → (Γ1 ++ Γ2 ++ Γ3) ⊢t v ⋮v T)
            (fun Γ e T P => ∀ (Γ1 Γ2 Γ3 : list (atom * ty)),
                 (Γ = Γ1 ++ Γ3) -> ok (Γ1 ++ Γ2 ++ Γ3) → (Γ1 ++ Γ2 ++ Γ3) ⊢t e ⋮t T)
-        ); simpl; intros; subst; econstructor; auto;
+        ); simpl; intros; subst; econstructor; eauto;
     try (instantiate_atom_listctx; auto_apply; listctx_set_solver);
     try listctx_set_solver.
 Qed.
@@ -193,6 +193,22 @@ Proof.
   eapply basic_typing_subst_tm; eauto.
 Qed.
 
+Lemma basic_typing_subst_value_post: forall Γ1 z u U (v: value) T,
+    ((z, U) :: Γ1) ⊢t v ⋮v T -> [] ⊢t u ⋮v U -> Γ1 ⊢t {z := u}v v ⋮v T.
+Proof.
+  intros.
+  assert (([] ++ [(z, U)] ++ Γ1) ⊢t v ⋮v T) by listctx_set_simpl.
+  apply (basic_typing_subst_value [] z u) in H1; listctx_set_simpl.
+Qed.
+
+Lemma basic_typing_subst_tm_post: forall Γ1 z u U (v: tm) T,
+    ((z, U) :: Γ1) ⊢t v ⋮t T -> [] ⊢t u ⋮v U -> Γ1 ⊢t {z := u}t v ⋮t T.
+Proof.
+  intros.
+  assert (([] ++ [(z, U)] ++ Γ1) ⊢t v ⋮t T) by listctx_set_simpl.
+  apply (basic_typing_subst_tm [] z u) in H1; listctx_set_simpl.
+Qed.
+
 (* Lemma basic_typing_subst_value_post *)
 
 Lemma eval_op_type_safe: forall op c1 c2 c3 (T1 T2 T3: base_ty),
@@ -203,7 +219,7 @@ Proof.
   repeat split; intros; destruct op; inversion H; subst; rewrite op_ty_spec in H0; inversion H0; subst; auto.
 Qed.
 
-Lemma eval_op_preservation_aux: forall Γ op c1 c2 c3 (T1 T2 T3: base_ty),
+Lemma eval_op_preservation: forall Γ op c1 c2 c3 (T1 T2 T3: base_ty),
     eval_op op c1 c2 c3 ->
     ty_of_op op = T1 ⤍ T2 ⤍ T3 ->
     ok Γ ->
@@ -214,15 +230,15 @@ Proof.
   repeat destruct_hyp_conj; subst. repeat split; auto.
 Qed.
 
-Lemma eval_op_preservation: forall Γ op c1 c2 c3 (T1 T2 T3: base_ty),
-    eval_op op c1 c2 c3 ->
-    Γ ⊢t op ⋮v T1 ⤍ T2 ⤍ T3 ->
-    Γ ⊢t c1 ⋮v T1 /\ Γ ⊢t c2 ⋮v T2 /\ Γ ⊢t c3 ⋮v T3.
-Proof.
-  intros.
-  inversion H0; subst.
-  eapply eval_op_preservation_aux; eauto.
-Qed.
+(* Lemma eval_op_preservation: forall Γ op c1 c2 c3 (T1 T2 T3: base_ty), *)
+(*     eval_op op c1 c2 c3 -> *)
+(*     ty_of_op op = T1 ⤍ T2 ⤍ T3 -> *)
+(*     Γ ⊢t c1 ⋮v T1 /\ Γ ⊢t c2 ⋮v T2 /\ Γ ⊢t c3 ⋮v T3. *)
+(* Proof. *)
+(*   intros. *)
+(*   inversion H0; subst. *)
+(*   eapply eval_op_preservation_aux; eauto. *)
+(* Qed. *)
 
 Ltac basic_typing_simpl1 :=
   step_regular_simp;
@@ -232,11 +248,38 @@ Ltac basic_typing_simpl1 :=
     | [H: ?Γ ⊢t (tvalue ?v) ⋮t ?T |- _ ] => inversion H; subst; clear H; auto
     end.
 
+Lemma basic_typing_weaken_tm_empty: forall Γ (e: tm) (T: ty), ok Γ -> [] ⊢t e ⋮t T -> Γ ⊢t e ⋮t T.
+Proof.
+  intros.
+  assert (Γ = [] ++ Γ) by auto. rewrite H1.
+  apply basic_typing_weaken_tm_pre; basic_typing_solver1.
+Qed.
+
+Lemma basic_typing_weaken_value_empty: forall Γ (e: value) (T: ty), ok Γ -> [] ⊢t e ⋮v T -> Γ ⊢t e ⋮v T.
+Proof.
+  intros.
+  assert (Γ = [] ++ Γ) by auto. rewrite H1.
+  apply basic_typing_weaken_value_pre; basic_typing_solver1.
+Qed.
+
+Lemma ty_tlete_dummy: forall Γ Tx T (e_x e: tm), Γ ⊢t e_x ⋮t Tx -> Γ ⊢t e ⋮t T -> Γ ⊢t (tlete e_x e) ⋮t T.
+Proof.
+  intros.
+  auto_exists_L; intros. rewrite open_rec_lc_tm; basic_typing_solver1.
+  apply basic_typing_weaken_tm_pre; auto; basic_typing_solver1.
+Qed.
 
 Ltac basic_typing_solver2 :=
   basic_typing_simpl1;
   try match goal with
-    | [H: ?Γ ⊢t (vbiop _) ⋮v _ ⤍ _ ⤍ ?T |- ?Γ ⊢t (vconst _) ⋮v ?T ] => eapply eval_op_preservation; eauto
+    | [H: ?Γ ⊢t ?e ⋮v ?T |- _ ⊢t (tvalue ?e) ⋮t _ ] => constructor; auto
+    | [H: ty_of_op _ =  _ ⤍ _ ⤍ ?T |- ?Γ ⊢t (vconst _) ⋮v ?T ] => eapply eval_op_preservation; eauto
+    | [H: [] ⊢t ?e ⋮t ?T |- _ ⊢t ?e ⋮t ?T ] => apply basic_typing_weaken_tm_empty; eauto
+    | [H: [] ⊢t ?e ⋮v ?T |- _ ⊢t ?e ⋮v ?T ] => apply basic_typing_weaken_value_empty; eauto
+    | [H: ?Γ ⊢t ?e ⋮t ?T |- (?Γ ++ _) ⊢t ?e ⋮t ?T ] =>
+        apply basic_typing_weaken_tm_pre; auto; basic_typing_solver2
+    | [H: ?Γ ⊢t ?e1 ⋮t _, H': ?Γ ⊢t ?e2 ⋮t ?T |- ?Γ ⊢t tlete ?e1 ?e2 ⋮t ?T ] =>
+        eapply ty_tlete_dummy; eauto
     end;
   (basic_typing_solver1).
 
@@ -283,6 +326,27 @@ Proof.
   intros.
   eapply multi_preservation in H0; eauto. inversion H0; subst; auto.
 Qed.
+
+(* Facts *)
+
+Lemma empty_basic_typing_eval_op_result_exists: forall (op:biop) (v1 v2: value) (T1 T2 Tx: base_ty),
+    ty_of_op op = T1 ⤍ T2 ⤍ Tx -> [] ⊢t v2 ⋮v T2 -> [] ⊢t v1 ⋮v T1 ->
+    exists (c1 c2 c3: constant), v1 = c1 /\ v2 = c2 /\ eval_op op c1 c2 c3 /\ [] ⊢t c3 ⋮v Tx.
+Proof.
+  intros.
+  inversion H; subst.
+  assert (exists (c1: constant), v1 = c1) as Htmp. eapply empty_basic_typing_base_const_exists; eauto. destruct Htmp; subst.
+  assert (exists (c2: constant), v2 = c2) as Htmp. eapply empty_basic_typing_base_const_exists; eauto. destruct Htmp; subst.
+  destruct op;
+    simpl in H0; apply empty_basic_typing_nat_value_exists in H0; destruct H0; subst;
+    simpl in H1; apply empty_basic_typing_nat_value_exists in H1; destruct H1; subst.
+  - exists x2, x1, (x2 + x1). repeat split; auto. econstructor; auto.
+  - exists x2, x1, (Nat.eqb x2 x1). repeat split; auto. econstructor; auto.
+  - exists x2, x1, (Nat.ltb x2 x1). repeat split; auto. econstructor; auto.
+  - exists x2, x1, 0. repeat split; auto. econstructor; auto.
+Qed.
+
+(* Ltacs *)
 
 Ltac op_simpl :=
   basic_typing_simpl1;
@@ -385,3 +449,216 @@ Ltac basic_typing_vfavr_solver :=
   | [|- (_ ++ _) ⊢t (vfvar ?x) ⋮v _] =>
       apply basic_typing_weaken_value_post; eauto; basic_typing_vfavr_solver
   end.
+
+(* Lemma basic_typing_subst_value_post: forall Γ1 z u U (v: value) T, *)
+(*     ((z, U) :: Γ1) ⊢t v ⋮v T -> [] ⊢t u ⋮v U -> Γ1 ⊢t {z := u}v v ⋮v T. *)
+(* Proof. *)
+(*   intros. *)
+(*   assert (([] ++ [(z, U)] ++ Γ1) ⊢t v ⋮v T) by listctx_set_simpl. *)
+(*   apply (basic_typing_subst_value [] z u) in H1; listctx_set_simpl. *)
+(* Qed. *)
+
+(* Lemma basic_typing_subst_tm_post: forall Γ1 z u U (v: tm) T, *)
+(*     ((z, U) :: Γ1) ⊢t v ⋮t T -> [] ⊢t u ⋮v U -> Γ1 ⊢t {z := u}t v ⋮t T. *)
+(* Proof. *)
+(*   intros. *)
+(*   assert (([] ++ [(z, U)] ++ Γ1) ⊢t v ⋮t T) by listctx_set_simpl. *)
+(*   apply (basic_typing_subst_tm [] z u) in H1; listctx_set_simpl. *)
+(* Qed. *)
+
+Ltac basic_typing_solver3 :=
+  match goal with
+  | [H: [] ⊢t ?v ⋮v _ |- closed_value ?v ] => apply basic_typing_contains_fv_value in H; basic_typing_solver2
+  | [H: [] ⊢t ?e ⋮t _ |- closed_tm ?e ] => apply basic_typing_contains_fv_tm in H; basic_typing_solver2
+  | [H: ((?z, ?U) :: ?Γ1) ⊢t ?v ⋮v ?T , H': [] ⊢t ?u ⋮v ?U |- ?Γ1 ⊢t {?z := ?u}v ?v ⋮v ?T] => eapply basic_typing_subst_value_post; eauto
+  | [H: ((?z, ?U) :: ?Γ1) ⊢t ?v ⋮t ?T , H': [] ⊢t ?u ⋮v ?U |- ?Γ1 ⊢t {?z := ?u}t ?v ⋮t ?T] => eapply basic_typing_subst_tm_post; eauto
+  | [H: [] ⊢t ?u ⋮v _ |- context [ fv_value ?u] ] =>
+      assert (fv_value u = ∅) as Htmp by
+        (apply basic_typing_contains_fv_value in H; set_solver);
+      rewrite Htmp; auto; try clear Htmp; try fast_set_solver
+  | [H: ?Γ ⊢t ?e ⋮t ?T, H': ?e ↪* (tvalue ?v) |- ?Γ ⊢t ?v ⋮v ?T ] =>
+      eapply multi_preservation_value; eauto
+  end || basic_typing_solver2.
+
+Lemma closed_has_type_under_empty_value: forall Γ (v: value) T, Γ ⊢t v ⋮v T -> closed_value v -> [] ⊢t v ⋮v T.
+Proof.
+  apply (rev_ind (fun Γ => forall (v: value) T, Γ ⊢t v ⋮v T -> closed_value v -> [] ⊢t v ⋮v T)); intros; auto.
+  auto_destruct_pair.
+  destruct (tricky_closed_value_exists t) as (vv & Hvv).
+  apply (basic_typing_subst_value_pre _ a vv) in H0. rewrite subst_fresh_value in H0. auto. my_set_solver.
+  apply Hvv. op_simpl.
+Qed.
+
+Lemma closed_has_type_under_empty_tm: forall Γ (v: tm) T, Γ ⊢t v ⋮t T -> closed_tm v -> [] ⊢t v ⋮t T.
+Proof.
+  apply (rev_ind (fun Γ => forall (v: tm) T, Γ ⊢t v ⋮t T -> closed_tm v -> [] ⊢t v ⋮t T)); intros; auto.
+  auto_destruct_pair.
+  destruct (tricky_closed_value_exists t) as (vv & Hvv).
+  apply (basic_typing_subst_tm_pre _ a vv) in H0. rewrite subst_fresh_tm in H0. auto. my_set_solver.
+  apply Hvv. op_simpl.
+Qed.
+
+Lemma basic_has_type_swap_tm_aux: forall Γ e T,
+    Γ ⊢t e ⋮t T -> (forall Γ1 Γ2 Γ3, Γ = Γ1 ++ Γ2 ++ Γ3 -> (Γ2 ++ Γ1 ++ Γ3) ⊢t e ⋮t T).
+Proof.
+ apply (tm_has_type_mutual_rec
+           (fun Γ e T P => forall Γ1 Γ2 Γ3, Γ = Γ1 ++ Γ2 ++ Γ3 -> (Γ2 ++ Γ1 ++ Γ3) ⊢t e ⋮v T)
+           (fun Γ e T P => forall Γ1 Γ2 Γ3, Γ = Γ1 ++ Γ2 ++ Γ3 -> (Γ2 ++ Γ1 ++ Γ3) ⊢t e ⋮t T)
+        ); simpl; intros; subst; listctx_set_simpl.
+ - constructor. listctx_set_solver5.
+ - constructor. listctx_set_solver5.
+   rewrite ctxfind_app in e; try listctx_set_solver5.
+   rewrite ctxfind_app in e; try listctx_set_solver5.
+   destruct_hyp_disj; rewrite ctxfind_app; try listctx_set_solver5.
+   + right. rewrite ctxfind_app; listctx_set_solver5.
+   + right. rewrite ctxfind_app; listctx_set_solver5.
+ - auto_exists_L; intros.
+   assert ((Γ2 ++ Γ1 ++ (Γ3 ++ [(x, Tx)])) ⊢t e ^t^ x ⋮t T).
+   { apply H; listctx_set_solver5. }
+   listctx_set_solver5.
+ - auto_exists_L; intros.
+   assert ((Γ2 ++ Γ1 ++ (Γ3 ++ [(f, Tx ⤍ T)])) ⊢t vlam Tx e ^v^ f ⋮v Tx ⤍ T).
+   { apply H; listctx_set_solver5. }
+   listctx_set_solver5.
+ - constructor. listctx_set_solver5.
+ - auto_exists_L; intros.
+   assert ((Γ2 ++ Γ1 ++ (Γ3 ++ [(x, T1)])) ⊢t e2 ^t^ x ⋮t T2).
+   { apply H0; listctx_set_solver5. }
+   listctx_set_solver5.
+ - auto_exists_L; intros.
+   assert ((Γ2 ++ Γ1 ++ (Γ3 ++ [(x, TBase Tx)])) ⊢t e ^t^ x ⋮t T).
+   { apply H1; listctx_set_solver5. }
+   listctx_set_solver5.
+ - auto_exists_L; intros.
+   assert ((Γ2 ++ Γ1 ++ (Γ3 ++ [(x, Tx)])) ⊢t e ^t^ x ⋮t T).
+   { apply H1; listctx_set_solver5. }
+   listctx_set_solver5.
+Qed.
+
+Lemma basic_has_type_swap_tm: forall Γ1 Γ2 Γ3 e T,
+    (Γ1 ++ Γ2 ++ Γ3) ⊢t e ⋮t T <-> (Γ2 ++ Γ1 ++ Γ3) ⊢t e ⋮t T.
+Proof.
+  split; intros; eapply basic_has_type_swap_tm_aux in H; eauto.
+Qed.
+
+Lemma basic_has_type_swap_value_aux: forall Γ e T,
+    Γ ⊢t e ⋮v T -> (forall Γ1 Γ2 Γ3, Γ = Γ1 ++ Γ2 ++ Γ3 -> (Γ2 ++ Γ1 ++ Γ3) ⊢t e ⋮v T).
+Proof.
+ apply (value_has_type_mutual_rec
+           (fun Γ e T P => forall Γ1 Γ2 Γ3, Γ = Γ1 ++ Γ2 ++ Γ3 -> (Γ2 ++ Γ1 ++ Γ3) ⊢t e ⋮v T)
+           (fun Γ e T P => forall Γ1 Γ2 Γ3, Γ = Γ1 ++ Γ2 ++ Γ3 -> (Γ2 ++ Γ1 ++ Γ3) ⊢t e ⋮t T)
+        ); simpl; intros; subst; listctx_set_simpl.
+ - constructor. listctx_set_solver5.
+ - constructor. listctx_set_solver5.
+   rewrite ctxfind_app in e; try listctx_set_solver5.
+   rewrite ctxfind_app in e; try listctx_set_solver5.
+   destruct_hyp_disj; rewrite ctxfind_app; try listctx_set_solver5.
+   + right. rewrite ctxfind_app; listctx_set_solver5.
+   + right. rewrite ctxfind_app; listctx_set_solver5.
+ - auto_exists_L; intros.
+   assert ((Γ2 ++ Γ1 ++ (Γ3 ++ [(x, Tx)])) ⊢t e ^t^ x ⋮t T).
+   { apply H; listctx_set_solver5. }
+   listctx_set_solver5.
+ - auto_exists_L; intros.
+   assert ((Γ2 ++ Γ1 ++ (Γ3 ++ [(f, Tx ⤍ T)])) ⊢t vlam Tx e ^v^ f ⋮v Tx ⤍ T).
+   { apply H; listctx_set_solver5. }
+   listctx_set_solver5.
+ - constructor. listctx_set_solver5.
+ - auto_exists_L; intros.
+   assert ((Γ2 ++ Γ1 ++ (Γ3 ++ [(x, T1)])) ⊢t e2 ^t^ x ⋮t T2).
+   { apply H0; listctx_set_solver5. }
+   listctx_set_solver5.
+ - auto_exists_L; intros.
+   assert ((Γ2 ++ Γ1 ++ (Γ3 ++ [(x, TBase Tx)])) ⊢t e ^t^ x ⋮t T).
+   { apply H1; listctx_set_solver5. }
+   listctx_set_solver5.
+ - auto_exists_L; intros.
+   assert ((Γ2 ++ Γ1 ++ (Γ3 ++ [(x, Tx)])) ⊢t e ^t^ x ⋮t T).
+   { apply H1; listctx_set_solver5. }
+   listctx_set_solver5.
+Qed.
+
+Lemma basic_has_type_swap_value: forall Γ1 Γ2 Γ3 e T,
+    (Γ1 ++ Γ2 ++ Γ3) ⊢t e ⋮v T <-> (Γ2 ++ Γ1 ++ Γ3) ⊢t e ⋮v T.
+Proof.
+  split; intros; eapply basic_has_type_swap_value_aux in H; eauto.
+Qed.
+
+Lemma basic_has_type_swap2_tm: forall Γ1 Γ2 e T,
+    (Γ1 ++ Γ2) ⊢t e ⋮t T <-> (Γ2 ++ Γ1) ⊢t e ⋮t T.
+Proof.
+  intros.
+  assert ((Γ1 ++ Γ2 ++ []) ⊢t e ⋮t T <-> (Γ2 ++ Γ1 ++ []) ⊢t e ⋮t T).
+  eapply basic_has_type_swap_tm. listctx_set_simpl.
+Qed.
+
+Lemma basic_has_type_swap2_value: forall Γ1 Γ2 e T,
+    (Γ1 ++ Γ2) ⊢t e ⋮v T <-> (Γ2 ++ Γ1) ⊢t e ⋮v T.
+Proof.
+  intros.
+  assert ((Γ1 ++ Γ2 ++ []) ⊢t e ⋮v T <-> (Γ2 ++ Γ1 ++ []) ⊢t e ⋮v T).
+  eapply basic_has_type_swap_value. listctx_set_simpl.
+Qed.
+
+Lemma basic_has_type_head_to_tail_tm: forall x Tx Γ e T, ((x, Tx) :: Γ) ⊢t e ⋮t T <-> (Γ ++ [(x, Tx)]) ⊢t e ⋮t T.
+Proof.
+  split; intros.
+  - assert (([(x, Tx)] ++ Γ ++ []) ⊢t e ⋮t T) by listctx_set_simpl.
+    rewrite basic_has_type_swap_tm in H0. listctx_set_simpl.
+  - assert ((Γ ++ [(x, Tx)] ++ []) ⊢t e ⋮t T) by listctx_set_simpl.
+    rewrite basic_has_type_swap_tm in H0. listctx_set_simpl.
+Qed.
+
+Lemma basic_has_type_head_to_tail_value: forall x Tx Γ e T, ((x, Tx) :: Γ) ⊢t e ⋮v T <-> (Γ ++ [(x, Tx)]) ⊢t e ⋮v T.
+Proof.
+  split; intros.
+  - assert (([(x, Tx)] ++ Γ ++ []) ⊢t e ⋮v T) by listctx_set_simpl.
+    rewrite basic_has_type_swap_value in H0. listctx_set_simpl.
+  - assert ((Γ ++ [(x, Tx)] ++ []) ⊢t e ⋮v T) by listctx_set_simpl.
+    rewrite basic_has_type_swap_value in H0. listctx_set_simpl.
+Qed.
+
+Lemma basic_has_type_renaming: forall e γ x Tx x0 T,
+    x <> x0 ->
+    (γ ++ [(x, Tx)]) ⊢t e ⋮t T -> ok (γ ++ [(x0, Tx)]) ->
+    (γ ++ [(x0, Tx)]) ⊢t {x := x0 }t e ⋮t T.
+Proof.
+  intros.
+  assert (([(x0, Tx)] ++ (γ ++ [(x, Tx)])) ⊢t e ⋮t T).
+  { apply basic_typing_weaken_tm_post; auto.
+  listctx_set_simpl. rewrite ok_pre_destruct. split; basic_typing_solver3. }
+  assert ((((x0, Tx) :: γ) ++ [(x, Tx)]) ⊢t e ⋮t T) by listctx_set_simpl.
+  apply basic_typing_subst_tm with (u := x0) in H3; auto.
+  - listctx_set_simpl. rewrite <- basic_has_type_head_to_tail_tm; auto.
+  - econstructor; eauto; basic_typing_solver3. repeat var_dec_solver.
+Qed.
+
+
+Ltac basic_typing_solver4 :=
+  match goal with
+  | [H: (?Γ1 ++ ?Γ2) ⊢t ?e ⋮t ?T |- (?Γ2 ++ ?Γ1) ⊢t ?e ⋮t ?T ] => rewrite basic_has_type_swap2_tm; auto
+  | [H: (?Γ1 ++ ?Γ2) ⊢t ?e ⋮v ?T |- (?Γ2 ++ ?Γ1) ⊢t ?e ⋮v ?T ] => rewrite basic_has_type_swap2_value; auto
+  end || basic_typing_solver3.
+
+Ltac basic_typing_solver := basic_typing_solver4.
+
+Ltac lc_simpl :=
+  simpl;
+  repeat match goal with
+    | [H: context [(?e ^t^ ?x)] |- _ ] =>
+        simpl;
+        assert (lc e) as Htmp by (auto; (lc_solver || fast_set_solver || basic_typing_solver))
+        ;rewrite open_rec_lc_tm in H; auto; try clear Htmp
+    | [ |- context [(?e ^t^ ?x)] ] =>
+        simpl;
+        assert (lc e) as Htmp by (auto; (lc_solver || fast_set_solver || basic_typing_solver))
+        ;rewrite open_rec_lc_tm; auto; try clear Htmp
+    | [H: context [(?x \t\ ?e)] |- _ ] =>
+        simpl;
+        assert (x # e) as Htmp by (auto; (lc_solver || fast_set_solver || basic_typing_solver))
+        ;rewrite close_fresh_rec_tm in H; auto; try clear Htmp
+    | [ |- context [(?x \t\ ?e)] ] =>
+        simpl;
+        assert (x # e) as Htmp by (auto; (lc_solver || fast_set_solver || basic_typing_solver))
+        ;rewrite close_fresh_rec_tm; auto; try clear Htmp
+    end.
