new_proof/OperationalSemanticsProp.v
@@ -1,0 +1,204 @@
+From stdpp Require Import mapset.
+From Coq Require Import Logic.ClassicalFacts.
+From Coq Require Import Classical.
+From CT Require Import CoreLang.
+From CT Require Import CoreLangProp.
+From CT Require Import OperationalSemantics.
+
+Import Atom.
+Import CoreLang.
+Import Tactics.
+Import NamelessTactics.
+Import OperationalSemantics.
+
+Inductive multistep_length : tm -> tm -> nat -> Prop :=
+| multistep_length_refl : forall (x : tm),
+    lc x ->
+    multistep_length x x 0
+| multistep_length_step : forall (x y z : tm) n,
+    step x y ->
+    multistep_length y z n ->
+    multistep_length x z (S n).
+
+Notation "t1 '↪{' n '}' t2" := (multistep_length t1 t2 n) (at level 40).
+
+Lemma multistep_has_length: forall (e e': tm), e ↪* e' <-> (exists n, e ↪{n} e').
+Proof.
+  split; intros.
+  - induction H.
+    + exists 0. constructor; auto.
+    + destruct IHmultistep as (n & Hn). exists (S n). econstructor; eauto.
+  - destruct H as (n & Hn). generalize dependent e. generalize dependent e'.
+    induction n; intros; inversion Hn; subst.
+    + constructor; auto.
+    + eapply multistep_step; eauto.
+Qed.
+
+Lemma multi_step_length_regular: forall e1 e2 n, e1 ↪{n} e2 -> lc e1 /\ lc e2.
+Proof.
+  intros.
+  apply multi_step_regular. rewrite multistep_has_length. eexists; eauto.
+Qed.
+
+Ltac step_length_regular_simp1 :=
+  repeat match goal with
+    | [H: _ ↪ _ |- lc _] => apply step_regular in H; destruct H; auto
+    | [H: _ ↪ _ |- body _] => apply step_regular in H; destruct H; auto
+    | [H: _ ↪* _ |- lc _] => apply multi_step_regular in H; destruct H; auto
+    | [H: _ ↪* _ |- body _] => apply multi_step_regular in H; destruct H; auto
+    | [H: _ ↪{_} _ |- lc _] => apply multi_step_length_regular in H; destruct H; auto
+    | [H: _ ↪{_} _ |- body _] => apply multi_step_length_regular in H; destruct H; auto
+    | [H: ?a ↪{_} ?b |- ?a ↪* ?b] => rewrite multistep_has_length; eexists; eauto
+    end.
+
+Ltac step_length_regular_solver1 :=
+  step_length_regular_simp1; lc_solver.
+
+Theorem multistep_length_R : forall (x y : tm),
+    step x y -> multistep_length x y 1.
+Proof.
+  intros x y H.
+  apply multistep_length_step with y. apply H. apply multistep_length_refl; eauto.
+Qed.
+
+Theorem multistep_length_trans :
+  forall (x y z : tm) n1 n2,
+      multistep_length x y n1 ->
+      multistep_length y z n2 ->
+      multistep_length x z (n1 + n2).
+Proof.
+  intros.
+  induction H.
+    - (* multistep_refl *) simpl. assumption.
+    - rewrite PeanoNat.Nat.add_succ_l. econstructor; eauto.
+Qed.
+
+Lemma multi_ruduction_lete: forall n e_x e_x' e, body e -> e_x ↪{n} e_x' -> (tlete e_x e) ↪{n} (tlete e_x' e).
+Proof.
+  induction n; intros; invclear H0.
+  - constructor. lc_solver.
+  - econstructor; eauto.
+    econstructor; eauto.
+Qed.
+
+Lemma lete_reduction_spec_forward: forall n (e_x: tm) e (v: value),
+    (tlete e_x e ↪{n} v -> exists (v_x: value) n1 n2, n = S (n1 + n2) /\ e_x ↪{n1} v_x /\ e ^t^ v_x ↪{n2} v).
+Proof.
+  induction n; intros; invclear H.
+  - invclear H1.
+    + apply IHn in H4. destruct H4 as (v_x & n1 & n2 & HH). repeat destruct_hyp_conj.
+      exists v_x, (S n1), n2. repeat split; auto. econstructor; eauto.
+    + exists v1, 0, n. intros. repeat split; auto. constructor; auto.
+Qed.
+
+Lemma lete_reduction_spec_backward: forall n (e_x: tm) e (v: value),
+    (body e /\ exists (v_x: value) n1 n2, n = S (n1 + n2) /\ e_x ↪{n1} v_x /\ e ^t^ v_x ↪{n2} v) -> tlete e_x e ↪{n} v.
+Proof.
+  intros. repeat destruct_hyp_conj; subst.
+  assert (S (x0 + x1) = (x0 + S x1)) as Htmp by lia. rewrite Htmp. clear Htmp.
+  apply multistep_length_trans with (tlete x e). apply multi_ruduction_lete; eauto.
+  econstructor; eauto.
+  econstructor; eauto; step_length_regular_simp1.
+Qed.
+
+Lemma lete_reduction_spec: forall n (e_x: tm) e (v: value),
+    (tlete e_x e ↪{n} v <-> body e /\ exists (v_x: value) n1 n2, n = S (n1 + n2) /\ e_x ↪{n1} v_x /\ e ^t^ v_x ↪{n2} v).
+Proof.
+  split.
+  - split.
+    + step_length_regular_solver1.
+    + apply lete_reduction_spec_forward; auto.
+  - apply lete_reduction_spec_backward.
+Qed.
+
+Lemma letapp_reduction_spec_aux: forall (v1 v2 : value) e e',
+    tletapp v1 v2 e ↪ e' -> (exists T e1, v1 = vlam T e1) \/ (exists T (v1': value), v1 = vfix T v1').
+Proof.
+  intros.
+  invclear H.
+  - left. eexists; eauto.
+  - right. eexists; eauto.
+Qed.
+
+Lemma letapp_reduction_spec: forall n (v1 v2 : value) (v : value) e,
+    tletapp v1 v2 e ↪{n} v <->
+      exists n', n = S n' /\ lc v1 /\ lc v2 /\ body e /\
+              ((exists T e1,  v1 = vlam T e1 /\ (tlete (e1 ^t^ v2) e) ↪{n'} v) \/
+                 (exists T (v1': value), v1 = vfix T v1' /\ (tletapp (v1' ^v^ (vfix T v1')) v2 e) ↪{n'} v)).
+Proof.
+  split; intros.
+  - destruct n. inversion H.
+    exists n. repeat split; auto; step_length_regular_solver1. invclear H.
+    destruct (letapp_reduction_spec_aux v1 v2 _ _ H1); repeat destruct_hyp_conj; subst; invclear H1.
+    + left. repeat eexists; eauto.
+    + right. repeat eexists; eauto.
+  - repeat destruct_hyp_conj; subst.
+    destruct H3; repeat destruct_hyp_conj; subst.
+    + econstructor; eauto. econstructor; eauto; lc_solver.
+    + econstructor; eauto. econstructor; eauto; lc_solver.
+Qed.
+
+Lemma multistep_lete: forall e_x e_x' e, body e -> e_x ↪* e_x' -> (tlete e_x e) ↪* (tlete e_x' e).
+Proof.
+  intros. rewrite multistep_has_length in H0. rewrite multistep_has_length.
+  mydestr. eexists.
+  eapply multi_ruduction_lete; eauto.
+Qed.
+
+Lemma lete_step_spec: forall (e_x: tm) e (v: value),
+    (tlete e_x e ↪* v <-> body e /\ exists (v_x: value), e_x ↪* v_x /\ e ^t^ v_x ↪* v).
+Proof.
+  split; intros.
+  - split. step_length_regular_solver1.
+    rewrite multistep_has_length in H. mydestr. rewrite lete_reduction_spec in H. mydestr; subst.
+    eexists. split; rewrite multistep_has_length; eauto.
+  - mydestr. rewrite multistep_has_length.
+    rewrite multistep_has_length in H0.
+    rewrite multistep_has_length in H1.
+    mydestr.
+    exists (S (x1 + x0)). rewrite lete_reduction_spec. split; auto.
+    repeat eexists; repeat split; eauto.
+Qed.
+
+Lemma letapp_step_spec: forall (v1 v2: value) e (v: value),
+    tletapp v1 v2 e ↪* v <->
+       lc v1 /\ lc v2 /\ body e /\
+         ((exists T e1, v1 = vlam T e1 /\ (tlete (e1 ^t^ v2) e) ↪* v) \/
+                 (exists T (v1': value), v1 = vfix T v1' /\ (tletapp (v1' ^v^ (vfix T v1')) v2 e) ↪* v)).
+Proof.
+  split; intros.
+  - repeat split; step_length_regular_solver1.
+    rewrite multistep_has_length in H. mydestr. rewrite letapp_reduction_spec in H. mydestr; subst.
+    destruct_hyp_disj; mydestr; subst.
+    + left. repeat eexists; repeat split; eauto. step_length_regular_solver1.
+    + right. repeat eexists; repeat split; eauto. step_length_regular_solver1.
+  - mydestr.
+    destruct_hyp_disj; mydestr; subst; econstructor; eauto.
+    + econstructor; eauto. step_length_regular_solver1.
+    + econstructor; eauto. step_length_regular_solver1.
+Qed.
+
+Lemma terr_reduction_exfalso1: forall (v: value), ~ terr ↪* v.
+Proof.
+  intros. intro Hf. invclear Hf.
+  - inversion H.
+Qed.
+
+Ltac auto_reduction_exfalso1 :=
+  match goal with
+  | [H: ?P, H': ~ ?P |- _ ] => apply H' in H; inversion H
+  | [H: terr ↪ _ |- _ ] => inversion H
+  | [H: terr ↪* (tvalue _) |- _ ] => apply terr_reduction_exfalso1 in H; inversion H
+  end.
+
+Lemma tlete_terr_not_reduce_to_value: forall e (v: value), ~ tlete e terr ↪* v.
+Proof.
+  intros. intro Hf. rewrite lete_step_spec in Hf; mydestr. simpl in H1. auto_reduction_exfalso1.
+Qed.
+
+Ltac auto_reduction_exfalso2 :=
+  match goal with
+  | [H: tlete _ terr ↪* (tvalue _) |- _ ] => apply tlete_terr_not_reduce_to_value in H; invclear H
+  end || auto_reduction_exfalso1.
+
+Ltac auto_reduction_exfalso := auto_reduction_exfalso2.
