new_proof/RefinementDenotation.v
@@ -1,0 +1,231 @@
+From stdpp Require Import mapset.
+From stdpp Require Import natmap.
+From CT Require Import CoreLangProp.
+From CT Require Import OperationalSemanticsProp.
+From CT Require Import BasicTypingProp.
+From CT Require Import SyntaxSugar.
+From CT Require Import Refinement.
+From CT Require Import RefinementTac.
+
+Import Atom.
+Import CoreLang.
+Import Tactics.
+Import NamelessTactics.
+Import ListCtx.
+Import OperationalSemantics.
+Import OperationalSemanticsProp.
+Import BasicTyping.
+Import SyntaxSugar.
+Import Refinement.
+Import RefinementTac.
+
+(* Denotation: *)
+
+Fixpoint rR (n: nat) (bst: bstate) (st: state) (τ: rty) (e: tm) : Prop :=
+  [] ⊢t e ⋮t ⌊ τ ⌋ /\ closed_rty n (dom _ st) τ /\
+    match τ with
+    | {v: B | _ | _ | ϕ} => exists (c: constant), [] ⊢t c ⋮v B /\ ϕ bst st c /\ e = c
+    | [v: B | _ | _ | ϕ] => forall (c: constant), [] ⊢t c ⋮v B -> ϕ bst st c -> e ↪* c
+    | -:{v: B | _ | d | ϕ } ⤑ τ =>
+        forall (c_x: constant),
+          [] ⊢t c_x ⋮v B -> ϕ bst st c_x -> rR (S n) (<b[↦ c_x ]> bst) st τ (mk_app e c_x)
+    | τ1 ⤑ τ2 => forall (e_x: tm), rR n bst st τ1 e_x -> rR n bst st τ2 (mk_app e e_x)
+    end.
+
+Lemma bst_eq_trans: forall n n' (bst1 bst2: bstate), n' <= n -> bst_eq n bst1 bst2 -> bst_eq n' bst1 bst2.
+Proof.
+  intros. intro i; intros. apply H0. lia.
+Qed.
+
+Lemma closed_rty_n_overbase: forall (n1 n2: nat) d1 d2 B ϕ, closed_rty n1 d1 {v:B|n2|d2|ϕ} -> n2 <= n1.
+Proof.
+  intros. invclear H; mydestr. invclear H0. invclear H; auto.
+Qed.
+
+Lemma closed_rty_n_underbase: forall (n1 n2: nat) d1 d2 B ϕ, closed_rty n1 d1 [v:B|n2|d2|ϕ] -> n2 <= n1.
+Proof.
+  intros. invclear H; mydestr. invclear H0. invclear H; auto.
+Qed.
+
+Lemma closed_rty_0_overbase: forall (n2: nat) d1 d2 B ϕ, closed_rty 0 d1 {v:B|n2|d2|ϕ} -> n2 = 0.
+Proof.
+  intros. apply closed_rty_n_overbase in H. lia.
+Qed.
+
+Lemma closed_rty_0_underbase: forall (n2: nat) d1 d2 B ϕ, closed_rty 0 d1 [v:B|n2|d2|ϕ] -> n2 = 0.
+Proof.
+  intros. apply closed_rty_n_underbase in H. lia.
+Qed.
+
+Lemma bst_eq_symmetry: forall n bst1 bst2, bst_eq n bst2 bst1 <-> bst_eq n bst1 bst2.
+Proof.
+  unfold bst_eq. split; intros; rewrite H; auto.
+Qed.
+
+Lemma bst_eq_push: forall n c_x bst1 bst2, bst_eq n bst1 bst2 -> bst_eq  (S n) (<b[↦c_x]> bst1) (<b[↦c_x]> bst2).
+Proof.
+  intros. intro i; intros.
+  destruct i; simpl; auto. apply H. lia.
+Qed.
+
+Lemma rR_bst_bound_: forall τ (e: tm) st n (bst1 bst2: bstate), bst_eq n bst1 bst2 -> rR n bst1 st τ e -> rR n bst2 st τ e.
+Proof.
+  induction τ; intros; auto; invclear H0; mydestr; subst.
+  - constructor; auto. constructor; auto. exists x. repeat split; auto.
+    invclear H0; mydestr. invclear H0. invclear H4. invclear H6. eapply H4; eauto.
+    rewrite bst_eq_symmetry in H. eapply bst_eq_trans; eauto.
+  - constructor; auto. constructor; auto. intros. apply H2; auto.
+    invclear H0; mydestr. invclear H0. invclear H5. invclear H7. eapply H5; eauto. eapply bst_eq_trans; eauto.
+  - constructor; auto. constructor; auto. intros.
+    apply IHτ with (bst1 := (<b[↦c_x]> bst1)). apply bst_eq_push; auto. apply H2; auto.
+    invclear H0; mydestr. invclear H5. invclear H10. eapply H7; eauto. invclear H0. eapply bst_eq_trans; eauto.
+  - constructor; auto. constructor; auto. intros. eapply IHτ2; eauto. apply H2; auto.
+    eapply IHτ1; eauto. rewrite bst_eq_symmetry; auto.
+Qed.
+
+Lemma rR_bst_bound: forall τ (e: tm) st n (bst1 bst2: bstate), bst_eq n bst1 bst2 -> rR n bst1 st τ e <-> rR n bst2 st τ e.
+Proof.
+  split; intros; eapply rR_bst_bound_; eauto. rewrite bst_eq_symmetry; eauto.
+Qed.
+
+Lemma rR_0_empty_iff_forall: forall τ (e: tm) st, (forall bst1, rR 0 bst1 st τ e) <-> rR 0 b∅ st τ e.
+Proof.
+  split; intros; auto. rewrite rR_bst_bound; eauto. intro i; intros. invclear H0.
+Qed.
+
+Notation " '{' n ';' bst ';' st '}⟦' τ '⟧' " :=
+  (rR n bst st τ) (at level 20, format "{ n ; bst ; st }⟦ τ ⟧", bst constr, st constr, τ constr).
+Notation " '{' st '}⟦' τ '⟧' " := (fun e => rR 0 b∅ st τ e) (at level 20, format "{ st }⟦ τ ⟧", st constr, τ constr).
+Notation " '⟦' τ '⟧' " := (fun e => rR 0 b∅ ∅ τ e) (at level 20, format "⟦ τ ⟧", τ constr).
+
+(* regular of the denation *)
+
+Lemma rR_regular1:
+  forall τ n bst st e, { n; bst; st }⟦ τ ⟧ e -> closed_rty n (dom _ st) τ /\ [] ⊢t e ⋮t ⌊ τ ⌋.
+Proof.
+  induction τ; intros; invclear H; mydestr; subst; split; intros; auto.
+Qed.
+
+Lemma rR_regular2:
+  forall τ st e, { st }⟦ τ ⟧ e -> closed_rty 0 (dom _ st) τ /\ [] ⊢t e ⋮t ⌊ τ ⌋.
+Proof.
+  intros. eapply rR_regular1; eauto.
+Qed.
+
+Lemma rR_regular3:
+  forall τ e, ⟦ τ ⟧ e -> (closed_rty 0 ∅ τ) /\ [] ⊢t e ⋮t ⌊ τ ⌋.
+Proof.
+  intros. eapply rR_regular2 in H. mydestr; split; auto.
+Qed.
+
+Inductive ctxrR: state -> listctx rty -> rty -> tm -> Prop :=
+| ctxrR_nil: forall st τ e, { st }⟦ τ ⟧ e -> ctxrR st [] τ e
+| ctxrR_cons_over: forall st (x: atom) B n d ϕ Γ τ (e: tm),
+    closed_rty 0 ({[x]} ∪ ctxdom Γ ∪ (dom _ st)) τ ->
+    ok_dctx (dom _ st) ((x, {v: B | n | d | ϕ}) :: Γ) ->
+    ((x, TBase B) :: (⌊Γ⌋*)) ⊢t e ⋮t ⌊τ⌋ ->
+     (forall (c_x: constant), {st}⟦ {v: B | n | d | ϕ} ⟧ c_x ->
+                         ctxrR (<[ x := c_x ]> st) Γ τ (tlete c_x ({ 0 <t~ x} e))) ->
+     ctxrR st ((x, {v: B | n | d | ϕ}) :: Γ) τ e
+| ctxrR_cons_under: forall st (x: atom) τ_x τ Γ e,
+    not_overbasety τ_x ->
+    closed_rty 0 ({[x]} ∪ ctxdom Γ ∪ (dom _ st)) τ ->
+    ok_dctx (dom _ st) ((x, τ_x) :: Γ) ->
+    ((x, ⌊τ_x⌋ ) :: (⌊Γ⌋*)) ⊢t e ⋮t ⌊τ⌋ ->
+     (exists e_x_hat, {st}⟦ τ_x ⟧ e_x_hat /\
+                   (forall e_x, {st}⟦ τ_x ⟧ e_x ->
+                           (∀ (v_x: value), e_x_hat ↪* v_x ->
+                                            ctxrR ({ x ↦ v_x } st) Γ τ (tlete e_x ({ 0 <t~ x} e))))) ->
+     ctxrR st ((x, τ_x) :: Γ) τ e.
+
+Notation " '{' st '}⟦' τ '⟧{' Γ '}' " := (ctxrR st Γ τ) (at level 20, format "{ st }⟦ τ ⟧{ Γ }", st constr, τ constr, Γ constr).
+Notation " '⟦' τ '⟧{' Γ '}' " := (ctxrR ∅ Γ τ) (at level 20, format "⟦ τ ⟧{ Γ }", τ constr, Γ constr).
+
+Lemma ctxrR_regular0:
+  forall Γ τ st e, { st }⟦ τ ⟧{ Γ } e ->
+              closed_rty 0 (ctxdom Γ ∪ (dom _ st)) τ /\ ok_dctx (dom _ st) Γ.
+Proof.
+  induction Γ; simpl; intros; invclear H; simpl; auto.
+  - apply rR_regular2 in H0; mydestr.
+    constructor; simpl; auto.
+    + closed_rty_solver.
+    + constructor.
+Qed.
+
+(* Lemma ctxrR_wf_regular: *)
+(*   forall Γ τ d, ctxrR_wf d Γ τ -> (ok_dctx d Γ) /\ cl_dctx d Γ /\ closed_rty 0 (ctxdom Γ ∪ d) τ. *)
+(* Proof. *)
+(*   induction Γ; simpl; intros; invclear H; simpl. *)
+(*   - split. repeat constructor; auto; fast_set_solver. *)
+(*     split. constructor. *)
+(*     closed_rty_solver. *)
+(*   - mydestr. *)
+(*     assert (ctxrR_wf ({[a]} ∪ d) Γ τ) by (split; try closed_rty_solver; invclear H1; auto). *)
+(*     apply IHΓ in H. mydestr; listctx_set_simpl. invclear H1. *)
+(*     split; auto. split; auto. constructor; auto. *)
+(* Qed. *)
+
+Lemma ctxrR_regular1:
+  forall Γ τ st e, { st }⟦ τ ⟧{ Γ } e ->
+              (ok_dctx (dom _ st) Γ) /\
+                ctx_closed_rty (dom _ st) Γ /\
+                closed_rty 0 (ctxdom Γ ∪ (dom _ st)) τ.
+Proof.
+  intros. apply ctxrR_regular0 in H. mydestr.
+  do 2 (split; auto). apply ok_dctx_regular2 in H0; mydestr; auto.
+Qed.
+
+Lemma ctxrR_regular2:
+  forall Γ τ st e, { st }⟦ τ ⟧{ Γ } e -> ⌊ Γ ⌋* ⊢t e ⋮t ⌊ τ ⌋.
+Proof.
+  induction Γ; simpl; intros; invclear H; simpl; auto.
+  - apply rR_regular2 in H0; mydestr; auto.
+Qed.
+
+Lemma ctxrR_regular:
+  forall Γ τ st e, { st }⟦ τ ⟧{ Γ } e ->
+              ⌊ Γ ⌋* ⊢t e ⋮t ⌊ τ ⌋ /\
+                (ok_dctx (dom _ st) Γ) /\
+                ctx_closed_rty (dom _ st) Γ /\
+                closed_rty 0 (ctxdom Γ ∪ (dom _ st)) τ.
+Proof.
+  intros. split.
+  - eapply ctxrR_regular2; eauto.
+  - eapply ctxrR_regular1; eauto.
+Qed.
+
+(* Lemma ctxrR_regular1: *)
+(*   forall Γ τ st e, { st }⟦ τ ⟧{ Γ } e -> closed_rty 0 (ctxdom Γ ∪ dom _ st) τ /\ *)
+(*                 ⌊ Γ ⌋* ⊢t e ⋮t ⌊ τ ⌋ /\ (ok_dctx (dom _ st) Γ). *)
+(* Proof. *)
+(*   induction Γ; simpl; intros; invclear H; simpl. *)
+(*   - apply rR_regular2 in H0; mydestr; split; intros; my_simplify_map_eq. *)
+(*     closed_rty_solver. *)
+(*     split; auto. constructor; auto. fast_set_solver. *)
+(*   - split; auto. closed_rty_solver. *)
+(*   - mydestr. split; auto. apply rR_regular2 in H; mydestr. closed_rty_solver. *)
+(* Qed. *)
+
+Inductive ctxrR2: bstate -> state -> listctx rty -> rty -> rty -> Prop :=
+| ctxrR2_nil: forall bst st τ1 τ2,
+    closed_rty 0 (dom _ st) τ1 -> closed_rty 0 (dom _ st) τ2 ->
+    (forall e, { st }⟦ τ1 ⟧ e -> { st }⟦ τ2 ⟧ e) ->
+    ctxrR2 bst st [] τ1 τ2
+| ctxrR2_cons_over: forall bst st (x: atom) B d ϕ Γ τ1 τ2,
+    ok_dctx (dom _ st) ((x, {v: B | 0 | d | ϕ}) :: Γ) ->
+    closed_rty 0 (ctxdom ((x, {v: B | 0 | d | ϕ}) :: Γ) ∪ dom _ st) τ1 ->
+    closed_rty 0 (ctxdom ((x, {v: B | 0 | d | ϕ}) :: Γ) ∪ dom _ st) τ2 ->
+    (forall (c_x: constant), {st}⟦ {v: B | 0 | d | ϕ} ⟧ c_x -> ctxrR2 bst (<[ x := c_x ]> st) Γ τ1 τ2) ->
+    ctxrR2 bst st ((x, {v: B | 0 | d | ϕ}) :: Γ) τ1 τ2
+| ctxrR2_cons_under: forall bst st (x: atom) τ_x τ1 τ2 Γ,
+    ok_dctx (dom _ st) ((x, τ_x) :: Γ) ->
+    closed_rty 0 (ctxdom ((x, τ_x) :: Γ) ∪ dom _ st) τ1 ->
+    closed_rty 0 (ctxdom ((x, τ_x) :: Γ) ∪ dom _ st) τ2 ->
+    not_overbasety τ_x ->
+    (exists e_x_hat, {st}⟦ τ_x ⟧ e_x_hat /\
+                  (forall e_x, {st}⟦ τ_x ⟧ e_x ->
+                          (∀ (v_x: value), e_x_hat ↪* v_x -> ctxrR2 bst ({ x ↦ v_x } st) Γ τ1 τ2))) ->
+    ctxrR2 bst st ((x, τ_x) :: Γ) τ1 τ2.
+
+Notation " '{' st '}⟦' τ1 '⟧⊆⟦' τ2 '⟧{' Γ '}' " := (forall bst, ctxrR2 bst st Γ τ1 τ2) (at level 20, format "{ st }⟦ τ1 ⟧⊆⟦ τ2 ⟧{ Γ }", st constr, τ1 constr, τ2 constr, Γ constr).
+Notation " '⟦' τ1 '⟧⊆⟦' τ2 '⟧{' Γ '}' " := (forall bst, ctxrR2 bst ∅ Γ τ1 τ2) (at level 20, format "⟦ τ1 ⟧⊆⟦ τ2 ⟧{ Γ }", τ1 constr, τ2 constr, Γ constr).
