new_proof/RefinementDenotationProp.v
@@ -1,0 +1,537 @@
+From stdpp Require Import mapset.
+From stdpp Require Import natmap.
+From stdpp Require Import fin_map_dom.
+From CT Require Import CoreLangProp.
+From CT Require Import OperationalSemanticsProp.
+From CT Require Import BasicTypingProp.
+From CT Require Import SyntaxSugar.
+From CT Require Import Refinement.
+From CT Require Import RefinementTac.
+From CT Require Import RefinementDenotation.
+From CT Require Import RefinementDenotationTac.
+From CT Require Import TermOrdering.
+From Coq Require Import Logic.ClassicalFacts.
+From Coq Require Import Classical.
+
+Import Atom.
+Import CoreLang.
+Import Tactics.
+Import NamelessTactics.
+Import ListCtx.
+Import OperationalSemantics.
+Import OperationalSemanticsProp.
+Import BasicTyping.
+Import SyntaxSugar.
+Import Refinement.
+Import RefinementTac.
+Import RefinementDenotation.
+Import RefinementDenotationTac.
+Import TermOrdering.
+
+Lemma over_inhabitant_only_constant: forall (u: value) st b n d ϕ,
+    ({0;b∅;st}⟦{v:b|n|d|ϕ}⟧) u -> (exists (c: constant), u = c).
+Proof.
+  intros. invclear H; mydestr. exists x. invclear H3. auto.
+Qed.
+
+Ltac RD_simp :=
+  repeat match goal with
+  | [H: ({_}⟦ _ ⟧{ [] }) _ |- _ ] => invclear H
+  | [|- ({_}⟦ _ ⟧{ [] }) _ ] => constructor
+  | [H: ({_}⟦_⟧{ (_, {v:_|_|_|_}) :: _ }) _ |- _ ] => invclear H; try auto_ty_exfalso
+  | [H: ({0;b∅;_}⟦{v:_|_|_|_}⟧) (tvalue ?u) |- _ ] =>
+      match u with
+      | vconst _ => idtac
+      | _ => destruct (over_inhabitant_only_constant _ _ _ _ _ _ H); subst
+      end
+  end.
+
+Ltac my_simplify_map_eq3 :=
+  repeat match goal with
+  | [ |- context [(<[?x:=?c_x]> (<[?x:=?c_y]> ?m))] ] =>
+      setoid_rewrite insert_insert; auto
+  | [ H: ?x <> ?y |- context [(<[?x:=?c_x]> (<[?y:=?c_y]> ?m))] ] =>
+      fail 1
+  | [ |- context [(<[?x:=?c_x]> (<[?y:=?c_y]> ?m))] ] =>
+      destruct (Atom.atom_dec x y); subst
+  end.
+
+Global Hint Constructors lc_rty_idx: core.
+
+Lemma closed_rty_subst_excluded_forward: forall (n1 n2: nat) (z: atom) (c: constant) B (d1 d2: aset) ϕ,
+    z ∉ d1 -> z ∈ d2 ->
+    closed_rty n1 ({[z]} ∪ d1) {v:B|n2|d2|ϕ} ->
+    closed_rty n1 d1 {v:B|n2|d2 ∖ {[z]}|refinement_subst z c ϕ}.
+Proof.
+  unfold closed_rty. intros; mydestr. repeat split.
+  - denotation_simp. invclear H1. constructor. invclear H5. constructor; auto.
+    + intros.
+      unfold not_fv_in_refinement. intros. unfold refinement_subst. simpl.
+      unfold not_fv_in_refinement in H1. unfold refinement_subst in H1.
+      destruct (atom_dec x z); subst.
+      { my_simplify_map_eq. destruct (m !! z); my_simplify_map_eq3. apply H1. set_solver.  }
+      amap_solver1 Hstx. setoid_rewrite insert_commute. apply H0. set_solver. set_solver.
+      apply H0. set_solver.
+      my_simplify_map_eq3. setoid_rewrite insert_commute; set_solver.
+    + unfold bound_in_refinement in H2. unfold bound_in_refinement. eauto.
+  - refinement_solver3.
+  - set_solver.
+Qed.
+
+(* Lemma closed_rty_subst_excluded_backward: forall (n1 n2: nat) (z: atom) (c: constant) B (d1 d2: aset) ϕ, *)
+(*     z ∉ d1 -> *)
+(*     closed_rty n1 d1 {v:B|n2|d2 ∖ {[z]}|refinement_subst z c ϕ} -> closed_rty n1 ({[z]} ∪ d1) {v:B|n2|d2|ϕ}. *)
+(* Proof. *)
+(*   unfold closed_rty. intros; mydestr. repeat split. *)
+(*   - invclear H0. constructor. simpl in H2. invclear H4. constructor; auto. *)
+(*     + intros. *)
+(*       unfold not_fv_in_refinement. intros. unfold refinement_subst. simpl. *)
+(*       unfold not_fv_in_refinement in H0. unfold refinement_subst in H0. simpl in H0. *)
+(*       assert (x ∉ d2 ∖ {[z]}) as Htmp by fast_set_solver. *)
+(*       apply H0 with (m:=m) (bst:=bst) (c0:=c0) (v:=v) in Htmp. *)
+(*       destruct (Atom.atom_dec x z); subst. *)
+(*       setoid_rewrite insert_insert in Htmp; auto. simpl in Htmp. *)
+
+(*       my_simplify_map_eq2. setoid_rewrite insert_commute; set_solver. *)
+(*     + unfold bound_in_refinement in H2. unfold bound_in_refinement. eauto. *)
+(*   - refinement_solver3. *)
+(*   - set_solver. *)
+(* Qed. *)
+
+Lemma denotation_st_update_iff_subst:
+  forall τ (z: atom) (c: constant) n bst (st: state) e,
+    z ∉ (dom aset st) ->
+    ({n;bst;<[z:=c]> st}⟦τ⟧) e <-> ({n;bst;st}⟦({z:=c}r) τ⟧) e.
+Proof.
+  induction τ; split; simpl; intros; mydestr; subst.
+  - destruct (decide (z ∈ d)).
+    + split; auto. split; auto. denotation_simp.
+    apply closed_rty_subst_excluded; auto.
+    eexists; eauto.
+  - split; auto. split; auto. apply closed_rty_subst_excluded; auto.
+
+    admit. eexists; eauto.
+  - split; auto. split; auto. admit.
+  - split; auto. split; auto. admit.
+  - split; auto. admit. split; auto. admit. intros. apply H1 in H3; auto. rewrite <- IHτ; auto.
+  - split; auto. admit. split; auto. admit. intros. apply H1 in H3; auto. rewrite IHτ; auto.
+  - split; auto. admit. split; auto. admit. intros.
+    rewrite <- IHτ1 in H2. apply H1 in H2; auto.
+    rewrite <- IHτ2; auto.
+  - split; auto. admit. split; auto. admit. intros.
+    rewrite IHτ1 in H2. apply H1 in H2; auto.
+    rewrite IHτ2; auto.
+Admitted.
+
+Lemma rRctx_backward_over: forall Γ st z b n d ϕ (e: tm) τ,
+    {st}⟦ τ ⟧{ Γ ++ [(z, {v: b | n | d | ϕ})] } e <->
+    (forall (u: value), {st}⟦ {v: b | n | d | ϕ} ⟧{ Γ } u -> {st}⟦ { z := u }r τ ⟧{ Γ } ({ z := u }t e)).
+Proof.
+  induction Γ; split; simpl; intros; denotation_simp.
+  - RD_simp. apply H13 in H1. RD_simp. invclear H11.
+
+    
+
+  - constructor. admit. admit. admit. intros.
+    assert (({st}⟦{v:b|n|d|ϕ}⟧{ [] }) c_x). constructor; auto. apply H in H1.
+    invclear H1. constructor. admit.
+  - invclear H.
+    + constructor; auto. admit. admit. simpl. simpl in H9. ctx_erase_simp. admit.
+      intros. apply H10 in H. rewrite IHΓ in H. admit.
+    + mydestr. constructor; auto. admit. admit. admit.
+      eexists x. split; auto. intros. eapply H1 in H2; eauto.
+      rewrite IHΓ in H2.
+
+Admitted.
+
+Lemma rRctx_backward_under: forall Γ z τ_z (e: tm) τ,
+    ~ not_overbasety τ_z ->
+    ⟦ τ ⟧{ Γ ++ [(z, τ_z)] } e <->
+      (∃ (u_hat: tm), ⟦ τ_z ⟧{ Γ } u_hat /\
+                        (forall (u: tm), ⟦ τ_z ⟧{ Γ } u ->
+                                    (∀ (v_u: value), u_hat ↪* v_u -> ⟦ { z:= v_u }r τ ⟧{ Γ } (tlete u (e ^t^ z)))
+                        )).
+Admitted.
+
+Fixpoint random_inhabitant (τ: rty) :=
+  match τ with
+  | {v: _ | _ | _ | _ } => terr
+  | [v: TNat | _ | _ | _ ] => nat-gen
+  | [v: TBool | _ | _ | _ ] => bool-gen
+  | -:{v: T1 | _ | _ | _ } ⤑ τ => vlam T1 (random_inhabitant τ)
+  | τ1 ⤑ τ2 => vlam (rty_erase τ1) (random_inhabitant τ2)
+  end.
+
+(* Lemma no_halting_term_is_inhabitant: forall τ (st: state) n bst e, *)
+(*     not_overbasety τ -> *)
+(*     closed_rty n (dom aset st) τ -> *)
+(*     (∀ (v: value), ~ e ↪* v) -> [] ⊢t e ⋮t ⌊ τ ⌋ -> {n;bst;st}⟦τ⟧ e. *)
+(* Proof. *)
+(*   induction τ; simpl; intros. *)
+(*   - invclear H. *)
+(*   - constructor; auto. constructor; auto. intros. *)
+(*   intros. *)
+
+Inductive ctxrR_halt: state -> listctx rty -> rty -> tm -> Prop :=
+| ctxrR_halt_nil: forall st τ e, { st }⟦ τ ⟧ e -> ctxrR_halt st [] τ e
+| ctxrR_halt_cons_over: forall st (x: atom) B n d ϕ Γ τ (e: tm),
+    closed_rty 0 ({[x]} ∪ ctxdom Γ ∪ (dom _ st)) τ ->
+    ok_dctx (dom _ st) ((x, {v: B | n | d | ϕ}) :: Γ) ->
+    ((x, TBase B) :: (⌊Γ⌋*)) ⊢t e ⋮t ⌊τ⌋ ->
+     (forall (c_x: constant), {st}⟦ {v: B | n | d | ϕ} ⟧ c_x ->
+                         ctxrR_halt  (<[ x := c_x ]> st) Γ τ (tlete c_x ({ 0 <t~ x} e))) ->
+     ctxrR_halt st ((x, {v: B | n | d | ϕ}) :: Γ) τ e
+| ctxrR_halt_cons_under: forall st (x: atom) τ_x τ Γ e,
+    not_overbasety τ_x ->
+    closed_rty 0 ({[x]} ∪ ctxdom Γ ∪ (dom _ st)) τ ->
+    ok_dctx (dom _ st) ((x, τ_x) :: Γ) ->
+    ((x, ⌊τ_x⌋ ) :: (⌊Γ⌋*)) ⊢t e ⋮t ⌊τ⌋ ->
+     (exists e_x_hat, {st}⟦ τ_x ⟧ e_x_hat /\
+                   (∃ (v_x_hat: value), e_x_hat ↪* v_x_hat) /\
+                   (forall e_x, {st}⟦ τ_x ⟧ e_x ->
+                           (∀ (v_x: value), e_x_hat ↪* v_x ->
+                                            ctxrR_halt ({ x ↦ v_x } st) Γ τ (tlete e_x ({ 0 <t~ x} e))))) ->
+     ctxrR_halt  st ((x, τ_x) :: Γ) τ e.
+
+Inductive halt_ctx: state -> listctx rty -> Prop :=
+| halt_ctx_nil: ∀ st, halt_ctx st []
+| halt_ctx_cons_ubase: forall st Γ x b n d ϕ,
+    halt_ctx st Γ ->
+    ~ ({st}⟦ [v: b | n | d | ϕ ] ⟧{ Γ } terr) ->
+    halt_ctx st (Γ ++ [(x, [v: b | n | d | ϕ ])])
+| halt_ctx_cons: forall st Γ x τ,
+    not_underbasety τ ->
+    halt_ctx st Γ ->
+    halt_ctx st (Γ ++ [(x, τ)]).
+
+Inductive halt_ctx_rev: state -> listctx rty -> Prop :=
+| halt_ctx_rev_nil: ∀ st, halt_ctx_rev st []
+| halt_ctx_rev_cons_obase: forall st Γ x (b: base_ty) n d (ϕ: refinement),
+    (forall (c: constant), [] ⊢t c ⋮v b -> ϕ b∅ ∅ c -> halt_ctx_rev ({ x ↦ c } st) Γ) ->
+    halt_ctx_rev st ((x, {v: b | n | d | ϕ }) :: Γ)
+| halt_ctx_rev_cons_ubase: forall st Γ x (b: base_ty) n d (ϕ: refinement),
+    (exists (c: constant), ϕ b∅ ∅ c) ->
+    (forall (c: constant), [] ⊢t c ⋮v b -> halt_ctx_rev ({ x ↦ c } st) Γ) ->
+    halt_ctx_rev st ((x, [v: b | n | d | ϕ ]) :: Γ)
+| halt_ctx_rev_cons_arr: forall st Γ x τ,
+    is_arr τ -> halt_ctx_rev st Γ -> halt_ctx_rev st ((x, τ) :: Γ).
+
+Lemma halt_ctx_pre_destruct: forall Γ x b n d ϕ st,
+    halt_ctx st ((x, [v: b | n | d | ϕ ]) :: Γ) <->
+      (exists (c: constant), ϕ b∅ ∅ c) /\ (forall (c: constant), [] ⊢t c ⋮v b -> halt_ctx ({ x ↦ c } st) Γ).
+Proof.
+  apply (rev_ind (fun Γ => forall x b n d ϕ st,
+                      halt_ctx st ((x, [v: b | n | d | ϕ ]) :: Γ) <->
+                        (exists (c: constant), ϕ b∅ ∅ c) /\ (forall (c: constant), [] ⊢t c ⋮v b -> halt_ctx ({ x ↦ c } st) Γ)));
+  repeat split; simpl; intros.
+  - invclear H. admit. admit.
+  - constructor.
+  - mydestr. rewrite <- app_nil_l. constructor. constructor. admit.
+  - invclear H0.
+    + rewrite app_comm_cons in H1. apply app_inj_tail in H1. mydestr. invclear H1.
+      apply H in H2. mydestr. exists x. auto.
+    + rewrite app_comm_cons in H1. apply app_inj_tail in H1. mydestr. invclear H1.
+      apply H in H4. mydestr. exists x. auto.
+  - admit.
+  - mydestr. rewrite app_comm_cons. destruct (classic (not_underbasety r)).
+    + apply halt_ctx_cons; auto. rewrite H. split. exists x; auto. intros. apply H1 in H3. simpl. invclear H3.
+
+Lemma halt_ctx_implies_halt_ctx_rev: forall Γ, halt_ctx Γ -> halt_ctx_rev ∅ Γ.
+Proof.
+  induction Γ; intros.
+  - constructor.
+  - mydestr. invclear H.
+
+Lemma halt_ctx_plus_ctxrR_implies_ctxrR_halt: forall Γ τ e, halt_ctx Γ -> ⟦ τ ⟧{ Γ } e -> ctxrR_halt ∅ Γ τ e.
+Proof.
+  induction Γ; intros.
+  - invclear H0. constructor; auto.
+  - mydestr. invclear H.
+
+Lemma random_inhabitant_in_any_under: ∀ (τ: rty) (bst : bstate) n st,
+    not_overbasety τ ->
+    closed_rty n (dom _ st) τ ->
+    ({n;bst;st}⟦τ⟧) (random_inhabitant τ).
+Proof.
+  induction τ; intros; invclear H; mydestr.
+  - destruct B.
+    + split; simpl; auto. admit. split; auto. intros. admit.
+    + split; simpl; auto. apply mk_bool_gen_typable; auto. split; auto. intros. destruct c; invclear H.
+      apply mk_bool_gen_reduce_to_all_bool.
+  - denotation_simp. constructor; auto. admit. constructor; auto.
+    intros.
+    apply (termR_perserve_rR _ (random_inhabitant τ)); auto; try refinement_solver1. admit.
+    apply IHτ; refinement_solver1.
+  - denotation_simp. constructor; auto. admit. constructor; auto.
+    intros.
+    assert (exists (v_x: value), e_x ↪* v_x). admit. destruct H1.
+    apply (termR_perserve_rR _ (random_inhabitant τ2)); auto; try refinement_solver1. admit.
+    apply IHτ2; refinement_solver1.
+Admitted.
+
+Lemma denotation_weaken_empty: forall Γ (e: tm) τ (st: state),
+    not_overbasety τ ->
+    valid_rty τ ->
+    ok_dctx (dom _ st) Γ -> { st }⟦ τ ⟧ e -> {st}⟦ τ ⟧{ Γ } e.
+Proof.
+  induction Γ; intros; denotation_simp; mydestr.
+  constructor; auto.
+  destruct (classic (not_overbasety r)).
+  - constructor; auto; try refinement_solver1.
+    exists (random_inhabitant r); invclear H1;
+    assert (({0;b∅;st}⟦r⟧) (random_inhabitant r)) by
+      (intros; apply random_inhabitant_in_any_under; auto);
+    split; try (apply random_inhabitant_in_any_under; auto); intros.
+    + assert ([] ⊢t v_x ⋮v ⌊r⌋) as Hv_x by refinement_solver1.
+      destruct v_x; mydestr; simpl; try auto_ty_exfalso.
+      apply (termR_perserve_ctxrR _ _ e); auto. admit.
+      apply IHΓ; auto. denotation_simp. intros. rewrite rR_shadow_update_st; auto; refinement_solver1.
+      apply rR_regular1 in H2; mydestr. refinement_solver1.
+    + apply (termR_perserve_ctxrR _ _ e); auto. admit.
+      apply IHΓ; auto. denotation_simp. admit. admit.
+  - refinement_solver1. constructor; auto; try refinement_solver1.
+    intros. apply (termR_perserve_ctxrR _ _ e); auto. admit.
+    invclear H1; apply IHΓ; auto; try auto_ty_exfalso; try ok_dctx_solver_slow.
+    intros. rewrite rR_shadow_update_st; auto; refinement_solver1.
+    apply rR_regular1 in H2; mydestr. refinement_solver1.
+Admitted.
+
+Lemma denotation_weaken: forall Γ1 Γ3 (e: tm) τ (st: state) Γ2,
+    ctxrR_wf (dom _ st) (Γ1 ++ Γ2 ++ Γ3) τ -> {st}⟦ τ ⟧{ Γ1 ++ Γ3 } e -> {st}⟦ τ ⟧{ Γ1 ++ Γ2 ++ Γ3 } e.
+Proof.
+  intros. generalize dependent Γ2.
+  induction H0; intros; listctx_set_simpl.
+  - specialize (H b∅). invclear H; mydestr. denotation_simp.
+  induction Γ1; intros; listctx_set_simpl.
+  - admit.
+  - 
+
+Lemma err_exists_denotation_excluded: forall Γ b n (d: aset) (ϕ: refinement),
+    closed_rty 0 (dom aset (∅: state)) [v:b|n|d|ϕ] ->
+    ~ (⟦ [v: b | n | d | ϕ ] ⟧{ Γ } terr) -> (∃ (v: value), ⟦ {v: b | n | d | ϕ } ⟧{ Γ } v).
+Proof.
+  induction Γ; intros.
+  - destruct (classic (∃ v : value, (⟦{v:b|n|d|ϕ}⟧{ [] }) v)); auto; exfalso; apply H0; clear H0.
+    rewrite forall_iff_not_exists1 in H1.
+    constructor. intros.
+    do 2 constructor; auto. rewrite terr_reduction_iff_false_phi.
+    intros. intros Hf.
+    specialize (H1 c). apply H1.
+    constructor; auto. intros. constructor; auto. constructor; auto.
+    rewrite closed_rty_under_iff_over; auto.
+    exists c. constructor; auto. constructor; auto.
+    rewrite bound_in_refinement_0. apply Hf. refinement_solver1.
+  - mydestr. refinement_simp1.
+    destruct (classic (∃ v : value, (⟦{v:b|n|d|ϕ}⟧{ a :: Γ }) v)); auto; exfalso; apply H0; clear H0.
+    rewrite forall_iff_not_exists1 in H1.
+    mydestr.
+    constructor.
+
+
+    repeat match goal with
+           | [H: closed_rty _ _ _ |- bound_in_refinement _ _ ] => destruct H; mydestr
+           | [H: valid_rty _ |- bound_in_refinement _ _ ] => invclear H
+           | [H: wf_r _ _ ?ϕ |- bound_in_refinement _ ?ϕ ] =>  destruct H
+           end.
+    refinement_simp1; auto.
+    repeat match goal with
+    | [H: lc_rty_idx 0 [v:_|?n|_|_] |- _ ] =>
+        match n with
+        | 0 => fail 1
+        | _ =>  assert (n = 0) by (apply lc_rty_idx_under_0_is_0 in H; auto); subst
+        end
+    end.
+    repeat match goal with
+           | [H: closed_rty _ _ _ |- bound_in_refinement _ _ ] => destruct H; mydestr
+           | [H: valid_rty _ |- bound_in_refinement _ _ ] => invclear H
+           | [H: wf_r _ _ ?ϕ |- bound_in_refinement _ ?ϕ ] =>  destruct H
+           end.
+    assert (n = 0) by (apply lc_rty_idx_under_0_is_0 in H2; auto); subst.
+    invclear H2.
+    destruct H5. 
+    invclear H.
+ mydestr. invclear H. invclear H6. unfold bound_in_refinement in H5.
+    assert (closed_rty 0 ∅ [v:b|n|d|ϕ]). setoid_rewrite <- H2; auto.
+
+    setoid_rewrite H2 in H.
+
+    admit. auto.
+    intros. apply multistep_R.
+
+    constructor.
+    exfalso. apply H. constructor; intros. rewrite terr_inhabitant_iff_false_phi.
+
+
+  intros. destruct (classic (∃ v : value, (⟦[v:b|n|d|ϕ]⟧{Γ}) v)); auto.
+  exfalso. apply H. rewrite terr_inhabitant_iff_false_phi.
+
+  intro Hf. mydestr. invclear Hf.
+    + invclear H. denotation_simp.
+      match goal with
+      | [H: ∀ c, [] ⊢t (vconst c) ⋮v _ → _ _ ∅ c → terr ↪* (tvalue (vconst c)) |- _ ] => idtac H
+      end.
+      rewrite terr_inhabitant_implies_false_phi in H4.
+      apply H4 in H7.
+      repeat match goal with
+      | [H: _ ⊢t ?v ⋮v (TBase _) |- _ ] =>
+          match v with
+          | vconst _ => fail 1
+          | _ => set H7 as Htmp; apply empty_basic_typing_base_const_exists in Htmp; mydestr; subst
+          end
+      end.
+      set H7 as Htmp; apply empty_basic_typing_base_const_exists in Htmp; mydestr; subst.
+      match goal with
+      | [H: _ ⊢t (tvalue ?v) ⋮t _ |- _ ] => invclear H
+      end.
+
+      apply empty_basic_typing_base_const_exists in H.
+
+       specialize (H1 b∅).
+      invclear H0. invclear H1. mydestr.
+Admitted.
+
+(* Denotation: *)
+
+Fixpoint rR (n: nat) (bst: bstate) (st: state) (τ: rty) (e: tm) : Prop :=
+  [] ⊢t e ⋮t ⌊ τ ⌋ /\ closed_rty n (dom _ st) τ /\
+    match τ with
+    | {v: B | _ | _ | ϕ} => exists (c: constant), [] ⊢t c ⋮v B /\ ϕ bst st c /\ e = c
+    | [v: B | _ | _ | ϕ] => forall (c: constant), [] ⊢t c ⋮v B -> ϕ bst st c -> e ↪* c
+    | -:{v: B | _ | _ | ϕ } ⤑ τ =>
+        forall (c_x: constant), [] ⊢t c_x ⋮v B -> ϕ bst st c_x -> rR (S n) (<b[↦ c_x ]> bst) st τ (mk_app e c_x)
+    | τ1 ⤑ τ2 => forall (e_x: tm), rR n bst st τ1 e_x -> rR n bst st τ2 (mk_app e e_x)
+    end.
+
+Notation " '{' n ';' bst ';' st '}⟦' τ '⟧' " :=
+  (rR n bst st τ) (at level 20, format "{ n ; bst ; st }⟦ τ ⟧", bst constr, st constr, τ constr).
+Notation " '{' st '}⟦' τ '⟧' " := (fun e => forall bst, rR 0 bst st τ e) (at level 20, format "{ st }⟦ τ ⟧", st constr, τ constr).
+Notation " '⟦' τ '⟧' " := (fun e => forall bst, rR 0 bst ∅ τ e) (at level 20, format "⟦ τ ⟧", τ constr).
+
+(* regular of the denation *)
+
+Lemma rR_regular1:
+  forall τ n bst st e, { n; bst; st }⟦ τ ⟧ e -> closed_rty n (dom _ st) τ /\ [] ⊢t e ⋮t ⌊ τ ⌋.
+Proof.
+  induction τ; intros; invclear H; mydestr; subst; split; intros; auto.
+Qed.
+
+Lemma rR_regular2:
+  forall τ st e, { st }⟦ τ ⟧ e -> closed_rty 0 (dom _ st) τ /\ [] ⊢t e ⋮t ⌊ τ ⌋.
+Proof.
+  intros. specialize (H b∅). eapply rR_regular1; eauto.
+Qed.
+
+Lemma rR_regular3:
+  forall τ e, ⟦ τ ⟧ e -> (closed_rty 0 ∅ τ) /\ [] ⊢t e ⋮t ⌊ τ ⌋.
+Proof.
+  intros. eapply rR_regular2 in H. mydestr; split; auto.
+  intros. apply H. my_set_solver.
+Qed.
+
+Inductive ctxrR_wf: aset -> listctx rty -> rty -> Prop :=
+| ctxrR_wf_nil: forall d τ, closed_rty 0 d τ -> ctxrR_wf d [] τ
+| ctxrR_wf_cons_over: forall d (x: atom) τ_x Γ τ,
+    ok_dctx d ((x, τ_x) :: Γ) ->
+    closed_rty 0 d τ_x ->
+    ctxrR_wf ({[x]} ∪ d) Γ τ ->
+    ctxrR_wf d ((x, τ_x) :: Γ) τ.
+
+Inductive ctxrR: state -> listctx rty -> rty -> tm -> Prop :=
+| ctxrR_nil: forall st τ e, { st }⟦ τ ⟧ e -> ctxrR st [] τ e
+| ctxrR_cons_over: forall st (x: atom) B d ϕ Γ τ (e: tm),
+    ctxrR_wf (dom _ st) ((x, {v: B | 0 | d | ϕ}) :: Γ) τ ->
+    ((x, TBase B) :: (⌊Γ⌋*)) ⊢t e ⋮t ⌊τ⌋ ->
+     (forall (c_x: constant), {st}⟦ {v: B | 0 | d | ϕ} ⟧ c_x ->
+                         ctxrR (<[ x := c_x ]> st) Γ τ (tlete c_x ({ 0 <t~ x} e))) ->
+     ctxrR st ((x, {v: B | 0 | d | ϕ}) :: Γ) τ e
+| ctxrR_cons_under: forall st (x: atom) τ_x τ Γ e,
+        ctxrR_wf (dom _ st) ((x, τ_x) :: Γ) τ ->
+        ((x, ⌊τ_x⌋ ) :: (⌊Γ⌋*)) ⊢t e ⋮t ⌊τ⌋ ->
+         not_overbasety τ_x ->
+         (exists e_x_hat, {st}⟦ τ_x ⟧ e_x_hat /\
+                       (forall e_x, {st}⟦ τ_x ⟧ e_x ->
+                               (∀ (v_x: value), e_x_hat ↪* v_x ->
+                                                ctxrR ({ x ↦ v_x } st) Γ τ (tlete e_x ({ 0 <t~ x} e))))) ->
+         ctxrR st ((x, τ_x) :: Γ) τ e.
+
+Notation " '{' st '}⟦' τ '⟧{' Γ '}' " := (ctxrR st Γ τ) (at level 20, format "{ st }⟦ τ ⟧{ Γ }", st constr, τ constr, Γ constr).
+Notation " '⟦' τ '⟧{' Γ '}' " := (ctxrR ∅ Γ τ) (at level 20, format "⟦ τ ⟧{ Γ }", τ constr, Γ constr).
+
+Lemma ctxrR_implies_ctxrR_wf:
+  forall Γ τ st e, { st }⟦ τ ⟧{ Γ } e -> ctxrR_wf (dom _ st) Γ τ.
+Proof.
+  induction Γ; simpl; intros; invclear H; simpl; auto.
+  - apply rR_regular2 in H0; mydestr. constructor; auto.
+Qed.
+
+Lemma ctxrR_wf_regular:
+  forall Γ τ d, ctxrR_wf d Γ τ -> (ok_dctx d Γ) /\ cl_dctx d Γ /\ closed_rty 0 (ctxdom Γ ∪ d) τ.
+Proof.
+  induction Γ; simpl; intros; invclear H; simpl.
+  - split. repeat constructor; auto; fast_set_solver.
+    split. constructor.
+    closed_rty_solver.
+  - apply IHΓ in H6; mydestr2.
+    split; auto.
+    split. constructor; listctx_set_simpl. closed_rty_solver.
+Qed.
+
+Lemma ctxrR_regular0:
+  forall Γ τ st e, { st }⟦ τ ⟧{ Γ } e ->
+              (ok_dctx (dom _ st) Γ) /\ cl_dctx (dom _ st) Γ /\ closed_rty 0 (ctxdom Γ ∪ (dom _ st)) τ.
+Proof.
+  intros. apply ctxrR_wf_regular. eapply ctxrR_implies_ctxrR_wf; eauto.
+Qed.
+
+Lemma ctxrR_regular1:
+  forall Γ τ st e, { st }⟦ τ ⟧{ Γ } e -> ⌊ Γ ⌋* ⊢t e ⋮t ⌊ τ ⌋.
+Proof.
+  induction Γ; simpl; intros; invclear H; simpl; auto.
+  - apply rR_regular2 in H0; mydestr; auto.
+Qed.
+
+Lemma ctxrR_regular:
+  forall Γ τ st e, { st }⟦ τ ⟧{ Γ } e ->
+              ⌊ Γ ⌋* ⊢t e ⋮t ⌊ τ ⌋ /\
+                (ok_dctx (dom _ st) Γ) /\
+                cl_dctx (dom _ st) Γ /\
+                closed_rty 0 (ctxdom Γ ∪ (dom _ st)) τ.
+Proof.
+  intros. split.
+  - eapply ctxrR_regular1; eauto.
+  - eapply ctxrR_regular0; eauto.
+Qed.
+
+(* Lemma ctxrR_regular1: *)
+(*   forall Γ τ st e, { st }⟦ τ ⟧{ Γ } e -> closed_rty 0 (ctxdom Γ ∪ dom _ st) τ /\ *)
+(*                 ⌊ Γ ⌋* ⊢t e ⋮t ⌊ τ ⌋ /\ (ok_dctx (dom _ st) Γ). *)
+(* Proof. *)
+(*   induction Γ; simpl; intros; invclear H; simpl. *)
+(*   - apply rR_regular2 in H0; mydestr; split; intros; my_simplify_map_eq. *)
+(*     closed_rty_solver. *)
+(*     split; auto. constructor; auto. fast_set_solver. *)
+(*   - split; auto. closed_rty_solver. *)
+(*   - mydestr. split; auto. apply rR_regular2 in H; mydestr. closed_rty_solver. *)
+(* Qed. *)
+
+Inductive ctxrR2: bstate -> state -> listctx rty -> rty -> rty -> Prop :=
+| ctxrR2_nil: forall bst st τ1 τ2,
+    closed_rty 0 (dom _ st) τ1 -> closed_rty 0 (dom _ st) τ2 ->
+    (forall e, { st }⟦ τ1 ⟧ e -> { st }⟦ τ2 ⟧ e) ->
+    ctxrR2 bst st [] τ1 τ2
+| ctxrR2_cons_over: forall bst st (x: atom) B d ϕ Γ τ1 τ2,
+    ctxrR_wf (dom _ st) ((x, {v: B | 0 | d | ϕ}) :: Γ) τ1 ->
+    ctxrR_wf (dom _ st) ((x, {v: B | 0 | d | ϕ}) :: Γ) τ2 ->
+    (forall (c_x: constant), {st}⟦ {v: B | 0 | d | ϕ} ⟧ c_x -> ctxrR2 bst (<[ x := c_x ]> st) Γ τ1 τ2) ->
+    ctxrR2 bst st ((x, {v: B | 0 | d | ϕ}) :: Γ) τ1 τ2
+| ctxrR2_cons_under: forall bst st (x: atom) τ_x τ1 τ2 Γ,
+    ctxrR_wf (dom _ st) ((x, τ_x) :: Γ) τ1 ->
+    ctxrR_wf (dom _ st) ((x, τ_x) :: Γ) τ2 ->
+    not_overbasety τ_x ->
+    (exists e_x_hat, {st}⟦ τ_x ⟧ e_x_hat /\
+                  (forall e_x, {st}⟦ τ_x ⟧ e_x ->
+                          (∀ (v_x: value), e_x_hat ↪* v_x -> ctxrR2 bst ({ x ↦ v_x } st) Γ τ1 τ2))) ->
+    ctxrR2 bst st ((x, τ_x) :: Γ) τ1 τ2.
+
+Notation " '{' st '}⟦' τ1 '⟧⊆⟦' τ2 '⟧{' Γ '}' " := (forall bst, ctxrR2 bst st Γ τ1 τ2) (at level 20, format "{ st }⟦ τ1 ⟧⊆⟦ τ2 ⟧{ Γ }", st constr, τ1 constr, τ2 constr, Γ constr).
+Notation " '⟦' τ1 '⟧⊆⟦' τ2 '⟧{' Γ '}' " := (forall bst, ctxrR2 bst ∅ Γ τ1 τ2) (at level 20, format "⟦ τ1 ⟧⊆⟦ τ2 ⟧{ Γ }", τ1 constr, τ2 constr, Γ constr).
