new_proof/RefinementDenotationTac.v
@@ -1,0 +1,625 @@
+From stdpp Require Import mapset.
+From stdpp Require Import natmap.
+From stdpp Require Import fin_map_dom.
+From CT Require Import CoreLangProp.
+From CT Require Import OperationalSemanticsProp.
+From CT Require Import BasicTypingProp.
+From CT Require Import SyntaxSugar.
+From CT Require Import Refinement.
+From CT Require Import RefinementTac.
+From CT Require Import RefinementDenotation.
+From CT Require Import TermOrdering.
+From Coq Require Import Logic.ClassicalFacts.
+From Coq Require Import Classical.
+
+Import Atom.
+Import CoreLang.
+Import Tactics.
+Import NamelessTactics.
+Import ListCtx.
+Import OperationalSemantics.
+Import OperationalSemanticsProp.
+Import BasicTyping.
+Import SyntaxSugar.
+Import Refinement.
+Import RefinementTac.
+Import RefinementDenotation.
+Import TermOrdering.
+
+Ltac my_simplify_map_eq2 :=
+  repeat (match goal with
+          | [|- context [ <[?a:=_]> (<[?a:=_]> ?st) ]] =>
+              setoid_rewrite insert_insert
+          | [H: context [ <[?a:=_]> (<[?a:=_]> ?st) ] |- _ ] =>
+              setoid_rewrite insert_insert in H
+          | [|- context [<[?b:=?c0]> ?st !! ?b ] ] => setoid_rewrite lookup_insert
+          | [H: context [<[?b:=?c0]> ?st !! ?b ] |- _ ] => setoid_rewrite lookup_insert in H
+          | [H: ?st !! ?x = Some _ |- context [?st !! ?x]] => setoid_rewrite H
+          | [H: ?x ∈ dom _ ?st |- context [?st !! ?x]] =>
+              assert (exists c, st !! x = Some c) as Htmp by
+                (destruct (st !! x) eqn: HH; eauto;
+                 setoid_rewrite <- not_elem_of_dom in HH; set_solver); mydestr
+          | [H': ?a ∉ dom _ ?st |- context [?st !! ?a]] =>
+              assert (st !! a = None) as Htmp by (apply not_elem_of_dom; fast_set_solver);
+              rewrite Htmp; try clear Htmp
+          | [H': ?a ∉ dom _ ?st, H: context [?st !! ?a] |- _ ] =>
+              assert (st !! a = None) as Htmp by (apply not_elem_of_dom; fast_set_solver);
+              rewrite Htmp in H; try clear Htmp
+          end || my_simplify_map_eq1).
+
+Lemma refinement_exclude_const: forall b (ϕ: refinement),
+    (∀ c: constant, [] ⊢t c ⋮v b → ~ ϕ b∅ ∅ c) \/ (exists c: constant, [] ⊢t c ⋮v b /\ ϕ b∅ ∅ c).
+Proof.
+  intros.
+  destruct (classic (exists c: constant, [] ⊢t c ⋮v b /\ ϕ b∅ ∅ c)); auto.
+  - left. intros. intro Hf. apply H. exists c. split; auto.
+Qed.
+
+Lemma terr_reduction_iff_false_phi: forall bst st b (ϕ: refinement),
+    (∀ c : constant, [] ⊢t c ⋮v b → ϕ bst st c → terr ↪* c) <-> (forall c: constant, [] ⊢t c ⋮v b → ~ ϕ bst st c).
+Proof.
+  split; intros.
+  - intros Hf. apply H in Hf; auto. auto_reduction_exfalso.
+  - apply H in H0. auto_reduction_exfalso.
+Qed.
+
+Lemma terr_inhabitant_iff_false_phi: forall n1 n2 bst st (d: aset) b (ϕ: refinement),
+    {n1; bst; st}⟦ [v: b | n2 | d | ϕ ] ⟧ terr <->
+      (closed_rty n1 (dom aset st) [v:b|n2|d|ϕ] /\ forall c: constant, [] ⊢t c ⋮v b → ~ ϕ bst st c).
+Proof.
+  split; intros.
+  - invclear H. mydestr; subst. rewrite terr_reduction_iff_false_phi in H1; auto.
+  - mydestr. constructor; auto. split; auto. rewrite terr_reduction_iff_false_phi; auto.
+Qed.
+
+Lemma ctxrR_empty_iff_rR: forall st τ e, ({st}⟦τ⟧{ [] }) e <-> {st}⟦τ⟧ e.
+Proof.
+  split; intros; auto.
+  - invclear H; auto.
+  - constructor; auto.
+Qed.
+
+Lemma not_ctxrR_empty_iff_not_rR: forall st τ e, ~ ({st}⟦τ⟧{ [] }) e <-> ~ {st}⟦τ⟧ e.
+Proof.
+  split; intros; auto.
+  - intros HF. apply H. constructor; auto.
+  - intros HF. apply H. invclear HF; auto.
+Qed.
+
+Definition base_type_max_term (b: base_ty) :=
+  match b with
+  | TNat => nat-gen
+  | TBool => bool-gen
+  end.
+
+Ltac denotation_simp0 :=
+  my_simplify_map_eq2;
+  repeat match goal with
+    | [H: forall bst, ({0;bst; _ }⟦ _ ⟧) _ |- _ ] => specialize (H b∅); invclear H; mydestr
+    | [H: _ ⊢t (tvalue ?v) ⋮t _ |- _ ] => invclear H
+    | [H: _ ⊢t _ ⋮t ⌊ _ ⌋ |- _ ] => progress simpl in H
+    | [H: _ ⊢t _ ⋮v ⌊ _ ⌋ |- _ ] => progress simpl in H
+    | [H: ({_}⟦?τ⟧{_}) _  |- closed_rty _ _ ?τ] => apply ctxrR_regular in H; mydestr
+    | [H: ({_}⟦_⟧{?Γ}) _  |- ok_dctx _ ?Γ] => apply ctxrR_regular in H; mydestr; my_simplify_map_eq
+    | [H: _ ⊢t ?v ⋮v (TBase _) |- _ ] =>
+        match v with
+        | vconst _ => fail 1
+        | _ => set H as Htmp; apply empty_basic_typing_base_const_exists in Htmp; mydestr; subst
+        end
+    | [H: ∀ c, [] ⊢t (vconst c) ⋮v _ → _ _ ∅ c → terr ↪* (tvalue (vconst c)) |- _ ] =>
+        rewrite terr_reduction_iff_false_phi in H
+    end.
+
+Lemma base_type_max_term_typable: forall b, [] ⊢t base_type_max_term b ⋮t b.
+Proof.
+  destruct b; simpl; eauto.
+Qed.
+
+Global Hint Resolve base_type_max_term_typable: core.
+
+Lemma base_type_max_term_spec: forall (b: base_ty) (c: constant), [] ⊢t c ⋮v b -> base_type_max_term b ↪* c.
+Proof.
+  destruct b; simpl; intros; eauto; destruct c; invclear H; subst; eauto.
+Qed.
+
+Global Hint Resolve base_type_max_term_spec: core.
+
+Lemma base_type_reduce_to_constant: forall e (b: base_ty) (v: value), [] ⊢t e ⋮t b -> e ↪* v -> (∃ c, v = vconst c).
+Proof.
+  intros.
+  eapply multi_preservation in H; eauto. denotation_simp0. eapply empty_basic_typing_base_const_exists; eauto.
+Qed.
+
+Lemma base_type_max_term_reduce_to_constant: forall b (v: value), base_type_max_term b ↪* v -> (∃ c, v = vconst c).
+Proof.
+  intros. assert ([] ⊢t base_type_max_term b ⋮t b); eauto.
+  eapply multi_preservation in H; eauto. denotation_simp0. eapply empty_basic_typing_base_const_exists; eauto.
+Qed.
+
+Global Hint Resolve base_type_max_term_reduce_to_constant: core.
+
+Ltac denotation_simp1 :=
+  repeat (denotation_simp0;
+   mydestr;
+   repeat match goal with
+   | [H: ¬ is_arr _ |- _ ] => apply not_is_arr in H; destruct H; mydestr; subst
+   | [H: ¬ not_underbasety _ |- _ ] => apply not_not_underbasety in H; mydestr; subst
+   | [H: ¬ ({_}⟦ _ ⟧{ [] }) _ |- _ ] => rewrite not_ctxrR_empty_iff_not_rR in H
+   | [ |- ¬ ({_}⟦ _ ⟧{ [] }) _ ] => rewrite not_ctxrR_empty_iff_not_rR
+   (* | [H: {_}⟦ _ ⟧{ [] } _ |- _ ] => invclear H *)
+   | [H: closed_rty 0 _ [v:_|?n|_|_] |- _ ] =>
+       match n with
+       | 0 => fail 1
+       | _ => assert (n = 0) by (apply closed_rty_0_underbase in H; auto); subst
+       end
+   | [H: closed_rty 0 _ {v:_|?n|_|_} |- _ ] =>
+       match n with
+       | 0 => fail 1
+       | _ => assert (n = 0) by (apply closed_rty_0_overbase in H; auto); subst
+       end
+   | [H: ?e ↪* (tvalue ?v), H': [] ⊢t ?e ⋮t (TBase _)  |- _ ] =>
+       match v with
+       | vconst _ => fail 1
+       | _ => assert (exists c, v = vconst c) as Htmp by (eapply base_type_reduce_to_constant in H; eauto);
+             destruct Htmp; subst
+       end
+   | [H: base_type_max_term _ ↪* (tvalue ?v) |- _ ] =>
+       match v with
+       | vconst _ => fail 1
+       | _ => assert (exists c, v = vconst c) as Htmp by (eapply base_type_max_term_reduce_to_constant in H; eauto);
+             destruct Htmp; subst
+       end
+   end).
+
+Ltac denotation_simp := denotation_simp1.
+
+
+Lemma valid_rty_under_iff_over: forall n b (d2: aset) (ϕ: refinement),
+    valid_rty {v:b|n|d2|ϕ} <-> valid_rty [v:b|n|d2|ϕ].
+Proof.
+  split; intros; invclear H; constructor; auto.
+Qed.
+
+Lemma closed_rty_under_iff_over: forall n1 n2 b (d1 d2: aset) (ϕ: refinement),
+    closed_rty n1 d1 {v:b|n2|d2|ϕ} <-> closed_rty n1 d1 [v:b|n2|d2|ϕ].
+Proof.
+  split; unfold closed_rty; intros.
+  - invclear H; mydestr. constructor; auto.
+    rewrite <- valid_rty_under_iff_over; auto.
+    constructor; auto. invclear H. constructor; auto.
+  - invclear H; mydestr. constructor; auto.
+    rewrite valid_rty_under_iff_over; auto.
+    constructor; auto. invclear H. constructor; auto.
+Qed.
+
+Lemma crxrR_perservation: forall st r e e', ({st}⟦r⟧) e -> e ↪* e' -> [] ⊢t e' ⋮t ⌊r⌋.
+Proof.
+  intros. apply rR_regular1 in H; mydestr. eapply multi_preservation in H0; eauto.
+Qed.
+
+Ltac refinement_solver0 :=
+  repeat (match goal with
+          | [H: {_;_;_}⟦_⟧ ?e |- lc ?e] => apply rR_regular1 in H; mydestr; basic_typing_solver2
+          | [H: ({0;b∅;_}⟦?r⟧) ?x, H': ?x ↪* ?y |- [] ⊢t ?y ⋮t ⌊?r⌋ ] =>
+              apply (crxrR_perservation _ r x y) in H; auto
+          | [H: ({0;b∅;_}⟦?r⟧) ?x, H': ?x ↪* (tvalue ?y) |- [] ⊢t ?y ⋮v ⌊?r⌋ ] =>
+              (apply (crxrR_perservation _ r x y) in H; auto); (invclear H; auto)
+          | [H: closed_rty _ _ _ |- bound_in_refinement _ _ ] => destruct H; mydestr
+          | [H: valid_rty _ |- bound_in_refinement _ _ ] => invclear H
+          | [H: valid_rty ?τ |- wf_r _ _ ?ϕ ] =>
+              match τ with
+              | context [ ϕ ] => invclear H; eauto
+              end
+          | [H: closed_rty _ _ ?τ |- wf_r _ _ ?ϕ ] =>
+              match τ with
+              | context [ ϕ ] => invclear H; mydestr; eauto
+              end
+          | [H: wf_r _ _ ?ϕ |- bound_in_refinement _ ?ϕ ] => destruct H
+          | [H: ({_;_;_}⟦?τ⟧) _ |- closed_rty _ _ ?τ ] =>
+              apply rR_regular1 in H; mydestr; eauto; try closed_rty_solver
+          | [H: ({_;_;_}⟦?τ⟧) _ |- _ ⊢t _ ⋮t _ ] =>
+              apply rR_regular1 in H; mydestr; eauto; try basic_typing_solver
+          | [ |- closed_rty _ _ _ ] => closed_rty_solver
+          | [H: ok_dctx _ _ |- ok _ ] => ok_dctx_solver
+          | [ |- ok ((_, _) :: _)] => rewrite ok_pre_destruct; split; ctx_erase_simp
+          | [H: closed_rty _ _ ?τ |- _ ∉ rty_fv ?τ ] => invclear H; mydestr; try fast_set_solver
+          | [H: closed_rty _ _ (-:{v: _ | _ | _ | _}⤑ ?τ) |- ?ret ] =>
+               match ret with
+               | not_overbasety ?τ => invclear H; mydestr; auto
+               | valid_rty ?τ => invclear H; mydestr; auto
+               end
+           | [H: valid_rty (-:{v: _ | _ | _ | _}⤑ ?τ) |- ?ret ] =>
+               match ret with
+               | not_overbasety ?τ => invclear H; auto
+               | valid_rty ?τ => invclear H; auto
+               end
+           | [H: closed_rty _ _ (?τ1 ⤑ ?τ2) |- ?ret ] =>
+               match ret with
+               | not_overbasety ?τ1 => invclear H; mydestr; auto
+               | valid_rty ?τ1 => invclear H; mydestr; auto
+               | not_overbasety ?τ2 => invclear H; mydestr; auto
+               | valid_rty ?τ2 => invclear H; mydestr; auto
+               end
+           | [H: valid_rty (?τ1 ⤑ ?τ2) |- ?ret ] =>
+               match ret with
+               | not_overbasety ?τ1 => invclear H; auto
+               | valid_rty ?τ1 => invclear H; auto
+               | not_overbasety ?τ2 => invclear H; auto
+               | valid_rty ?τ2 => invclear H; auto
+               end
+          end || refinement_simp1 || eauto || listctx_set_solver || fast_set_solver).
+
+Ltac refinement_solver2 :=
+  repeat (
+      try auto_reduction_exfalso;
+      match goal with
+      | [H: {?st}⟦ ?τ ⟧{ [] } ?e |- {?st}⟦ ?τ ⟧ ?e ] => invclear H
+      | [H: closed_rty _ _ ?τ |- valid_rty ?τ] => destruct H; auto
+      | [ |- _ ⊢t terr ⋮t _ ] => constructor; auto
+      | [H: ok_dctx ?d ((_, ?τ) :: _) |- closed_rty 0 ?d ?τ ] => invclear H; auto
+      | [H: ok_dctx _ _ |- ok _ ] => apply ok_dctx_regular1 in H; mydestr
+      | [H: ok (_ :: ?Γ) |- ok ⌊?Γ⌋* ] => rewrite ok_pre_destruct in H; mydestr; ctx_erase_simp
+      | [ |- context [ ⌊ _ ⌋* ] ] => ctx_erase_simp; fast_set_solver
+      | [H: ?e ↪* (tvalue ?v), H': [] ⊢t ?e ⋮t ?T |- [] ⊢t ?v ⋮v ?T ] =>
+          eapply multi_preservation_value in H'; eauto
+      | [H: [] ⊢t ?e ⋮t ?T |- _ ⊢t ?e ⋮t _ ] => apply basic_typing_weaken_tm_empty; eauto
+      | [H: lc_rty_idx _ _ |- lc_rty_idx _ _ ] => invclear H; auto
+      end || refinement_solver0).
+
+Ltac refinement_solver := refinement_solver2.
+
+
+Lemma refinement_shadow_update_st: forall bst c n ϕ (x: atom) d st (v: constant),
+    x ∉ d -> wf_r n d ϕ -> ϕ bst (<[x:=c]> st) v <-> ϕ bst st v.
+Proof.
+  intros.
+  destruct H0. apply H0; auto.
+Qed.
+
+Ltac rR_shadow_update_st_tac :=
+  repeat match goal with
+    | [H: valid_rty {v: _ |_ |?d|?ϕ} |- ?ϕ _ (<[_:=_]> _) _ ] =>
+        rewrite refinement_shadow_update_st with (d:=d); auto; refinement_solver
+    | [H: valid_rty [v: _ |_ |?d|?ϕ] |- ?ϕ _ (<[_:=_]> _) _ ] =>
+        rewrite refinement_shadow_update_st with (d:=d); auto; refinement_solver
+    | [H: valid_rty {v: _ |_ |?d|?ϕ}, H': ?ϕ _ (<[_:=_]> _) _ |- ?ϕ _ _ _ ] =>
+        rewrite refinement_shadow_update_st with (d:=d) in H'; auto; refinement_solver
+    | [H: valid_rty [v: _ |_ |?d|?ϕ], H': ?ϕ _ (<[_:=_]> _) _ |- ?ϕ _ _ _ ] =>
+        rewrite refinement_shadow_update_st with (d:=d) in H'; auto; refinement_solver
+    | [H: closed_rty _ _ ?τ, H': ?ϕ ?bst _ ?c_x |- ?ϕ ?bst _ ?c_x] =>
+        match τ with
+        | context [ϕ] => destruct H; mydestr
+        end
+    end.
+
+Lemma rR_shadow_update_st: forall τ n st,
+    closed_rty n (dom aset st) τ ->
+    (forall bst (a: atom) c e, a ∉ (rty_fv τ) ->
+                      ({n; bst; <[a:=c]> st}⟦τ⟧) e <-> ({n; bst; st}⟦τ⟧) e
+    ).
+Proof.
+  induction τ; split; simpl; intros; mydestr; subst;
+    split; auto; split; try closed_rty_solver.
+  - exists x. repeat split; auto. rR_shadow_update_st_tac.
+  - exists x. repeat split; auto. rR_shadow_update_st_tac.
+  - intros. apply H3; auto. rR_shadow_update_st_tac.
+  - intros. apply H3; auto. rR_shadow_update_st_tac.
+  - intros. refinement_simp1. apply H3 in H4. apply IHτ in H4; refinement_solver.
+    rewrite refinement_shadow_update_st with (d:=d); auto; refinement_solver.
+  - intros. refinement_simp1. apply H3 in H4. apply IHτ; refinement_solver.
+    rewrite <- refinement_shadow_update_st with (d:=d); auto; refinement_solver.
+  - intros. refinement_simp1.
+    rewrite <- IHτ1 with (a:= a) (c:=c) in H4; auto; refinement_solver.
+    apply H3 in H4. rewrite IHτ2 in H4; by refinement_solver.
+  - intros. refinement_simp1.
+    rewrite IHτ1 in H4 by refinement_solver.
+    apply H3 in H4; rewrite IHτ2; auto; refinement_solver.
+Qed.
+
+Lemma lc_rR_shadow_update_st: forall τ st (a: atom) c e,
+    closed_rty 0 (dom aset st) τ -> a ∉ (rty_fv τ) ->
+    ({<[a:=c]> st}⟦τ⟧) e <-> ({st}⟦τ⟧) e.
+Proof.
+  split; intros.
+  - rewrite rR_shadow_update_st in H1; eauto.
+  - rewrite rR_shadow_update_st; eauto.
+Qed.
+
+Lemma subst_insert_lookup_neq_Some {A:Type}: forall (a b: atom) (c0 c1: A) (st: amap A),
+    a <> b -> st !! a = Some c1 -> <[b:=c0]> st !! a = Some c1.
+Proof.
+  intros. setoid_rewrite lookup_insert_Some; auto.
+Qed.
+
+Lemma subst_insert_lookup_neq_None {A:Type}: forall (a b: atom) (c0: A) (st: amap A),
+    a <> b -> st !! a = None -> <[b:=c0]> st !! a = None.
+Proof.
+  intros. setoid_rewrite lookup_insert_None; auto.
+Qed.
+
+Ltac amap_solver1 Hsta :=
+  repeat match goal with
+  | [|- <[?a:=_]> (<[?b:=_]> ?st) = <[?b:=_]> (<[?a:=_]> ?st)] =>
+      setoid_rewrite (insert_commute st a b); auto; try fast_set_solver
+  | [H: ?st !! ?a = None |- context [<[?b:=?c0]> ?st !! ?a ] ] =>
+      setoid_rewrite (subst_insert_lookup_neq_None a b c0); auto; try fast_set_solver
+  | [H: ?st !! ?a = Some ?c1 |- context [<[?b:=?c0]> ?st !! ?a ] ] =>
+      setoid_rewrite (subst_insert_lookup_neq_Some a b c0 c1); auto; try fast_set_solver
+  | [|- context [<[?b:=?c0]> ?st !! ?a ] ] =>
+      destruct (st !! a) eqn: Hsta
+  end.
+
+Lemma subst_st_insert_commute:forall (v_x: value) (a b: atom) (c: constant) st,
+    fv_value v_x ∩ {[a; b]} = ∅ ->
+    a <> b -> ({a↦v_x}) (<[b:=c]> st) = (<[b:=c]>) ({a↦v_x} st).
+Proof.
+  destruct v_x; intros; simpl; auto.
+  - amap_solver1 Hsta.
+  - simpl. my_simplify_map_eq.
+    amap_solver1 Hsta1. amap_solver1 Hsta2. set_solver. set_solver.
+Qed.
+
+Lemma insert_constant_in_st: forall (v_x: constant) (a: atom) (st: state),
+    a ∉ (dom aset st) -> (dom aset (({a↦v_x}) st)) ≡ ({[a]} ∪ dom aset st).
+Proof.
+  intros; simpl; auto. my_simplify_map_eq2.
+Qed.
+
+Lemma insert_vfvar_in_st: forall (v_x: atom) (a: atom) (st: state),
+    v_x ∈ dom aset st -> a ∉ (dom aset st) ->
+    (dom aset (({a↦v_x}) st)) ≡ ({[a]} ∪ dom aset st).
+Proof.
+  intros; simpl; auto.
+  - simpl in H. my_simplify_map_eq2.
+Qed.
+
+Ltac ok_dctx_solver_slow :=
+  match goal with
+  | [H1: ok_dctx ?d1 ?τ, H2: ok_dctx ?d2 ?τ |- ok_dctx ?d3 ?τ ] =>
+      apply (ok_dctx_cap τ d1 d2 d3); auto; simpl; refinement_set_simp; set_solver
+  | [H: ok_dctx ?d1 ?τ |- ok_dctx ?d2 ?τ ] =>
+      apply (ok_dctx_trans τ d1 d2); simpl; auto; refinement_set_simp; set_solver
+  end.
+
+Ltac ctxrR_shadow_update_st_tac :=
+  match goal with
+  | [H: context [{0;b∅;<[?a0:=?c]> ?st}⟦?τ⟧ _],
+        H': ({0;b∅;?st}⟦?τ⟧) _ |- ?ret ] =>
+      (* idtac H' *)
+      (rewrite <- lc_rR_shadow_update_st with (a:=a0) (c:=c) in H'
+       ;eauto; refinement_solver);
+      match ret with
+      | context [({_↦?v_x}) _] => eapply H with (v_x := v_x) in H'; eauto
+      | _ => apply H in H'
+      end
+  end.
+
+Ltac auto_ty_exfalso :=
+  match goal with
+  | [H: [] ⊢t (vfvar _) ⋮v _ |- _ ] => invclear H; listctx_set_simpl
+  | [H: [] ⊢t (vbvar _) ⋮v _ |- _ ] => invclear H
+  | [H: is_arr {v:_|_|_|_} |- _ ] => invclear H
+  | [H: is_arr [v:_|_|_|_] |- _ ] => invclear H
+  | [H: ¬ is_arr ?r, H': [] ⊢t vlam _ _ ⋮v ⌊?r⌋ |- _ ] => (destruct r; invclear H'; exfalso; auto)
+  | [H: ¬ is_arr ?r, H': [] ⊢t vfix _ _ ⋮v ⌊?r⌋ |- _ ] => (destruct r; invclear H'; exfalso; auto)
+  | [H: is_arr ?r, H': [] ⊢t (vconst _) ⋮v ⌊?r⌋ |- _ ] => (destruct r; invclear H'; invclear H)
+  | [H: not_overbasety {v: _ |_|_|_} |- _ ] => invclear H
+  end.
+
+Lemma ctxrR_shadow_update_st: forall Γ st τ,
+    closed_rty 0 (ctxdom Γ ∪ dom aset st) τ ->
+    ok_dctx (dom aset st) Γ ->
+    (forall (a: atom) c e, a ∉ (ctxdom Γ ∪ dom aset st) ->
+                        ({<[a:=c]> st}⟦τ⟧{Γ}) e <-> ({st}⟦τ⟧{Γ}) e
+    ).
+Proof.
+  induction Γ; split; simpl; intros; mydestr; subst.
+  - invclear H2. constructor; auto; intros.
+    rewrite <- rR_shadow_update_st; eauto; refinement_solver.
+  - invclear H2. constructor; auto; intros.
+    rewrite rR_shadow_update_st; eauto; refinement_solver.
+  - invclear H0; invclear H2; mydestr; try auto_ty_exfalso.
+    + constructor; auto. constructor; auto.
+      intros.
+      ctxrR_shadow_update_st_tac.
+      setoid_rewrite insert_commute in H0; try fast_set_solver.
+      rewrite IHΓ in H0; auto; denotation_simp.
+      refinement_solver.
+    + constructor; auto. constructor; auto.
+      exists x. split. intros. rewrite <- rR_shadow_update_st; eauto. refinement_solver.
+      intros; mydestr.
+      ctxrR_shadow_update_st_tac.
+      assert ([] ⊢t v_x ⋮v ⌊r⌋) by refinement_solver.
+      simpl in H1. destruct v_x; try auto_ty_exfalso.
+      { rewrite subst_st_insert_commute in H3; try fast_set_solver.
+        rewrite IHΓ in H3; auto; denotation_simp.
+        refinement_solver. }
+      (* { denotation_simp; rewrite IHΓ in H3; auto; denotation_simp. refinement_solver. ok_dctx_solver_slow. } *)
+      (* { denotation_simp; rewrite IHΓ in H3; auto; denotation_simp. refinement_solver. ok_dctx_solver_slow. } *)
+    + constructor; auto. apply ok_dctx_cons_arr; auto.
+      exists x. split. intros. rewrite <- rR_shadow_update_st; eauto. refinement_solver.
+      intros; mydestr.
+      ctxrR_shadow_update_st_tac.
+      assert ([] ⊢t v_x ⋮v ⌊r⌋) by refinement_solver.
+      simpl in H1. destruct v_x; try auto_ty_exfalso;
+        denotation_simp; rewrite IHΓ in H3; auto; denotation_simp; refinement_solver.
+   - invclear H0; invclear H2; mydestr; try auto_ty_exfalso.
+    + constructor; auto; denotation_simp. refinement_solver. ok_dctx_solver_slow.
+      intros. specialize (H16 c_x).
+      assert ({0;b∅; st}⟦{v:B|0|d|ϕ}⟧ c_x) by
+      (rewrite <- lc_rR_shadow_update_st with (a:=a0) (c:=c); eauto; refinement_solver).
+      apply H16 in H2.
+      setoid_rewrite insert_commute; refinement_solver.
+      rewrite IHΓ; auto; denotation_simp; refinement_solver.
+    + invclear H7; mydestr.
+      constructor; auto. refinement_solver. ok_dctx_solver_slow.
+      exists x. split. rewrite rR_shadow_update_st; eauto; refinement_solver.
+      intros; mydestr.
+      rewrite lc_rR_shadow_update_st in H12; auto; try refinement_solver.
+      eapply H2 with (v_x := v_x) in H12; eauto.
+      assert ([] ⊢t v_x ⋮v ⌊r⌋) by refinement_solver.
+      simpl in H1. destruct v_x; try auto_ty_exfalso.
+      { rewrite subst_st_insert_commute; denotation_simp.
+        rewrite IHΓ; auto; denotation_simp; refinement_solver. }
+    + invclear H7; mydestr.
+      constructor; auto. refinement_solver. ok_dctx_solver_slow.
+      exists x. split. intros. rewrite rR_shadow_update_st; eauto; refinement_solver.
+      intros; mydestr.
+      rewrite lc_rR_shadow_update_st in H12; auto; try refinement_solver.
+      eapply H2 with (v_x := v_x) in H12; eauto.
+      assert ([] ⊢t v_x ⋮v ⌊r⌋) by refinement_solver.
+      simpl in H1. destruct v_x; try auto_ty_exfalso;
+        denotation_simp; rewrite IHΓ; auto; denotation_simp; refinement_solver.
+Qed.
+
+(* Lemma denotation_lc_lete: forall Γ (e_x e: tm) τ (st: state), *)
+(*   {st}⟦τ⟧{Γ} e_x -> {st}⟦τ⟧{Γ} e -> ({st}⟦τ⟧{Γ}) (tlete e_x e). *)
+(* Proof. *)
+(*   induction Γ; intros; denotation_simp; invclear H; invclear H0. *)
+(*   - constructor. admit. *)
+(*   - constructor; auto. admit. *)
+(*     intros. apply IHΓ; auto. admit. simpl. apply IHΓ; auto. *)
+(*     + apply IHΓ; auto. admit. simpl. *)
+
+
+(*       rewrite ctxrR_shadow_update_st; auto. *)
+(*       apply H. *)
+(*     apply H16 in H. apply IHΓ. *)
+(*     + rewrite ctxrR_shadow_update_st; auto. *)
+(*     simpl. *)
+
+Lemma termR_perserve_rR: forall τ (e e': tm),
+    not_overbasety τ ->
+    valid_rty τ ->
+    e <-<{[]; ⌊ τ ⌋ } e' -> (forall n bst st, {n;bst;st}⟦τ⟧ e -> {n;bst;st}⟦τ⟧ e').
+Proof.
+  induction τ; simpl; intros; invclear H0; mydestr; subst.
+  - invclear H.
+  - repeat (split; try termR_solver).
+  - repeat (split; try termR_solver).
+    intros. apply IHτ with (e := (mk_app e c_x)); eauto; termR_solver.
+  - repeat (split; try termR_solver).
+    intros. apply IHτ2 with (e := (mk_app e e_x)); eauto. termR_solver; refinement_solver.
+  - repeat (split; try termR_solver).
+    intros. apply IHτ2 with (e := (mk_app e e_x)); eauto. termR_solver; refinement_solver.
+Qed.
+
+Lemma termR_perserve_ctxrR: forall Γ τ (e e': tm),
+    not_overbasety τ ->
+    valid_rty τ ->
+    e <-<{ ⌊ Γ ⌋* ;  ⌊ τ ⌋ } e' -> (forall st, {st}⟦τ⟧{Γ} e -> {st}⟦τ⟧{Γ} e').
+Proof.
+  induction Γ; intros; invclear H2.
+  - constructor. intros. eapply termR_perserve_rR; eauto.
+  - constructor; auto. termR_solver.
+    intros. apply IHΓ with (e:= (tlete c_x (x \t\ e))); eauto.
+    apply termR_elete with (Tx := B); auto. constructor; auto; refinement_solver; basic_typing_solver2.
+    simpl in H1. termR_solver.
+  - constructor; auto. termR_solver.
+    destruct H12 as (e_x_hat & He_x_hat & HH). exists e_x_hat. split; auto.
+    intros. apply IHΓ with (e:= (tlete e_x (x \t\ e))); eauto.
+    apply termR_elete with (Tx := ⌊ τ_x ⌋ ); auto. constructor; auto; refinement_solver.
+    simpl in H1. termR_solver.
+Qed.
+
+(* terr *)
+
+Lemma terr_is_not_inhabitant_of_overbase: forall τ n bst st,
+    {n; bst; st}⟦τ⟧ terr -> not_overbasety τ.
+Proof.
+  destruct τ; intros; invclear H; mydestr; simpl; auto.
+  invclear H3.
+Qed.
+
+Lemma ctxrR_err_overbase_forall_forward: forall Γ st τ x b n d ϕ,
+    ¬ ({st}⟦τ⟧{(x, {v:b|n|d|ϕ}) :: Γ}) terr ->
+    ok_dctx (dom aset st) ((x, {v:b|n|d|ϕ}) :: Γ) ->
+    closed_rty 0 ({[x]} ∪ ctxdom Γ ∪ dom aset st) τ ->
+    not_overbasety τ ->
+    (exists (c: constant), {st}⟦{v:b|n|d|ϕ}⟧ c /\ ¬ ({<[x:=c]> st}⟦τ⟧{Γ}) terr).
+Proof.
+  intros. pbc. apply H. clear H. neg_simpl.
+  constructor; auto; refinement_solver2.
+  intros.
+  assert (({<[x:=c_x]> st}⟦τ⟧{Γ}) terr); auto.
+  apply termR_perserve_ctxrR with (e:= terr); auto; refinement_solver2.
+  apply tyable_implies_terr_termR.
+  econstructor; eauto; refinement_solver2; mydestr.
+  apply basic_typing_weaken_value_empty; eauto. refinement_solver2.
+  auto_exists_L_intros. do 2 constructor; refinement_solver2.
+Qed.
+
+Lemma ctxrR_err_overbase_forall_backward: forall Γ st τ x b n d ϕ,
+    ok_dctx (dom aset st) ((x, {v:b|n|d|ϕ}) :: Γ) ->
+    closed_rty 0 ({[x]} ∪ ctxdom Γ ∪ dom aset st) τ ->
+    not_overbasety τ ->
+    (exists (c: constant), {st}⟦{v:b|n|d|ϕ}⟧ c /\ ¬ ({<[x:=c]> st}⟦τ⟧{Γ}) terr) ->
+    ¬ ({st}⟦τ⟧{(x, {v:b|n|d|ϕ}) :: Γ}) terr.
+Proof.
+  intros. mydestr. intro Hf. apply H3. clear H3.
+  invclear Hf; try invclear H6.
+  apply termR_perserve_ctxrR with (e:= (tlete x0 (x \t\ terr))); auto; refinement_solver2.
+  eapply tyable_implies_terr_termR_terr; refinement_solver2.
+  apply basic_typing_weaken_value_empty; eauto. refinement_solver2.
+Qed.
+
+Lemma ctxrR_err_overbase_forall: forall Γ st τ x b n d ϕ,
+    ok_dctx (dom aset st) ((x, {v:b|n|d|ϕ}) :: Γ) ->
+    closed_rty 0 ({[x]} ∪ ctxdom Γ ∪ dom aset st) τ ->
+    not_overbasety τ ->
+    ¬ ({st}⟦τ⟧{(x, {v:b|n|d|ϕ}) :: Γ}) terr <->
+    (exists (c: constant), {st}⟦{v:b|n|d|ϕ}⟧ c /\ ¬ ({<[x:=c]> st}⟦τ⟧{Γ}) terr).
+Proof.
+  split; intros.
+  - eapply ctxrR_err_overbase_forall_forward; eauto.
+  - eapply ctxrR_err_overbase_forall_backward; eauto.
+Qed.
+
+Lemma ctxrR_err_underbase_forall_forward: forall Γ st τ x b n d ϕ,
+    ¬ ({st}⟦τ⟧{(x, [v:b|n|d|ϕ]) :: Γ}) terr ->
+    ok_dctx (dom aset st) ((x, [v:b|n|d|ϕ]) :: Γ) ->
+    closed_rty 0 ({[x]} ∪ ctxdom Γ ∪ dom aset st) τ ->
+    not_overbasety τ ->
+    (forall e_x_hat, {st}⟦[v:b|n|d|ϕ]⟧ e_x_hat ->
+                (exists (c: constant), [] ⊢t c ⋮v b /\ e_x_hat ↪* c /\ ¬ ({<[x:=c]> st}⟦τ⟧{Γ}) terr)
+    ).
+Proof.
+  intros. pbc. apply H. clear H. neg_simpl.
+  constructor; auto; refinement_solver2.
+  exists (e_x_hat). split; auto. intros. denotation_simp1.
+  apply termR_perserve_ctxrR with (e:= terr); auto; refinement_solver2.
+  - apply tyable_implies_terr_termR. econstructor; eauto; refinement_solver2; mydestr.
+    auto_exists_L_intros. do 2 constructor; refinement_solver2.
+  - invclear H0; denotation_simp; apply H4; auto; refinement_solver2.
+Qed.
+
+Lemma ctxrR_err_underbase_forall_backward: forall Γ st τ x b n d ϕ,
+    ok_dctx (dom aset st) ((x, [v:b|n|d|ϕ]) :: Γ) ->
+    closed_rty 0 ({[x]} ∪ ctxdom Γ ∪ dom aset st) τ ->
+    not_overbasety τ ->
+    (forall e_x_hat, {st}⟦[v:b|n|d|ϕ]⟧ e_x_hat ->
+                (exists (c: constant), [] ⊢t c ⋮v b /\ e_x_hat ↪* c /\ ¬ ({<[x:=c]> st}⟦τ⟧{Γ}) terr)
+    ) ->
+    ¬ ({st}⟦τ⟧{(x, [v:b|n|d|ϕ]) :: Γ}) terr.
+Proof.
+  intros. intro Hf. invclear Hf; mydestr.
+  assert ([] ⊢t x0 ⋮t b) by refinement_solver2.
+  assert (∃ c : constant, [] ⊢t c ⋮v b ∧ x0 ↪* c ∧ ¬ ({<[x:=c]> st}⟦τ⟧{Γ}) terr); auto.
+  mydestr. apply H11. clear H11. eapply H4 in H3; eauto.
+  apply termR_perserve_ctxrR with (e:= (tlete x0 (x \t\ terr))); auto; refinement_solver2; simpl.
+  eapply tyable_implies_terr_termR_terr; refinement_solver2.
+Qed.
+
+Lemma ctxrR_err_underbase_forall: forall Γ st τ x b n d ϕ,
+    ok_dctx (dom aset st) ((x, [v:b|n|d|ϕ]) :: Γ) ->
+    closed_rty 0 ({[x]} ∪ ctxdom Γ ∪ dom aset st) τ ->
+    not_overbasety τ ->
+    ¬ ({st}⟦τ⟧{(x, [v:b|n|d|ϕ]) :: Γ}) terr <->
+    (forall e_x_hat, {st}⟦[v:b|n|d|ϕ]⟧ e_x_hat ->
+                (exists (c: constant), [] ⊢t c ⋮v b /\ e_x_hat ↪* c /\ ¬ ({<[x:=c]> st}⟦τ⟧{Γ}) terr)
+    ).
+Proof.
+  split; intros.
+  - eapply ctxrR_err_underbase_forall_forward; eauto.
+  - eapply ctxrR_err_underbase_forall_backward; eauto.
+Qed.
