new_proof/RefinementTac.v
@@ -1,0 +1,363 @@
+From stdpp Require Import mapset.
+From stdpp Require Import natmap.
+From CT Require Import CoreLangProp.
+From CT Require Import OperationalSemanticsProp.
+From CT Require Import BasicTypingProp.
+From CT Require Import SyntaxSugar.
+From CT Require Import Refinement.
+From Coq Require Import Logic.ClassicalFacts.
+From Coq Require Import Classical.
+
+Import Atom.
+Import CoreLang.
+Import Tactics.
+Import NamelessTactics.
+Import ListCtx.
+Import OperationalSemantics.
+Import OperationalSemanticsProp.
+Import BasicTyping.
+Import SyntaxSugar.
+Import Refinement.
+
+Lemma dom_insert_simp: forall (a: atom) (c_x: constant) (st: state),
+    (dom aset (<[a:=c_x]> st)) = {[a]} ∪ dom aset st.
+Proof.
+  intros. my_set_solver.
+Qed.
+
+Ltac my_simplify_map_eq1 :=
+  repeat (
+      match goal with
+      | [|- Some ?x = Some ?y] => assert (x = y); auto
+      | [|- (?a = ?b) <-> (?a = ?c)] => assert (b = c) as Htmp; try rewrite Htmp; auto
+      | [|- (?a = ?b) = (?a = ?c)] => assert (b = c) as Htmp; try rewrite Htmp; auto
+      | [|- <[_:=_]> ?m !! ?x = ?m !! ?x] => setoid_rewrite lookup_insert_ne; simplify_map_eq; auto
+      | [|- <[_:=_]> ?m !! ?x = Some _ ] => setoid_rewrite lookup_insert_ne; simplify_map_eq; auto
+      | [|- Some _ = <[_:=_]> ?m !! ?x ] => setoid_rewrite lookup_insert_ne; simplify_map_eq; auto
+      | [H: <[_:=_]> ?m !! ?x = Some _ |- ?m !! ?x = Some _] => setoid_rewrite lookup_insert_ne in H; auto; fast_set_solver
+      | [H: Some _ = <[_:=_]> ?m !! ?x |- Some _ = ?m !! ?x ] => setoid_rewrite lookup_insert_ne in H; auto; fast_set_solver
+      | [H: context [ dom aset (<[?a:=?c_x]> ?st) ] |- _ ] =>
+          setoid_rewrite (dom_insert_simp a c_x st) in H
+      | [ |- context [ dom aset (<[?a:=?c_x]> ?st) ]] =>
+          setoid_rewrite (dom_insert_simp a c_x st)
+      end || simplify_map_eq || fast_set_solver).
+
+(* Ltac my_simplify_map_eq2 := *)
+(*   repeat ( *)
+(*       match goal with *)
+(*       | [H: context [dom aset (<[?a:=?c]> ?st)] |- _ ] => *)
+(*           assert (dom aset (<[a:=c]> st) = {[a]} ∪ dom aset st) as Htmp by my_simplify_map_eq1; *)
+(*           rewrite Htmp in H; try clear Htmp *)
+(*       end || simplify_map_eq1). *)
+
+Ltac my_simplify_map_eq := my_simplify_map_eq1.
+
+Lemma closed_rty_trans: forall n d1 d2 τ, d1 ⊆ d2 -> closed_rty n d1 τ -> closed_rty n d2 τ.
+Proof.
+  intros. destruct H0; mydestr.
+  repeat split; auto. fast_set_solver.
+Qed.
+
+Lemma lc_rty_idx_under_0_is_0: forall b n d ϕ, lc_rty_idx 0 [v:b|n|d|ϕ] -> n = 0.
+Proof.
+  intros. invclear H. lia.
+Qed.
+
+Lemma lc_rty_idx_over_0_is_0: forall b n d ϕ, lc_rty_idx 0 {v:b|n|d|ϕ} -> n = 0.
+Proof.
+  intros. invclear H. lia.
+Qed.
+
+Lemma forall_iff_not_exists1 {A: Type}: forall P: A -> Prop, ~ (exists x, P x) <-> forall x, ~ P x.
+Proof.
+  split; intros.
+  - destruct (classic (P x)); auto. exfalso. apply H. exists x; auto.
+  - intro Hf. mydestr. eapply H; eauto.
+Qed.
+
+Lemma inv_neg_not_overbasety: forall r, ¬ not_overbasety r -> (exists b n d ϕ, r = {v:b|n|d|ϕ}).
+Proof.
+  intros.
+  destruct (classic (∃ (b : base_ty) (n : nat) (d : aset) (ϕ : refinement), r = {v:b|n|d|ϕ})); auto; exfalso.
+  apply H. rewrite forall_iff_not_exists1 in H0.
+  destruct r; simpl; auto.
+  - eapply H0. repeat eexists.
+Qed.
+
+Ltac refinement_simp1 :=
+  repeat match goal with
+    | [H: context [ rty_fv (-:{v: _ | _ | _ | _}⤑ _) ] |- _ ] => simpl in H
+    | [H: context [ rty_fv (_ ⤑ _) ] |- _ ] => simpl in H
+    | [H: ¬ not_overbasety _ |- _] => apply inv_neg_not_overbasety in H; mydestr; subst
+    | [H: context [ dom aset ∅ ] |- _ ] =>
+        assert (dom aset (∅: state) = ∅) as Htmp by my_simplify_map_eq;
+        setoid_rewrite Htmp in H; try clear Htmp
+    | [H: lc_rty_idx 0 [v:_|?n|_|_] |- _ ] =>
+        match n with
+        | 0 => fail 1
+        | _ =>  assert (n = 0) by (apply lc_rty_idx_under_0_is_0 in H; auto); subst
+        end
+    end.
+
+Lemma closed_rty_cap: forall τ (d1 d2 d3: aset) n,
+    d1 ∩ d2 ⊆ d3 -> closed_rty n d1 τ -> closed_rty n d2 τ -> closed_rty n d3 τ.
+Proof.
+  induction τ; intros; invclear H0; invclear H1; mydestr; subst;
+    do 2 (constructor; auto); fast_set_solver.
+Qed.
+
+Lemma ok_dctx_single_implies_closed_rty: forall d x τ, ok_dctx d [(x, τ)] -> closed_rty 0 d τ.
+Proof.
+  intros. invclear H; auto.
+Qed.
+
+Ltac closed_rty_solver :=
+  repeat match goal with
+    | [H1: closed_rty ?n ?d1 ?τ, H2: closed_rty ?n ?d2 ?τ |- closed_rty ?n ?d3 ?τ ] =>
+            apply (closed_rty_cap τ d1 d2 d3); auto; simpl; fast_set_solver
+    | [H: closed_rty _ _ (-:{v: _ | _ | _ | _}⤑ ?τ) |- closed_rty _ _ ?τ] =>
+        destruct H; mydestr; repeat split; auto
+    | [H: valid_rty (-:{v: _ | _ | _ | _}⤑ ?τ) |- valid_rty ?τ] => invclear H; auto
+    | [H: lc_rty_idx _ (-:{v: _ | _ | _ | _}⤑ ?τ) |- lc_rty_idx _ ?τ] => invclear H; auto
+    | [H: closed_rty _ _ (-:{v: _ | _ | _ | ?ϕ}⤑ _) |- closed_rty _ _ {v: _ | _ | _ | ?ϕ}] =>
+        destruct H; mydestr; repeat split; auto
+    | [H: valid_rty (-:{v: _ | _ | _ | ?ϕ}⤑ _) |- valid_rty {v: _ | _ | _ | ?ϕ}] => invclear H; constructor; auto
+    | [H: lc_rty_idx _ (-:{v: _ | _ | _ | ?ϕ}⤑ _) |- lc_rty_idx _ {v: _ | _ | _ | ?ϕ}] => invclear H; constructor; auto
+    | [H: closed_rty _ _ (?τ1 ⤑ ?τ2) |- closed_rty _ _ ?τ1] =>
+        destruct H; mydestr; repeat split; auto
+    | [H: valid_rty (?τ1 ⤑ ?τ2) |- valid_rty ?τ1] => invclear H; auto
+    | [H: lc_rty_idx _ (?τ1 ⤑ ?τ2) |- lc_rty_idx _ ?τ1] => invclear H; auto
+    | [H: closed_rty _ _ (?τ1 ⤑ ?τ2) |- closed_rty _ _ ?τ2] =>
+        destruct H; mydestr; repeat split; auto
+    | [H: valid_rty (?τ1 ⤑ ?τ2) |- valid_rty ?τ2] => invclear H; auto
+    | [H: lc_rty_idx _ (?τ1 ⤑ ?τ2) |- lc_rty_idx _ ?τ2] => invclear H; auto
+    | [H: closed_rty ?n ?d1 ?τ |- closed_rty ?n ?d2 ?τ ] => apply (closed_rty_trans _ d1 d2); fast_set_solver
+    | [H: ok_dctx ?d [(_, ?τ)] |- closed_rty 0 ?d ?τ ] => apply ok_dctx_single_implies_closed_rty in H; auto
+    | [|- rty_fv ?x ⊆ _ ] => refinement_simp1; my_set_solver
+    end.
+
+Lemma empty_eq_app_exfalso {A: Type}: forall Γ1 (x: atom) (t: A) Γ2, ~ ([] = Γ1 ++ [(x, t)] ++ Γ2).
+Proof.
+  intros. intro H.
+  symmetry in H. apply app_eq_nil in H. mydestr.
+  apply app_eq_nil in H0. mydestr. inversion H0.
+Qed.
+
+Lemma ok_find_same {A: Type}: forall (a: atom) (τ1 τ2: A) Γ1 Γ2 Γ1' Γ2',
+    ok (Γ1 ++ ((a, τ1) :: Γ2)) -> (Γ1 ++ ((a, τ1) :: Γ2)) = (Γ1' ++ (a, τ2) :: Γ2') ->
+    Γ1 = Γ1' /\ τ1 = τ2 /\ Γ2 = Γ2'.
+Proof.
+  intros a τ1 τ2.
+  induction Γ1; intros; listctx_set_simpl2.
+  apply IHΓ1 in H0; auto. mydestr; subst.
+  repeat split; auto.
+Qed.
+
+Lemma ok_find_neq_head {A: Type}: forall (x a: atom) (τ_x τ_a: A) Γ1' Γ2 Γ2',
+    x <> a ->
+    ok ((x, τ_x) :: Γ2) -> ((x, τ_x) :: Γ2) = (Γ1' ++ (a, τ_a) :: Γ2') ->
+    (exists Γ1'', Γ1' = (x, τ_x) :: Γ1'' /\ Γ2 = (Γ1'' ++ (a, τ_a) :: Γ2')).
+Proof.
+  intros x a τ_x τ_a Γ1'.
+  induction Γ1'; intros; listctx_set_simpl2.
+  exists Γ1'. split; auto.
+Qed.
+
+Lemma ok_dctx_trans: forall Γ d1 d2,
+    d1 ⊆ d2 -> ctxdom Γ ∩ d2 ≡ ∅ -> ok_dctx d1 Γ -> ok_dctx d2 Γ.
+Proof.
+  induction Γ; intros; auto; mydestr.
+  - repeat constructor; fast_set_solver.
+  - invclear H1.
+    + constructor; eauto.
+      closed_rty_solver. my_set_solver.
+      apply (IHΓ ({[a]} ∪ d1) ({[a]} ∪ d2)); eauto; my_set_solver.
+    + apply ok_dctx_cons_arr; auto.
+      closed_rty_solver. my_set_solver.
+      apply (IHΓ d1 d2); eauto; my_set_solver.
+Qed.
+
+Lemma ok_dctx_cap: forall Γ (d1 d2 d3: aset),
+    d1 ∩ d2 ⊆ d3 -> ctxdom Γ ∩ d3 ≡ ∅ -> ok_dctx d1 Γ -> ok_dctx d2 Γ -> ok_dctx d3 Γ.
+Proof.
+  induction Γ; intros; invclear H1; invclear H2; mydestr; subst.
+  - constructor.
+  - constructor; auto. closed_rty_solver. my_set_solver.
+    apply (IHΓ ({[x]} ∪ d1) ({[x]} ∪ d2)); auto.
+    fast_set_solver. my_set_solver.
+  - exfalso; auto.
+  - exfalso; auto.
+  - apply ok_dctx_cons_arr; auto. closed_rty_solver. my_set_solver.
+    apply (IHΓ d1 d2); auto. my_set_solver.
+Qed.
+
+Lemma ok_dctx_implies_ctx_closed_rty:
+  forall Γ d, ok_dctx d Γ -> ctx_closed_rty d Γ.
+Proof.
+  induction Γ; intros. intros Γ1 x τ_x Γ2 Hin. inversion Hin. auto_exfalso.
+  invclear H.
+  - assert (ok Γ) by (apply ok_dctx_regular1 in H7; mydestr; auto).
+    apply IHΓ in H7. clear IHΓ. intros Γ1 a τ_a Γ2 Hin.
+    destruct (atom_dec x a); subst; list_simplifier.
+    + rewrite <- (app_nil_l ((a, τ) :: Γ )) in Hin.
+      apply ok_find_same in Hin; mydestr; subst. closed_rty_solver.
+      listctx_set_solver.
+    + apply (closed_rty_trans _ (ctxdom Γ1 ∪ d)); try fast_set_solver;
+      apply ok_find_neq_head in Hin; auto; mydestr; subst.
+      apply (closed_rty_trans _ (ctxdom x0 ∪ ({[x]} ∪ d))); try fast_set_solver.
+      eapply H7. list_simplifier; reflexivity.
+      listctx_set_solver.
+  - assert (ok Γ) by (apply ok_dctx_regular1 in H7; mydestr; auto).
+    apply IHΓ in H7. clear IHΓ. intros Γ1 a τ_a Γ2 Hin.
+    destruct (atom_dec x a); subst; list_simplifier.
+    + rewrite <- (app_nil_l ((a, τ) :: Γ )) in Hin.
+      apply ok_find_same in Hin; mydestr; subst. closed_rty_solver.
+      listctx_set_solver.
+    + apply (closed_rty_trans _ (ctxdom Γ1 ∪ d)); try fast_set_solver.
+      apply ok_find_neq_head in Hin; auto; mydestr; subst.
+      apply (closed_rty_trans _ (ctxdom x0 ∪ d)); try fast_set_solver.
+      eapply H7. list_simplifier; reflexivity.
+      listctx_set_solver.
+Qed.
+
+Lemma ok_dctx_regular2: forall d Γ,
+    ok_dctx d Γ -> ctx_closed_rty d Γ /\ ok Γ /\ (ctxdom Γ ∩ d ≡ ∅).
+Proof.
+  intros. split.
+  - apply ok_dctx_implies_ctx_closed_rty; auto.
+  - apply ok_dctx_regular1; auto.
+Qed.
+
+Lemma ok_dctx_shift: forall d a r Γ,
+    ok_dctx d ((a, r) :: Γ) -> ok_dctx ({[a]} ∪ d) Γ.
+Proof.
+  intros.
+  assert (({[a]} ∪ ctxdom Γ) ∩ d ≡ ∅). { apply ok_dctx_regular2 in H; mydestr. fast_set_solver. }
+  invclear H; auto. apply ok_dctx_trans with (d1:=d); eauto. fast_set_solver. set_solver.
+Qed.
+
+Ltac ok_dctx_solver1 :=
+  match goal with
+  | [H1: ok_dctx ?d1 ?τ, H2: ok_dctx ?d2 ?τ |- ok_dctx ?d3 ?τ ] =>
+            apply (ok_dctx_cap τ d1 d2 d3); auto; simpl; fast_set_solver
+  | [H: ok_dctx _ _ |- ok _ ] => apply ok_dctx_regular2 in H; mydestr; auto
+  | [H: ok_dctx _ _ |- _ ≡ _ ] => apply ok_dctx_regular2 in H; mydestr; auto
+  | [H: ok_dctx ?d1 ?τ |- ok_dctx ?d2 ?τ ] =>
+      apply (ok_dctx_trans τ d1 d2); simpl; auto; fast_set_solver
+  | [H: ok_dctx _ ((_, _) :: ?Γ) |- ok_dctx _ ?Γ] => apply ok_dctx_shift
+  end || listctx_set_solver.
+
+Fixpoint ctxdom_base (Γ: listctx rty) : aset :=
+  match Γ with
+  | [] => ∅
+  | (x, {v: _ | _ | _ | _ }) :: Γ => {[x]} ∪ ctxdom_base Γ
+  | (x, [v: _ | _ | _ | _ ]) :: Γ => {[x]} ∪ ctxdom_base Γ
+  | (x, _) :: Γ => ctxdom_base Γ
+  end.
+
+Lemma ok_dctx_post_destruct: forall Γ d x τ,
+    ok_dctx d (Γ ++ [(x, τ)]) <->
+      ok_dctx d Γ /\ x ∉ d /\ x ∉ ctxdom Γ /\ closed_rty 0 (ctxdom_base Γ ∪ d) τ.
+Proof.
+  induction Γ; simpl; split; intros; mydestr.
+  - invclear H; do 3 (constructor; auto); closed_rty_solver.
+  - destruct (classic (is_arr τ)).
+    + apply ok_dctx_cons_arr; auto; closed_rty_solver.
+    + apply ok_dctx_cons_base; auto; closed_rty_solver. constructor.
+  - invclear H.
+    + apply IHΓ in H8; mydestr. do 3 (constructor; auto; try listctx_set_solver).
+      destruct r; closed_rty_solver.
+    + apply IHΓ in H8; mydestr. do 3 (constructor; auto; try listctx_set_solver).
+      destruct r; invclear H3; closed_rty_solver.
+  - invclear H.
+    + apply ok_dctx_cons_base; auto; try listctx_set_solver.
+      rewrite IHΓ. do 3 (split; auto; try fast_set_solver).
+      destruct r; closed_rty_solver.
+    + apply ok_dctx_cons_arr; auto; try listctx_set_solver.
+      rewrite IHΓ. do 3 (split; auto; try fast_set_solver).
+      destruct r; invclear H6; closed_rty_solver.
+Qed.
+
+Ltac ok_dctx_solver2 :=
+  match goal with
+      | [H: ok_dctx ?d ((?a, ?b) :: ?l ++ [_]) |- ok_dctx ?d ((?a, ?b) :: ?l)] =>
+          rewrite app_comm_cons in H; rewrite ok_dctx_post_destruct in H; mydestr; auto
+  end || ok_dctx_solver1.
+
+Ltac ok_dctx_solver := ok_dctx_solver2.
+
+Ltac refinement_set_simp :=
+  repeat
+    match goal with
+    | [H: ok_dctx _ _ |- _ ≡ _ ] => apply ok_dctx_regular2 in H; mydestr
+    | [H: ok ((_, _) :: _) |- _ ≡ _ ] => rewrite ok_pre_destruct in H; mydestr
+    | [H: ok_dctx _ _ |- _ ⊆ _ ] => apply ok_dctx_regular2 in H; mydestr
+    | [H: ok ((_, _) :: _) |- _ ⊆ _ ] => rewrite ok_pre_destruct in H; mydestr
+    end.
+
+(* Lemma cl_dctx_trans: forall Γ d1 d2, d1 ⊆ d2 -> ctxdom Γ ∩ d2 ≡ ∅ -> cl_dctx d1 Γ -> cl_dctx d2 Γ. *)
+(* Proof. *)
+(*   induction Γ; intros; auto; mydestr. *)
+(*   - constructor. *)
+(*   - invclear H1. constructor; eauto. ok_dctx_solver. *)
+(*     apply (IHΓ ({[a]} ∪ d1)); eauto. fast_set_solver. *)
+(*     refinement_set_simp; my_set_solver. *)
+(*     closed_rty_solver. *)
+(* Qed. *)
+
+Lemma ctx_erase_perserve_ctxdom: forall Γ, ctxdom ⌊ Γ ⌋* = ctxdom Γ.
+Proof.
+  induction Γ; simpl; auto.
+  mydestr; simpl. rewrite IHΓ. auto.
+Qed.
+
+Ltac ctx_erase_simp1:=
+  repeat match goal with
+  | [H: context [ctxdom ⌊ ?Γ ⌋*] |- _ ] =>
+      setoid_rewrite (ctx_erase_perserve_ctxdom Γ) in H
+  | [ |- context [ctxdom ⌊ ?Γ ⌋*]] =>
+      setoid_rewrite (ctx_erase_perserve_ctxdom Γ)
+  end || listctx_set_simpl; simpl.
+
+Lemma ctx_erase_commute_okapp: forall Γ1 Γ2, ok ⌊ Γ1 ++ Γ2 ⌋* <-> ok ( ⌊ Γ1 ⌋* ++  ⌊ Γ2 ⌋*).
+Proof.
+  split; induction Γ1; simpl; listctx_set_simpl; intros; simpl; auto.
+  - rewrite ok_pre_destruct. rewrite ok_pre_destruct in H. mydestr.
+    split; auto. simpl in H0. ctx_erase_simp1.
+  - rewrite ok_pre_destruct. rewrite ok_pre_destruct in H. mydestr.
+    split; auto. simpl in H0. ctx_erase_simp1.
+Qed.
+
+Ltac ctx_erase_simp2:=
+  repeat match goal with
+    | [H: context [ctxdom ⌊ ?Γ ⌋*] |- _ ] =>
+        setoid_rewrite (ctx_erase_perserve_ctxdom Γ) in H
+    | [ |- context [ctxdom ⌊ ?Γ ⌋*]] =>
+        setoid_rewrite (ctx_erase_perserve_ctxdom Γ)
+    | [H: context [ ⌊ ?a ++ ?b ⌋* ] |- _ ] => rewrite (ctx_erase_commute_okapp a b) in H
+    | [ |- context [ ⌊ ?a ++ ?b ⌋* ] ] => rewrite (ctx_erase_commute_okapp a b)
+    end || listctx_set_simpl; simpl.
+
+Lemma ctx_erase_perserve_ok: forall Γ, ok Γ <-> ok ⌊ Γ ⌋*.
+Proof.
+  split; intros.
+  - induction H; simpl; auto. ctx_erase_simp2.
+    constructor; auto. ctx_erase_simp2.
+  - induction Γ; simpl; auto. mydestr. simpl in H.
+    rewrite ok_pre_destruct in H. mydestr. ctx_erase_simp2.
+    rewrite ok_pre_destruct. constructor; auto.
+Qed.
+
+Ltac ctx_erase_simp3:=
+  repeat match goal with
+    | [H: context [ctxdom ⌊ ?Γ ⌋*] |- _ ] =>
+        setoid_rewrite (ctx_erase_perserve_ctxdom Γ) in H
+    | [ |- context [ctxdom ⌊ ?Γ ⌋*]] =>
+        setoid_rewrite (ctx_erase_perserve_ctxdom Γ)
+    | [H: context [ ⌊ ?a ++ ?b ⌋* ] |- _ ] => setoid_rewrite (ctx_erase_commute_okapp a b) in H
+    | [ |- context [ ⌊ ?a ++ ?b ⌋* ] ] => setoid_rewrite (ctx_erase_commute_okapp a b)
+    | [H: context [ ok ⌊ ?a ⌋* ] |- _ ] => setoid_rewrite <- (ctx_erase_perserve_ok a) in H
+    | [ |- context [ ok ⌊ ?a ⌋* ] ] => setoid_rewrite <- (ctx_erase_perserve_ok a)
+    end || listctx_set_simpl; simpl.
+
+Ltac ctx_erase_simp:= ctx_erase_simp3.
